@prefix : <https://w3id.org/h2v#> .
@prefix owl: <http://www.w3.org/2002/07/owl#> .
@prefix rdf: <http://www.w3.org/1999/02/22-rdf-syntax-ns#> .
@prefix xml: <http://www.w3.org/XML/1998/namespace> .
@prefix xsd: <http://www.w3.org/2001/XMLSchema#> .
@prefix rdfs: <http://www.w3.org/2000/01/rdf-schema#> .
@base <https://w3id.org/h2v#> .

<https://w3id.org/h2v> rdf:type owl:Ontology ;
                        owl:versionIRI <https://w3id.org/h2v/2.0.0> ;
                        <http://purl.org/dc/elements/1.1/contributor> "Claudio Sesto (RSE)" ,
                                                                      "Francesca Soldan (RSE)" ,
                                                                      "Irene Celino (Cefriel)" ;
                        <http://purl.org/dc/elements/1.1/creator> "Gloria Re Calegari (Cefriel)" ,
                                                                  "Valentina Carriero (Cefriel)" ;
                        <http://purl.org/dc/elements/1.1/title> "Hydrogen Valley Ontology (H2V)" ;
                        <http://purl.org/dc/terms/description> "The Hydrogen Valley Ontology (H2V) models the Hydrogen Valley domain, with all its components and properties, and related activities." ;
                        <http://purl.org/dc/terms/license> <https://creativecommons.org/licenses/by/4.0/> ;
                        <http://purl.org/dc/terms/publisher> <https://ror.org/046bfkz44> ;
                        <http://purl.org/ontology/bibo/status> "Published"@en ;
                        <http://purl.org/vocab/vann/preferredNamespacePrefix> "h2v" ;
                        <http://purl.org/vocab/vann/preferredNamespaceUri> "https://w3id.org/h2v#" ;
                        rdfs:label "Hydrogen Valley Ontology (H2V)" ;
                        owl:priorVersion <https://w3id.org/h2v/1.0.0> ;
                        owl:versionInfo "2.0.0" ;
                        <https://w3id.org/mod#createdWith> <https://chowlk.linkeddata.es/> .

#################################################################
#    Annotation properties
#################################################################

###  http://purl.org/dc/elements/1.1/contributor
<http://purl.org/dc/elements/1.1/contributor> rdf:type owl:AnnotationProperty .


###  http://purl.org/dc/elements/1.1/creator
<http://purl.org/dc/elements/1.1/creator> rdf:type owl:AnnotationProperty .


###  http://purl.org/dc/elements/1.1/title
<http://purl.org/dc/elements/1.1/title> rdf:type owl:AnnotationProperty .


###  http://purl.org/dc/terms/description
<http://purl.org/dc/terms/description> rdf:type owl:AnnotationProperty .


###  http://purl.org/dc/terms/license
<http://purl.org/dc/terms/license> rdf:type owl:AnnotationProperty .


###  http://purl.org/dc/terms/publisher
<http://purl.org/dc/terms/publisher> rdf:type owl:AnnotationProperty .


###  http://purl.org/ontology/bibo/status
<http://purl.org/ontology/bibo/status> rdf:type owl:AnnotationProperty .


###  http://purl.org/vocab/vann/preferredNamespacePrefix
<http://purl.org/vocab/vann/preferredNamespacePrefix> rdf:type owl:AnnotationProperty .


###  http://purl.org/vocab/vann/preferredNamespaceUri
<http://purl.org/vocab/vann/preferredNamespaceUri> rdf:type owl:AnnotationProperty .


###  http://www.w3.org/2000/01/rdf-schema#label
rdfs:label rdf:type owl:AnnotationProperty .


###  http://www.w3.org/2002/07/owl#priorVersion
owl:priorVersion rdf:type owl:AnnotationProperty .


###  http://www.w3.org/2002/07/owl#versionIRI
owl:versionIRI rdf:type owl:AnnotationProperty .


###  http://www.w3.org/2002/07/owl#versionInfo
owl:versionInfo rdf:type owl:AnnotationProperty .


###  https://w3id.org/mod#createdWith
<https://w3id.org/mod#createdWith> rdf:type owl:AnnotationProperty .


#################################################################
#    Object Properties
#################################################################

###  http://qudt.org/schema/qudt/hasUnit
<http://qudt.org/schema/qudt/hasUnit> rdf:type owl:ObjectProperty ;
                                      rdfs:label "has unit" .


###  http://www.opengis.net/ont/geosparql#hasGeometry
<http://www.opengis.net/ont/geosparql#hasGeometry> rdf:type owl:ObjectProperty ;
                                                   rdfs:label "has geometry" .


###  http://www.w3.org/ns/sosa/hasFeatureOfInterest
<http://www.w3.org/ns/sosa/hasFeatureOfInterest> rdf:type owl:ObjectProperty ;
                                                 rdfs:label "has feature of interest" .


###  http://www.w3.org/ns/sosa/hasResult
<http://www.w3.org/ns/sosa/hasResult> rdf:type owl:ObjectProperty ;
                                      rdfs:label "has result" .


###  http://www.w3.org/ns/sosa/madeBySensor
<http://www.w3.org/ns/sosa/madeBySensor> rdf:type owl:ObjectProperty ;
                                         rdfs:label "made by sensor" .


###  http://www.w3.org/ns/sosa/observedProperty
<http://www.w3.org/ns/sosa/observedProperty> rdf:type owl:ObjectProperty ;
                                             rdfs:label "observed property" .


###  http://www.w3.org/ns/ssn/hasSubSystem
<http://www.w3.org/ns/ssn/hasSubSystem> rdf:type owl:ObjectProperty ;
                                        rdfs:label "has sub system" .


###  https://saref.etsi.org/core/hasPropertyKind
<https://saref.etsi.org/core/hasPropertyKind> rdf:type owl:ObjectProperty ;
                                              rdfs:label "has property kind" .


###  https://saref.etsi.org/core/hasPropertyOfInterest
<https://saref.etsi.org/core/hasPropertyOfInterest> rdf:type owl:ObjectProperty ;
                                                    rdfs:label "has property of interest" .


###  https://w3id.org/h2v#allocatedBy
:allocatedBy rdf:type owl:ObjectProperty ;
             rdfs:domain :HydrogenAllocation ;
             rdfs:range <http://www.w3.org/ns/ssn/System> ;
             rdfs:comment "This property links an Hydrogen Allocation activity to the System that is allocating hydrogen to another system."^^rdfs:Literal ;
             rdfs:label "allocated by" .


###  https://w3id.org/h2v#allocatedTo
:allocatedTo rdf:type owl:ObjectProperty ;
             rdfs:domain :HydrogenAllocation ;
             rdfs:range <http://www.w3.org/ns/ssn/System> ;
             rdfs:comment "This property links an Hydrogen Allocation activity to the System that is receiving hydrogen from another system. "^^rdfs:Literal ;
             rdfs:label "allocated to" .


###  https://w3id.org/h2v#appliesToSystem
:appliesToSystem rdf:type owl:ObjectProperty ;
                 rdfs:domain <http://www.w3.org/ns/ssn/Property> ;
                 rdfs:range <http://www.w3.org/ns/ssn/System> ;
                 rdfs:comment "This property links a Property to the System(s) it applies to. "^^rdfs:Literal ;
                 rdfs:label "applies to system" .


###  https://w3id.org/h2v#forecastedProperty
:forecastedProperty rdf:type owl:ObjectProperty ;
                    rdfs:domain :Forecast ;
                    rdfs:range :DynamicProperty ;
                    rdfs:comment "This property links a Forecast to the Dynamic Property the forecast is about."^^rdfs:Literal ;
                    rdfs:label "forecasted property" .


###  https://w3id.org/h2v#hasAllocatedValue
:hasAllocatedValue rdf:type owl:ObjectProperty ;
                   rdfs:domain :HydrogenAllocation ;
                   rdfs:range <http://qudt.org/schema/qudt/QuantityValue> ;
                   rdfs:comment "This property links an Hydrogen Allocation activity to the amount of hydrogen that is being allocated."^^rdfs:Literal ;
                   rdfs:label "has allocated value" .


###  https://w3id.org/h2v#hasExporter
:hasExporter rdf:type owl:ObjectProperty ;
             rdfs:domain :HydrogenImportExport ;
             rdfs:range <http://www.w3.org/ns/ssn/System> ;
             rdfs:comment "This property links an Hydrogen Import Export activity to the System that is exporting to another system."^^rdfs:Literal ;
             rdfs:label "has exporter" .


###  https://w3id.org/h2v#hasForecastedValue
:hasForecastedValue rdf:type owl:ObjectProperty ;
                    rdfs:domain :Forecast ;
                    rdfs:range <http://qudt.org/schema/qudt/QuantityValue> ;
                    rdfs:comment "This property links a Forecast to the Quantity Value of the Dynamic Property that the forecast is about."^^rdfs:Literal ;
                    rdfs:label "has forecasted value" .


###  https://w3id.org/h2v#hasImportedExportedValue
:hasImportedExportedValue rdf:type owl:ObjectProperty ;
                          rdfs:domain :HydrogenImportExport ;
                          rdfs:range <http://qudt.org/schema/qudt/QuantityValue> ;
                          rdfs:comment "This property links an Hydrogen Import Export activity to the amount of hydrogen that is being imported/exported."^^rdfs:Literal ;
                          rdfs:label "has imported exported value" .


###  https://w3id.org/h2v#hasImporter
:hasImporter rdf:type owl:ObjectProperty ;
             rdfs:domain :HydrogenImportExport ;
             rdfs:range <http://www.w3.org/ns/ssn/System> ;
             rdfs:comment "This property links an Hydrogen Import Export activity to the System that is importing from another system."^^rdfs:Literal ;
             rdfs:label "has importer" .


###  https://w3id.org/h2v#hasMaximumPropertyMember
:hasMaximumPropertyMember rdf:type owl:ObjectProperty ;
                          rdfs:subPropertyOf :hasPropertyMember ;
                          rdfs:domain :PropertySet ;
                          rdfs:range :StaticProperty ;
                          rdfs:comment "This property links a Property Set to the member property that is considered the maximum of a range."^^rdfs:Literal ;
                          rdfs:label "has maximum property member" .


###  https://w3id.org/h2v#hasMinimumPropertyMember
:hasMinimumPropertyMember rdf:type owl:ObjectProperty ;
                          rdfs:subPropertyOf :hasPropertyMember ;
                          rdfs:domain :PropertySet ;
                          rdfs:range :StaticProperty ;
                          rdfs:comment "This property links a Property Set to the member property that is considered the minimum of a range."^^rdfs:Literal ;
                          rdfs:label "has minimum property member" .


###  https://w3id.org/h2v#hasOptimalPropertyMember
:hasOptimalPropertyMember rdf:type owl:ObjectProperty ;
                          rdfs:subPropertyOf :hasPropertyMember ;
                          rdfs:domain :PropertySet ;
                          rdfs:range :StaticProperty ;
                          rdfs:comment "This property links a Property Set to the member property that is considered the optimal with respect to a range, that is ."^^rdfs:Literal ;
                          rdfs:label "has optimal property member" .


###  https://w3id.org/h2v#hasPropertyMember
:hasPropertyMember rdf:type owl:ObjectProperty ;
                   rdfs:domain :PropertySet ;
                   rdfs:range :StaticProperty ;
                   rdfs:comment "This property links a Property Set to the Properties that are its members."^^rdfs:Literal ;
                   rdfs:label "has property member" .


###  https://w3id.org/h2v#hasPropertyValue
:hasPropertyValue rdf:type owl:ObjectProperty ;
                  rdfs:domain <https://saref.etsi.org/core/PropertyOfInterest> ;
                  rdfs:range <http://qudt.org/schema/qudt/QuantityValue> ;
                  rdfs:comment "This property links a Property of Interest, which is a property specific to a feature of interest, to its value, that is the actual value of that property specific to that feature of interest."^^rdfs:Literal ;
                  rdfs:label "has property value" .


###  https://w3id.org/h2v#hasTechnicalDrawing
:hasTechnicalDrawing rdf:type owl:ObjectProperty ;
                     rdfs:domain <http://www.w3.org/ns/ssn/System> ;
                     rdfs:range :TechnicalDrawing ;
                     rdfs:comment "This property links an Hydrogen Valley to its Technical Drawing."^^rdfs:Literal ;
                     rdfs:label "has technical drawing" .


###  https://w3id.org/h2v#hasTerminal
:hasTerminal rdf:type owl:ObjectProperty ;
             rdfs:domain <http://www.w3.org/ns/ssn/System> ;
             rdfs:range :Terminal ;
             rdfs:comment "This property links a System to (one of) its Terminal(s)."^^rdfs:Literal ;
             rdfs:label "has terminal" .


###  https://w3id.org/h2v#inTechnicalDrawing
:inTechnicalDrawing rdf:type owl:ObjectProperty ;
                    rdfs:domain <http://www.opengis.net/ont/geosparql#Geometry> ;
                    rdfs:range :TechnicalDrawing ;
                    rdfs:comment "This property links a Geometry (e.g., point, polygon) to the Technical Drawing it is included in."^^rdfs:Literal ;
                    rdfs:label "in technical drawing" .


###  https://w3id.org/h2v#includesTerminal
:includesTerminal rdf:type owl:ObjectProperty ;
                  rdfs:domain :ConnectivityNode ;
                  rdfs:range :Terminal ;
                  rdfs:comment "This property links a Connectivity Node to (one of) the Terminal(s) it includes, that is all terminals that are physically connected together in the connectivity node."^^rdfs:Literal ;
                  rdfs:label "includes terminal" .


###  https://w3id.org/h2v#isIncludedInConnectivityNode
:isIncludedInConnectivityNode rdf:type owl:ObjectProperty ;
                              rdfs:domain :Terminal ;
                              rdfs:range :ConnectivityNode ;
                              rdfs:comment "This property links a Terminal to the Connectivity Node it is included in, that is, a physical connection point grouping all terminals that are physically connected together."^^rdfs:Literal ;
                              rdfs:label "is included in connectivity node" .


###  https://w3id.org/h2v#isTechnicalDrawingOf
:isTechnicalDrawingOf rdf:type owl:ObjectProperty ;
                      rdfs:domain :TechnicalDrawing ;
                      rdfs:range <http://www.w3.org/ns/ssn/System> ;
                      rdfs:comment "This property links a Technical Drawing to the Hydrogen Valley it represents."^^rdfs:Literal ;
                      rdfs:label "is technical drawing of" .


###  https://w3id.org/h2v#isTerminalOf
:isTerminalOf rdf:type owl:ObjectProperty ;
              rdfs:domain :Terminal ;
              rdfs:range <http://www.w3.org/ns/ssn/System> ;
              rdfs:comment "This property links a Terminal to the System it is a part of."^^rdfs:Literal ;
              rdfs:label "is terminal of" .


###  https://w3id.org/h2v#refersToFeature
:refersToFeature rdf:type owl:ObjectProperty ;
                 rdfs:domain :WeatherForecast ;
                 rdfs:range <http://www.opengis.net/ont/geosparql#Feature> ;
                 rdfs:comment "This property links a Weather Forecast to the geographical Feature to which the forecast applies."^^rdfs:Literal ;
                 rdfs:label "refers to feature" .


###  https://w3id.org/h2v#refersToFeatureOfInterest
:refersToFeatureOfInterest rdf:type owl:ObjectProperty ;
                           rdfs:domain :Forecast ;
                           rdfs:range <http://www.w3.org/ns/ssn/System> ;
                           rdfs:comment "This property links a Forecast to the Feature Of Interest (i.e., a System) to which the forecast applies."^^rdfs:Literal ;
                           rdfs:label "refers to feature of interest" .


#################################################################
#    Data properties
#################################################################

###  http://purl.org/dc/terms/description
<http://purl.org/dc/terms/description> rdf:type owl:DatatypeProperty .


###  http://purl.org/dc/terms/identifier
<http://purl.org/dc/terms/identifier> rdf:type owl:DatatypeProperty ;
                                      rdfs:label "identifier" .


###  http://purl.org/dc/terms/title
<http://purl.org/dc/terms/title> rdf:type owl:DatatypeProperty ;
                                 rdfs:label "title" .


###  http://qudt.org/schema/qudt/numericValue
<http://qudt.org/schema/qudt/numericValue> rdf:type owl:DatatypeProperty ;
                                           rdfs:label "numeric value" .


###  http://www.w3.org/ns/dcat#accessURL
<http://www.w3.org/ns/dcat#accessURL> rdf:type owl:DatatypeProperty ;
                                      rdfs:label "access u r l" .


###  http://www.w3.org/ns/prov#atTime
<http://www.w3.org/ns/prov#atTime> rdf:type owl:DatatypeProperty ;
                                   rdfs:label "at time" .


###  http://www.w3.org/ns/sosa/resultTime
<http://www.w3.org/ns/sosa/resultTime> rdf:type owl:DatatypeProperty ;
                                       rdfs:label "result time" .


###  https://w3id.org/h2v#forecastedForTime
:forecastedForTime rdf:type owl:DatatypeProperty ;
                   rdfs:domain :Forecast ;
                   rdfs:range xsd:dateTime ;
                   rdfs:comment "This property links a Forecast to the time in the future that the Forecast refers to."^^rdfs:Literal ;
                   rdfs:label "forecasted for time" .


###  https://w3id.org/h2v#issuedAtTime
:issuedAtTime rdf:type owl:DatatypeProperty ;
              rdfs:domain :Forecast ;
              rdfs:range xsd:dateTime ;
              rdfs:comment "This property link a Forecast to the time when a Forecast has been issued."^^rdfs:Literal ;
              rdfs:label "issued at time" .


#################################################################
#    Classes
#################################################################

###  http://qudt.org/schema/qudt/QuantityValue
<http://qudt.org/schema/qudt/QuantityValue> rdf:type owl:Class ;
                                            rdfs:label "Quantity Value" .


###  http://qudt.org/schema/qudt/Unit
<http://qudt.org/schema/qudt/Unit> rdf:type owl:Class ;
                                   rdfs:label "Unit" .


###  http://www.opengis.net/ont/geosparql#Feature
<http://www.opengis.net/ont/geosparql#Feature> rdf:type owl:Class ;
                                               rdfs:label "Feature" .


###  http://www.opengis.net/ont/geosparql#Geometry
<http://www.opengis.net/ont/geosparql#Geometry> rdf:type owl:Class ;
                                                rdfs:label "Geometry" .


###  http://www.w3.org/ns/prov#Activity
<http://www.w3.org/ns/prov#Activity> rdf:type owl:Class ;
                                     rdfs:label "Activity" .


###  http://www.w3.org/ns/sosa/ObservableProperty
<http://www.w3.org/ns/sosa/ObservableProperty> rdf:type owl:Class ;
                                               rdfs:label "Observable Property" .


###  http://www.w3.org/ns/sosa/Observation
<http://www.w3.org/ns/sosa/Observation> rdf:type owl:Class ;
                                        rdfs:label "Observation" .


###  http://www.w3.org/ns/sosa/Sensor
<http://www.w3.org/ns/sosa/Sensor> rdf:type owl:Class ;
                                   rdfs:label "Sensor" .


###  http://www.w3.org/ns/ssn/Property
<http://www.w3.org/ns/ssn/Property> rdf:type owl:Class ;
                                    rdfs:label "Property" .


###  http://www.w3.org/ns/ssn/System
<http://www.w3.org/ns/ssn/System> rdf:type owl:Class ;
                                  rdfs:label "System" .


###  https://saref.etsi.org/core/PropertyOfInterest
<https://saref.etsi.org/core/PropertyOfInterest> rdf:type owl:Class ;
                                                 rdfs:label "Property Of Interest" .


###  https://w3id.org/h2v#ActuatedOn-OffValve
:ActuatedOn-OffValve rdf:type owl:Class ;
                     rdfs:subClassOf :Valve ;
                     rdfs:comment "An Actuated On-Off Valve is a remoted controlled valve that either can be fully open or fully closed. An actuated on-off valve is part of the macrocomponent Hydrogen Production Area."^^rdfs:Literal ;
                     rdfs:label "Actuated On- Off Valve" .


###  https://w3id.org/h2v#Blender
:Blender rdf:type owl:Class ;
         rdfs:subClassOf :PointDevice ;
         rdfs:comment "The Blender is the transfer point of the HV with the gas network. The blender is a specific type of Point Device."^^rdfs:Literal ;
         rdfs:label "Blender" .


###  https://w3id.org/h2v#ConnectivityNode
:ConnectivityNode rdf:type owl:Class ;
                  rdfs:comment "The Connectivity Node within an HV is a point where terminals of (pieces of) pipes are connected together"^^rdfs:Literal ;
                  rdfs:label "Connectivity Node" ;
                  rdfs:seeAlso "https://cim.fein-aachen.org/libcimpp/doc/IEC61970_17v23/classIEC61970_1_1Base_1_1Core_1_1ConnectivityNode.html"^^rdfs:Literal .


###  https://w3id.org/h2v#DynamicProperty
:DynamicProperty rdf:type owl:Class ;
                 rdfs:subClassOf <http://www.w3.org/ns/sosa/ObservableProperty> ;
                 rdfs:comment "A Dynamic Property is a time-varying Property of a System that is dynamically observed or measured."^^rdfs:Literal ;
                 rdfs:label "Dynamic Property" .


###  https://w3id.org/h2v#ElectricityProductionArea
:ElectricityProductionArea rdf:type owl:Class ;
                           rdfs:subClassOf :HydrogenValleyArea ;
                           rdfs:comment "An Electricity Production Area is the geographical polygon where the hydrogen storage is located (given by a list of coordinates)."^^rdfs:Literal ;
                           rdfs:label "Electricity Production Area" .


###  https://w3id.org/h2v#Electrolyzer
:Electrolyzer rdf:type owl:Class ;
              rdfs:subClassOf <http://www.w3.org/ns/ssn/System> ;
              rdfs:comment "An Electrolyzer is a system that uses electrical energy to split water into hydrogen and oxygen. An electrolyzer is part of the macrocomponent Hydrogen Production Area"^^rdfs:Literal ;
              rdfs:label "Electrolyzer" .


###  https://w3id.org/h2v#FlowMeasuringSensor
:FlowMeasuringSensor rdf:type owl:Class ;
                     rdfs:subClassOf <http://www.w3.org/ns/sosa/Sensor> ;
                     rdfs:comment "The Flow Measuring Sensor is a tool used for measuring the flow of a fluid in a pipe"^^rdfs:Literal ;
                     rdfs:label "Flow Measuring Sensor" .


###  https://w3id.org/h2v#Forecast
:Forecast rdf:type owl:Class ;
          rdfs:subClassOf <http://www.w3.org/ns/prov#Activity> ;
          rdfs:comment "A Forecast is an activity that produces a prediction about the future value of some property, based on models, data, or prior observations."^^rdfs:Literal ;
          rdfs:label "Forecast" .


###  https://w3id.org/h2v#FuelCell
:FuelCell rdf:type owl:Class ;
          rdfs:subClassOf :PointDevice ;
          rdfs:comment "A Fuel Cell is a system that converts the chemical energy of a fuel (Hydrogen) into electricity through redox reaction. A Fuel Cell is a specific type of Point Device. A Fuel Cell is part of the macrocomponent Hydrogen Consumption Area."^^rdfs:Literal ;
          rdfs:label "Fuel Cell" .


###  https://w3id.org/h2v#GlobeValve
:GlobeValve rdf:type owl:Class ;
            rdfs:subClassOf :Valve ;
            rdfs:comment "A globe valve is a valve that allows to adjust the flow. A globe control valve is part of the macrocomponent Hydrogen Production Area."^^rdfs:Literal ;
            rdfs:label "Globe Valve" .


###  https://w3id.org/h2v#HydrogenAllocation
:HydrogenAllocation rdf:type owl:Class ;
                    rdfs:subClassOf <http://www.w3.org/ns/prov#Activity> ;
                    rdfs:comment "An Hydrogen Allocation is an activity in which an amount of hydrogen is allocated by a System, usually an Hydrogen Valley, to another System (e.g., an Hydrogen Consumer)."^^rdfs:Literal ;
                    rdfs:label "Hydrogen Allocation" .


###  https://w3id.org/h2v#HydrogenConsumer
:HydrogenConsumer rdf:type owl:Class ;
                  rdfs:subClassOf <http://www.w3.org/ns/ssn/System> ;
                  rdfs:comment "A Hydrogen Consumer is a system that uses hydrogen for various purposes, such as industry, transportation, or energy production. The Hydrogen Consumer is part of the macrocomponent Hydrogen Consumption Area."^^rdfs:Literal ;
                  rdfs:label "Hydrogen Consumer" .


###  https://w3id.org/h2v#HydrogenConsumptionArea
:HydrogenConsumptionArea rdf:type owl:Class ;
                         rdfs:subClassOf :HydrogenValleyArea ;
                         rdfs:comment "A Hydrogen Consumption Area is the geographical polygon where the hydrogen consumer is located (given by a list of coordinates)."^^rdfs:Literal ;
                         rdfs:label "Hydrogen Consumption Area" .


###  https://w3id.org/h2v#HydrogenImportExport
:HydrogenImportExport rdf:type owl:Class ;
                      rdfs:subClassOf <http://www.w3.org/ns/prov#Activity> ;
                      rdfs:comment "An Hydrogen Import Export is an activity in which an amount of hydrogen is exchanged between two systems, that is, an hydrogen importer and an hydrogen exporter."^^rdfs:Literal ;
                      rdfs:label "Hydrogen Import Export" .


###  https://w3id.org/h2v#HydrogenProductionArea
:HydrogenProductionArea rdf:type owl:Class ;
                        rdfs:subClassOf :HydrogenValleyArea ;
                        rdfs:comment "A Hydrogen Production Area is the geographical polygon where the electrolyzer is located (given by a list of coordinates)."^^rdfs:Literal ;
                        rdfs:label "Hydrogen Production Area" .


###  https://w3id.org/h2v#HydrogenStorage
:HydrogenStorage rdf:type owl:Class ;
                 rdfs:subClassOf <http://www.w3.org/ns/ssn/System> ;
                 rdfs:comment "A Hydrogen Storage is the system for storing the produced hydrogen, which can be stored in compressed gaseous form, as a liquid, or through other methods. Hydrogen storage is essential to ensure system flexibility and to balance energy production and demand. The Hydrogen Storage is the interface for import/export operations. The Hydrogen Storage is part of the macrocomponent Hydrogen Storage Area."^^rdfs:Literal ;
                 rdfs:label "Hydrogen Storage" .


###  https://w3id.org/h2v#HydrogenStorageArea
:HydrogenStorageArea rdf:type owl:Class ;
                     rdfs:subClassOf :HydrogenValleyArea ;
                     rdfs:comment "A Hydrogen Storage Area is the geographical polygon where the hydrogen storage is located (given by a list of coordinates)."^^rdfs:Literal ;
                     rdfs:label "Hydrogen Storage Area" .


###  https://w3id.org/h2v#HydrogenValley
:HydrogenValley rdf:type owl:Class ;
                rdfs:subClassOf <http://www.w3.org/ns/ssn/System> ;
                rdfs:comment "A Hydrogen Valley (HV) is a geographic area—such as a city, region, island, or industrial cluster—where various hydrogen applications are combined into an integrated hydrogen ecosystem that consumes a significant amount of hydrogen. An Hydrogen Valley can therefore encompass the entire hydrogen value chain: production, storage, distribution, and end use."^^rdfs:Literal ;
                rdfs:label "Hydrogen Valley" .


###  https://w3id.org/h2v#HydrogenValleyArea
:HydrogenValleyArea rdf:type owl:Class ;
                    rdfs:subClassOf <http://www.w3.org/ns/ssn/System> ;
                    rdfs:comment "A Hydrogen Valley Area is a System within a Hydrogen Valley that corresponds to a zone where specific hydrogen-related activities, like hydrogen storage or consumption, take place. An HydrogenValleyArea has at least one SubSystem. "^^rdfs:Literal ;
                    rdfs:label "Hydrogen Valley Area" .


###  https://w3id.org/h2v#HydrogenValleyComponent
:HydrogenValleyComponent rdf:type owl:Class ;
                         rdfs:subClassOf <http://www.w3.org/ns/ssn/System> ;
                         rdfs:comment "A Hydrogen Valley Component is a System within a Hydrogen Valley that contributes to the hydrogen value chain, such as hydrogen production. "^^rdfs:Literal ;
                         rdfs:label "Hydrogen Valley Component" .


###  https://w3id.org/h2v#LevelMeasuringSensor
:LevelMeasuringSensor rdf:type owl:Class ;
                      rdfs:subClassOf <http://www.w3.org/ns/sosa/Sensor> ;
                      rdfs:comment "The Level Measuring Sensor is a tool used for measuring the volume of a liquid in a tank"^^rdfs:Literal ;
                      rdfs:label "Level Measuring Sensor" .


###  https://w3id.org/h2v#ManualValve
:ManualValve rdf:type owl:Class ;
             rdfs:subClassOf :Valve ;
             rdfs:comment "A Manual Valve is a manual controlled valve that either can be fully open or fully closed. A manual valve is part of the macrocomponent Hydrogen Production Area."^^rdfs:Literal ;
             rdfs:label "Manual Valve" .


###  https://w3id.org/h2v#PhotovoltaicSystem
:PhotovoltaicSystem rdf:type owl:Class ;
                    rdfs:subClassOf :RESPlant ;
                    rdfs:comment "A Photovoltaic System is a complete electrical system that generates electricity from sunlight using solar panels. It comprises various components, including solar panels, inverters, and potentially batteries."^^rdfs:Literal ;
                    rdfs:label "Photovoltaic System" ;
                    rdfs:seeAlso "https://cim.fein-aachen.org/libcimpp/doc/IEC61970_17v23/classIEC61970_1_1Base_1_1Generation_1_1Production_1_1PhotoVoltaicUnit.html"^^rdfs:Literal .


###  https://w3id.org/h2v#Pipe
:Pipe rdf:type owl:Class ;
      rdfs:subClassOf <http://www.w3.org/ns/ssn/System> ;
      rdfs:comment "A Hydrogen Pipe is the system used to transport hydrogen gas across the different systems of a HV. The pipe connects a component X to a component Y."^^rdfs:Literal ;
      rdfs:label "Pipe" .


###  https://w3id.org/h2v#PointDevice
:PointDevice rdf:type owl:Class ;
             rdfs:subClassOf <http://www.w3.org/ns/ssn/System> ;
             rdfs:comment "The Point Device is the device for the exchange of energy vectors in general (hydrogen with heat/gas/electricity)"^^rdfs:Literal ;
             rdfs:label "Point Device" .


###  https://w3id.org/h2v#PressureControlValve
:PressureControlValve rdf:type owl:Class ;
                      rdfs:subClassOf :Valve ;
                      rdfs:comment "A Pressure Control Valve is a valve that adjusts the outlet pressure. A pressure control valve is part of the macrocomponent Hydrogen Production Area."^^rdfs:Literal ;
                      rdfs:label "Pressure Control Valve" .


###  https://w3id.org/h2v#PressureMeasuringSensor
:PressureMeasuringSensor rdf:type owl:Class ;
                         rdfs:subClassOf <http://www.w3.org/ns/sosa/Sensor> ;
                         rdfs:comment "The Pressure Measuring Sensor is a tool used for measuring the pressure of a gas in a pipe or in a gas tank."^^rdfs:Literal ;
                         rdfs:label "Pressure Measuring Sensor" .


###  https://w3id.org/h2v#PropertySet
:PropertySet rdf:type owl:Class ;
             rdfs:comment "A Property Set is a group of Properties, that are grouped for a specific purpose. They are usually members of a range (maximum/minimum), with a possible optimal value within the range."^^rdfs:Literal ;
             rdfs:label "Property Set" .


###  https://w3id.org/h2v#RESPlant
:RESPlant rdf:type owl:Class ;
          rdfs:subClassOf <http://www.w3.org/ns/ssn/System> ;
          rdfs:comment "A RES Plant is renewable energy system that powers the electrolyzer. This can be a photovoltaic, wind, hydroelectric, or geothermal plant. Its capacity and production profile directly affect the amount of green hydrogen that can be generated. An RES plant is part of the macrocomponent Electricity Production Area."^^rdfs:Literal ;
          rdfs:label "R E S Plant" .


###  https://w3id.org/h2v#StaticProperty
:StaticProperty rdf:type owl:Class ;
                rdfs:subClassOf <http://www.w3.org/ns/ssn/Property> ;
                rdfs:comment "A Static Property is a nominal Property of a System, typically defined by design or manufacturer specifications, that is not meant to be dynamically observed."^^rdfs:Literal ;
                rdfs:label "Static Property" .


###  https://w3id.org/h2v#TechnicalDrawing
:TechnicalDrawing rdf:type owl:Class ;
                  rdfs:comment "The technical drawing of an HV is the graphic representation of the HV, showing all the components included in the HV."^^rdfs:Literal ;
                  rdfs:label "Technical Drawing" .


###  https://w3id.org/h2v#TemperatureMeasuringSensor
:TemperatureMeasuringSensor rdf:type owl:Class ;
                            rdfs:subClassOf <http://www.w3.org/ns/sosa/Sensor> ;
                            rdfs:comment "The Temperature Measuring Sensor is a tool used for measuring the temperature of a fluid in a pipe or in a tank."^^rdfs:Literal ;
                            rdfs:label "Temperature Measuring Sensor" .


###  https://w3id.org/h2v#Terminal
:Terminal rdf:type owl:Class ;
          rdfs:comment "The Terminal of an HV Component is a connection point to a piece of pipe. Terminals are connected at physical connection points called connectivity nodes. A terminal, or multiple terminals, of an HV Component can be included in a connectivity node, meaning that all terminals in a connectivity node are physically connected together."^^rdfs:Literal ;
          rdfs:label "Terminal" ;
          rdfs:seeAlso "https://cim.fein-aachen.org/libcimpp/doc/IEC61970_17v23/classIEC61970_1_1Base_1_1Core_1_1ACDCTerminal.html"^^rdfs:Literal .


###  https://w3id.org/h2v#Valve
:Valve rdf:type owl:Class ;
       rdfs:subClassOf <http://www.w3.org/ns/ssn/System> ;
       rdfs:label "Valve" .


###  https://w3id.org/h2v#WaterPump
:WaterPump rdf:type owl:Class ;
           rdfs:subClassOf <http://www.w3.org/ns/ssn/System> ;
           rdfs:comment "A water pump is a system that allows water flow from water tank to electrolyzer. A water pump is part of the macrocomponent Hydrogen Production Area."^^rdfs:Literal ;
           rdfs:label "Water Pump" .


###  https://w3id.org/h2v#WaterTank
:WaterTank rdf:type owl:Class ;
           rdfs:subClassOf <http://www.w3.org/ns/ssn/System> ;
           rdfs:comment "A Water Tank is a storage system for distilled water used as water source for the electrolyzer. A water tank is part of the macrocomponent Hydrogen Production Area."^^rdfs:Literal ;
           rdfs:label "Water Tank" .


###  https://w3id.org/h2v#WeatherForecast
:WeatherForecast rdf:type owl:Class ;
                 rdfs:subClassOf :Forecast ;
                 rdfs:comment "A Forecast is an activity that produces a prediction about the future value of some weather property, based on models, data, or prior observations."^^rdfs:Literal ;
                 rdfs:label "Weather Forecast" .


###  https://w3id.org/h2v#WeatherProperty
:WeatherProperty rdf:type owl:Class ;
                 rdfs:subClassOf :DynamicProperty ;
                 rdfs:comment "A Weather Property is a specific type of Dynamic Property related to the weather."^^rdfs:Literal ;
                 rdfs:label "Weather Property" .


#################################################################
#    Annotations
#################################################################

<http://purl.org/dc/terms/description> rdfs:label "description" .


:BARG rdfs:comment "The BARG is a pressure unit measure used to express gauge pressure, which is the pressure above atmospheric pressure and is calculated by subtracting atmospheric pressure from the absolute pressure measured in bars."^^rdfs:Literal .


###  Generated by the OWL API (version 5.1.18) https://github.com/owlcs/owlapi/
