@prefix : <https://w3id.org/h2v/property#> .
@prefix owl: <http://www.w3.org/2002/07/owl#> .
@prefix rdf: <http://www.w3.org/1999/02/22-rdf-syntax-ns#> .
@prefix xml: <http://www.w3.org/XML/1998/namespace> .
@prefix xsd: <http://www.w3.org/2001/XMLSchema#> .
@prefix rdfs: <http://www.w3.org/2000/01/rdf-schema#> .
@base <https://w3id.org/h2v/property#> .

<https://w3id.org/h2v/property#> rdf:type owl:Ontology ;
                                  owl:versionIRI <https://w3id.org/h2v/property/2.0.0> ;
                                  <http://purl.org/dc/terms/contributor> "Claudio Sesto (RSE)" ,
                                                                         "Irene Celino (Cefriel)" ;
                                  <http://purl.org/dc/terms/creator> "Gloria Re Calegari (Cefriel)" ,
                                                                     "Valentina Carriero (Cefriel)" ;
                                  <http://purl.org/dc/terms/license> <https://creativecommons.org/licenses/by/4.0/> ;
                                  <http://purl.org/dc/terms/publisher> "Cefriel" ;
                                  <http://purl.org/dc/terms/title> "Hydrogen Valley Ontology (H2V) - Property module" ;
                                  <http://purl.org/ontology/bibo/status> "Published"@en ;
                                  rdfs:label "Hydrogen Valley Ontology (H2V) - Property module" ;
                                  owl:priorVersion <https://w3id.org/h2v/property/1.0.0> ;
                                  owl:versionInfo "2.0.0" .

#################################################################
#    Annotation properties
#################################################################

###  http://purl.org/dc/terms/contributor
<http://purl.org/dc/terms/contributor> rdf:type owl:AnnotationProperty .


###  http://purl.org/dc/terms/creator
<http://purl.org/dc/terms/creator> rdf:type owl:AnnotationProperty .


###  http://purl.org/dc/terms/license
<http://purl.org/dc/terms/license> rdf:type owl:AnnotationProperty .


###  http://purl.org/dc/terms/publisher
<http://purl.org/dc/terms/publisher> rdf:type owl:AnnotationProperty .


###  http://purl.org/dc/terms/title
<http://purl.org/dc/terms/title> rdf:type owl:AnnotationProperty .


###  http://purl.org/ontology/bibo/status
<http://purl.org/ontology/bibo/status> rdf:type owl:AnnotationProperty .


###  http://qudt.org/schema/qudt/applicableUnit
<http://qudt.org/schema/qudt/applicableUnit> rdf:type owl:AnnotationProperty .


###  http://www.w3.org/2004/02/skos/core#broader
<http://www.w3.org/2004/02/skos/core#broader> rdf:type owl:AnnotationProperty .


###  https://w3id.org/h2v#appliesToSystem
<https://w3id.org/h2v#appliesToSystem> rdf:type owl:AnnotationProperty .


###  https://w3id.org/h2v#hasMaximumPropertyMember
<https://w3id.org/h2v#hasMaximumPropertyMember> rdf:type owl:AnnotationProperty .


###  https://w3id.org/h2v#hasMinimumPropertyMember
<https://w3id.org/h2v#hasMinimumPropertyMember> rdf:type owl:AnnotationProperty .


###  https://w3id.org/h2v#hasOptimalPropertyMember
<https://w3id.org/h2v#hasOptimalPropertyMember> rdf:type owl:AnnotationProperty .


###  https://w3id.org/h2v#hasPropertyMember
<https://w3id.org/h2v#hasPropertyMember> rdf:type owl:AnnotationProperty .


#################################################################
#    Classes
#################################################################

###  https://w3id.org/h2v#DynamicProperty
<https://w3id.org/h2v#DynamicProperty> rdf:type owl:Class .


###  https://w3id.org/h2v#PropertySet
<https://w3id.org/h2v#PropertySet> rdf:type owl:Class .


###  https://w3id.org/h2v#StaticProperty
<https://w3id.org/h2v#StaticProperty> rdf:type owl:Class .


###  https://w3id.org/h2v#WeatherProperty
<https://w3id.org/h2v#WeatherProperty> rdf:type owl:Class .


#################################################################
#    Individuals
#################################################################

###  https://w3id.org/h2v/property#ActualStorageSizeMax
:ActualStorageSizeMax rdf:type owl:NamedIndividual ,
                               <https://w3id.org/h2v#DynamicProperty> ;
                      <http://qudt.org/schema/qudt/applicableUnit> <http://qudt.org/vocab/unit/KiloGM> ;
                      rdfs:comment "The Actual Storage Size Max [kg] of the storage of the HV is the maximum quantity of hydrogen that can be stored based on thermodynamic conditions"^^rdfs:Literal ;
                      rdfs:label "Actual Storage Size Max"^^rdfs:Literal ;
                      <http://www.w3.org/2004/02/skos/core#broader> <http://qudt.org/vocab/quantitykind/Mass> ;
                      <https://w3id.org/h2v#appliesToSystem> <https://w3id.org/h2v#HydrogenStorage> .


###  https://w3id.org/h2v/property#ActuatedOn-OffValveNormalOpen
:ActuatedOn-OffValveNormalOpen rdf:type owl:NamedIndividual ,
                                        <https://w3id.org/h2v#StaticProperty> ;
                               <http://qudt.org/schema/qudt/applicableUnit> <http://qudt.org/vocab/unit/UNITLESS> ;
                               rdfs:comment "The Actuated On-Off Valve Normal Open [boolean] is used when no measurements for the state of the value is present. If the value is 1, the valve is normally open, if the value is 0, the valve is normally closed."^^rdfs:Literal ;
                               rdfs:label "Actuated On-Off Valve Normal Open "^^rdfs:Literal ;
                               <http://www.w3.org/2004/02/skos/core#broader> <http://qudt.org/vocab/quantitykind/Dimensionless> ;
                               <https://w3id.org/h2v#appliesToSystem> <https://w3id.org/h2v#ActuatedOn-OffValve> .


###  https://w3id.org/h2v/property#ActuatedOn-OffValveState
:ActuatedOn-OffValveState rdf:type owl:NamedIndividual ,
                                   <https://w3id.org/h2v#DynamicProperty> ;
                          <http://qudt.org/schema/qudt/applicableUnit> <http://qudt.org/vocab/unit/UNITLESS> ;
                          rdfs:comment "The Actuated On-Off Valve State [boolean] of the actuated on-off valve of the HV is the actual state of the valve. If the value is 1, the valve is open, if the value is 0, the valve is closed."^^rdfs:Literal ;
                          rdfs:label "Actuated On-Off Valve State"^^rdfs:Literal ;
                          <http://www.w3.org/2004/02/skos/core#broader> <http://qudt.org/vocab/quantitykind/Dimensionless> ;
                          <https://w3id.org/h2v#appliesToSystem> <https://w3id.org/h2v#ActuatedOn-OffValve> .


###  https://w3id.org/h2v/property#AmountOfHydrogenStored
:AmountOfHydrogenStored rdf:type owl:NamedIndividual ,
                                 <https://w3id.org/h2v#DynamicProperty> ;
                        <http://qudt.org/schema/qudt/applicableUnit> <http://qudt.org/vocab/unit/KiloGM> ;
                        rdfs:comment "The Amount Of Hydrogen Stored [kg] is the quantity of hydrogen stored in the storage unit"^^rdfs:Literal ;
                        rdfs:label "Amount Of Hydrogen Stored"^^rdfs:Literal ;
                        <http://www.w3.org/2004/02/skos/core#broader> <http://qudt.org/vocab/quantitykind/Mass> ;
                        <https://w3id.org/h2v#appliesToSystem> <https://w3id.org/h2v#HydrogenStorage> .


###  https://w3id.org/h2v/property#AmountOfStoredDistilledWater
:AmountOfStoredDistilledWater rdf:type owl:NamedIndividual ,
                                       <https://w3id.org/h2v#DynamicProperty> ;
                              <http://qudt.org/schema/qudt/applicableUnit> <http://qudt.org/vocab/unit/KiloGM> ;
                              rdfs:comment "The Amount Of Stored Distilled Water [kg] of the electrolyzer is the measured distilled water contained in water storage of the electrolyzer"^^rdfs:Literal ;
                              rdfs:label "Amount Of Stored Distilled Water"^^rdfs:Literal ;
                              <http://www.w3.org/2004/02/skos/core#broader> <http://qudt.org/vocab/quantitykind/Mass> ;
                              <https://w3id.org/h2v#appliesToSystem> <https://w3id.org/h2v#Electrolyzer> .


###  https://w3id.org/h2v/property#BlenderActualH2O
:BlenderActualH2O rdf:type owl:NamedIndividual ,
                           <https://w3id.org/h2v#DynamicProperty> ;
                  <http://qudt.org/schema/qudt/applicableUnit> <http://qudt.org/vocab/unit/PPM> ;
                  rdfs:comment "The Blender Actual H2O [ppm] is the actual quantity of water vapor in the hydrogen mixture fed into the gas network"^^rdfs:Literal ;
                  rdfs:label "Blender Actual H2O "^^rdfs:Literal ;
                  <http://www.w3.org/2004/02/skos/core#broader> <http://qudt.org/vocab/quantitykind/DimensionlessRatio> ;
                  <https://w3id.org/h2v#appliesToSystem> <https://w3id.org/h2v#Blender> .


###  https://w3id.org/h2v/property#BlenderActualN2
:BlenderActualN2 rdf:type owl:NamedIndividual ,
                          <https://w3id.org/h2v#DynamicProperty> ;
                 <http://qudt.org/schema/qudt/applicableUnit> <http://qudt.org/vocab/unit/PPM> ;
                 rdfs:comment "The Blender Actual N2 [ppm] is the actual quantity of nitrogen in the hydrogen mixture fed into the gas network"^^rdfs:Literal ;
                 rdfs:label "Blender Actual N2"^^rdfs:Literal ;
                 <http://www.w3.org/2004/02/skos/core#broader> <http://qudt.org/vocab/quantitykind/DimensionlessRatio> ;
                 <https://w3id.org/h2v#appliesToSystem> <https://w3id.org/h2v#Blender> .


###  https://w3id.org/h2v/property#BlenderActualO2
:BlenderActualO2 rdf:type owl:NamedIndividual ,
                          <https://w3id.org/h2v#DynamicProperty> ;
                 <http://qudt.org/schema/qudt/applicableUnit> <http://qudt.org/vocab/unit/PPM> ;
                 rdfs:comment "The Blender Actual O2 [ppm] is the actual quantity of oxigen in the hydrogen mixture fed into the gas network"^^rdfs:Literal ;
                 rdfs:label "Blender Actual O2"^^rdfs:Literal ;
                 <http://www.w3.org/2004/02/skos/core#broader> <http://qudt.org/vocab/quantitykind/DimensionlessRatio> ;
                 <https://w3id.org/h2v#appliesToSystem> <https://w3id.org/h2v#Blender> .


###  https://w3id.org/h2v/property#BlenderChemicalComposition
:BlenderChemicalComposition rdf:type owl:NamedIndividual ,
                                     <https://w3id.org/h2v#DynamicProperty> ;
                            <http://qudt.org/schema/qudt/applicableUnit> <http://qudt.org/vocab/unit/PPM> ;
                            rdfs:comment "The Blender Chemical Composition [ppm] is the actual chemical composition of hydrogen fed into the gas network"^^rdfs:Literal ;
                            rdfs:label "Blender Chemical Composition"^^rdfs:Literal ;
                            <http://www.w3.org/2004/02/skos/core#broader> <http://qudt.org/vocab/quantitykind/DimensionlessRatio> ;
                            <https://w3id.org/h2v#appliesToSystem> <https://w3id.org/h2v#Blender> .


###  https://w3id.org/h2v/property#BlenderH2PressureSet
:BlenderH2PressureSet rdf:type owl:NamedIndividual ,
                               <https://w3id.org/h2v#PropertySet> ;
                      rdfs:label "Blender H2 Pressure Set"^^rdfs:Literal ;
                      <https://w3id.org/h2v#hasMaximumPropertyMember> :BlenderMaximumH2Pressure ;
                      <https://w3id.org/h2v#hasMinimumPropertyMember> :BlenderMinimumH2Pressure ;
                      <https://w3id.org/h2v#hasPropertyMember> :BlenderMaximumH2Pressure ,
                                                               :BlenderMinimumH2Pressure .


###  https://w3id.org/h2v/property#BlenderHydrogenMassFlow
:BlenderHydrogenMassFlow rdf:type owl:NamedIndividual ,
                                  <https://w3id.org/h2v#DynamicProperty> ;
                         <http://qudt.org/schema/qudt/applicableUnit> <http://qudt.org/vocab/unit/KiloGM-PER-HR> ;
                         rdfs:comment "The Hydrogen Mass Flow [kg/h] is the current hydrogen flow fed into the gas network"^^rdfs:Literal ;
                         rdfs:label "Blender Hydrogen Mass Flow"^^rdfs:Literal ;
                         <http://www.w3.org/2004/02/skos/core#broader> <http://qudt.org/vocab/quantitykind/MassFlowRate> ;
                         <https://w3id.org/h2v#appliesToSystem> <https://w3id.org/h2v#Blender> .


###  https://w3id.org/h2v/property#BlenderMaximumH2Flow
:BlenderMaximumH2Flow rdf:type owl:NamedIndividual ,
                               <https://w3id.org/h2v#StaticProperty> ;
                      <http://qudt.org/schema/qudt/applicableUnit> <http://qudt.org/vocab/unit/KiloGM-PER-HR> ;
                      rdfs:comment "The Blender Maximum H2 Flow [Kg/h] of the blender of the HV is the maximum value of H2 allowed in input of the blender"^^rdfs:Literal ;
                      rdfs:label "Blender Maximum H2 Flow"^^rdfs:Literal ;
                      <http://www.w3.org/2004/02/skos/core#broader> <http://qudt.org/vocab/quantitykind/MassFlowRate> ;
                      <https://w3id.org/h2v#appliesToSystem> <https://w3id.org/h2v#Blender> .


###  https://w3id.org/h2v/property#BlenderMaximumH2Pressure
:BlenderMaximumH2Pressure rdf:type owl:NamedIndividual ,
                                   <https://w3id.org/h2v#StaticProperty> ;
                          <http://qudt.org/schema/qudt/applicableUnit> <http://qudt.org/vocab/unit/BAR> ;
                          rdfs:comment "The Blender Maximum H2 Pressure [bar] is the maximum pressure of the H2 within which hydrogen can be delivered to the gas network"^^rdfs:Literal ;
                          rdfs:label "Blender Maximum H2 Pressure"^^rdfs:Literal ;
                          <http://www.w3.org/2004/02/skos/core#broader> <http://qudt.org/vocab/quantitykind/Pressure> ;
                          <https://w3id.org/h2v#appliesToSystem> <https://w3id.org/h2v#Blender> .


###  https://w3id.org/h2v/property#BlenderMinimumH2Pressure
:BlenderMinimumH2Pressure rdf:type owl:NamedIndividual ,
                                   <https://w3id.org/h2v#StaticProperty> ;
                          <http://qudt.org/schema/qudt/applicableUnit> <http://qudt.org/vocab/unit/BAR> ;
                          rdfs:comment "The Blender Minimum H2 Pressure [bar] is the minimum pressure of the H2 within which hydrogen can be delivered to the gas network"^^rdfs:Literal ;
                          rdfs:label "Blender Minimum H2 Pressure"^^rdfs:Literal ;
                          <http://www.w3.org/2004/02/skos/core#broader> <http://qudt.org/vocab/quantitykind/Pressure> ;
                          <https://w3id.org/h2v#appliesToSystem> <https://w3id.org/h2v#Blender> .


###  https://w3id.org/h2v/property#BlenderNominalChemicalCompositionTolerated
:BlenderNominalChemicalCompositionTolerated rdf:type owl:NamedIndividual ,
                                                     <https://w3id.org/h2v#StaticProperty> ;
                                            <http://qudt.org/schema/qudt/applicableUnit> <http://qudt.org/vocab/unit/PPM> ;
                                            rdfs:comment "The Blender Nominal Chemical Composition Tolerated [ppm] is the allowable hydrogen chemical composition in parts per million of hydrogen fouling (O2, H2O, N2)"^^rdfs:Literal ;
                                            rdfs:label "Blender Nominal Chemical Composition Tolerated"^^rdfs:Literal ;
                                            <http://www.w3.org/2004/02/skos/core#broader> <http://qudt.org/vocab/quantitykind/DimensionlessRatio> ;
                                            <https://w3id.org/h2v#appliesToSystem> <https://w3id.org/h2v#Blender> .


###  https://w3id.org/h2v/property#BlenderNominalH2OTolerated
:BlenderNominalH2OTolerated rdf:type owl:NamedIndividual ,
                                     <https://w3id.org/h2v#StaticProperty> ;
                            <http://qudt.org/schema/qudt/applicableUnit> <http://qudt.org/vocab/unit/PPM> ;
                            rdfs:comment "The Blender Nominal H2O Tolerated [ppm] is the maximum amount of water vapor tolerated in the hydrogen mixture to be fed into the gas network"^^rdfs:Literal ;
                            rdfs:label "Blender Nominal H2O Tolerated"^^rdfs:Literal ;
                            <http://www.w3.org/2004/02/skos/core#broader> <http://qudt.org/vocab/quantitykind/DimensionlessRatio> ;
                            <https://w3id.org/h2v#appliesToSystem> <https://w3id.org/h2v#Blender> .


###  https://w3id.org/h2v/property#BlenderNominalN2Tolerated
:BlenderNominalN2Tolerated rdf:type owl:NamedIndividual ,
                                    <https://w3id.org/h2v#StaticProperty> ;
                           <http://qudt.org/schema/qudt/applicableUnit> <http://qudt.org/vocab/unit/PPM> ;
                           rdfs:comment "The Blender Nominal N2 Tolerated [ppm] is the maximum amount of nitrogen tolerated in the hydrogen mixture to be fed into the gas network"^^rdfs:Literal ;
                           rdfs:label "Blender Nominal N2 Tolerated"^^rdfs:Literal ;
                           <http://www.w3.org/2004/02/skos/core#broader> <http://qudt.org/vocab/quantitykind/DimensionlessRatio> ;
                           <https://w3id.org/h2v#appliesToSystem> <https://w3id.org/h2v#Blender> .


###  https://w3id.org/h2v/property#BlenderNominalO2Tolerated
:BlenderNominalO2Tolerated rdf:type owl:NamedIndividual ,
                                    <https://w3id.org/h2v#StaticProperty> ;
                           <http://qudt.org/schema/qudt/applicableUnit> <http://qudt.org/vocab/unit/PPM> ;
                           rdfs:comment """
The Blender Nominal O2 Tolerated [ppm] is the maximum amount of oxigen tolerated in the hydrogen mixture to be fed into the gas network"""^^rdfs:Literal ;
                           rdfs:label "Blender Nominal O2 Tolerated"^^rdfs:Literal ;
                           <http://www.w3.org/2004/02/skos/core#broader> <http://qudt.org/vocab/quantitykind/DimensionlessRatio> ;
                           <https://w3id.org/h2v#appliesToSystem> <https://w3id.org/h2v#Blender> .


###  https://w3id.org/h2v/property#BlenderOutletNominalPressure
:BlenderOutletNominalPressure rdf:type owl:NamedIndividual ,
                                       <https://w3id.org/h2v#StaticProperty> ;
                              <http://qudt.org/schema/qudt/applicableUnit> <http://qudt.org/vocab/unit/BAR> ;
                              rdfs:comment "The Blender Outlet Nominal Pressure [bar] of the blender of the HV is the expected outlet pressure of the blender"^^rdfs:Literal ;
                              rdfs:label "Blender Outlet Nominal Pressure"^^rdfs:Literal ;
                              <http://www.w3.org/2004/02/skos/core#broader> <http://qudt.org/vocab/quantitykind/Pressure> ;
                              <https://w3id.org/h2v#appliesToSystem> <https://w3id.org/h2v#Blender> .


###  https://w3id.org/h2v/property#BlenderOutletNominalTemperature
:BlenderOutletNominalTemperature rdf:type owl:NamedIndividual ,
                                          <https://w3id.org/h2v#StaticProperty> ;
                                 <http://qudt.org/schema/qudt/applicableUnit> <http://qudt.org/vocab/unit/DEG_C> ;
                                 rdfs:comment "The Blender Outlet Nominal Temperature [°C] of the blender of the HV is expected outlet temperature of the blender"^^rdfs:Literal ;
                                 rdfs:label "Blender Outlet Nominal Temperature"^^rdfs:Literal ;
                                 <http://www.w3.org/2004/02/skos/core#broader> <http://qudt.org/vocab/quantitykind/Temperature> ;
                                 <https://w3id.org/h2v#appliesToSystem> <https://w3id.org/h2v#Blender> .


###  https://w3id.org/h2v/property#BlenderOutletPressure
:BlenderOutletPressure rdf:type owl:NamedIndividual ,
                                <https://w3id.org/h2v#DynamicProperty> ;
                       <http://qudt.org/schema/qudt/applicableUnit> <http://qudt.org/vocab/unit/BAR> ;
                       rdfs:comment "The Blender Outlet Pressure [bar] of the blender of the HV is the actual measured outlet pressure"^^rdfs:Literal ;
                       rdfs:label "Blender Outlet Pressure"^^rdfs:Literal ;
                       <http://www.w3.org/2004/02/skos/core#broader> <http://qudt.org/vocab/quantitykind/Pressure> ;
                       <https://w3id.org/h2v#appliesToSystem> <https://w3id.org/h2v#Blender> .


###  https://w3id.org/h2v/property#BlenderOutletTemperature
:BlenderOutletTemperature rdf:type owl:NamedIndividual ,
                                   <https://w3id.org/h2v#DynamicProperty> ;
                          <http://qudt.org/schema/qudt/applicableUnit> <http://qudt.org/vocab/unit/DEG_C> ;
                          rdfs:comment "The Blender Outlet Temperature [°C] of the blender of the HV is the actual measured outlet temperature"^^rdfs:Literal ;
                          rdfs:label "Blender Outlet Temperature"^^rdfs:Literal ;
                          <http://www.w3.org/2004/02/skos/core#broader> <http://qudt.org/vocab/quantitykind/Temperature> ;
                          <https://w3id.org/h2v#appliesToSystem> <https://w3id.org/h2v#Blender> .


###  https://w3id.org/h2v/property#BlenderPressureH2
:BlenderPressureH2 rdf:type owl:NamedIndividual ,
                            <https://w3id.org/h2v#DynamicProperty> ;
                   <http://qudt.org/schema/qudt/applicableUnit> <http://qudt.org/vocab/unit/BAR> ;
                   rdfs:comment "The Blender Pressure H2 [bar] is the current hydrogen pressure fed into the gas network"^^rdfs:Literal ;
                   rdfs:label "Blender Pressure H2"^^rdfs:Literal ;
                   <http://www.w3.org/2004/02/skos/core#broader> <http://qudt.org/vocab/quantitykind/Pressure> ;
                   <https://w3id.org/h2v#appliesToSystem> <https://w3id.org/h2v#Blender> .


###  https://w3id.org/h2v/property#CH4InletGasFlow
:CH4InletGasFlow rdf:type owl:NamedIndividual ,
                          <https://w3id.org/h2v#DynamicProperty> ;
                 <http://qudt.org/schema/qudt/applicableUnit> <http://qudt.org/vocab/unit/SCM-PER-HR> ;
                 rdfs:comment "The CH4 Inlet Gas Flow [Nm3/h] of the blender of the HV is the value of CH4 in input of the blender"^^rdfs:Literal ;
                 rdfs:label "CH4 Inlet Gas Flow"^^rdfs:Literal ;
                 <http://www.w3.org/2004/02/skos/core#broader> <http://qudt.org/vocab/quantitykind/MolarFlowRate> ;
                 <https://w3id.org/h2v#appliesToSystem> <https://w3id.org/h2v#Blender> .


###  https://w3id.org/h2v/property#CH4InletGasFlowSet
:CH4InletGasFlowSet rdf:type owl:NamedIndividual ,
                             <https://w3id.org/h2v#PropertySet> ;
                    rdfs:label "CH4 Inlet Gas Flow Set"^^rdfs:Literal ;
                    <https://w3id.org/h2v#hasMaximumPropertyMember> :MaximumCH4InletGasFlow ;
                    <https://w3id.org/h2v#hasMinimumPropertyMember> :MinimumCH4InletGasFlow ;
                    <https://w3id.org/h2v#hasPropertyMember> :MaximumCH4InletGasFlow ,
                                                             :MinimumCH4InletGasFlow .


###  https://w3id.org/h2v/property#DistilledWaterTemperature
:DistilledWaterTemperature rdf:type owl:NamedIndividual ,
                                    <https://w3id.org/h2v#DynamicProperty> ;
                           <http://qudt.org/schema/qudt/applicableUnit> <http://qudt.org/vocab/unit/DEG_C> ;
                           rdfs:comment "The Distilled Water Temperature [°C] of the electrolyzer of the HV is the measured water temperature to be compared with the allowed range"^^rdfs:Literal ;
                           rdfs:label "Distilled Water Temperature"^^rdfs:Literal ;
                           <http://www.w3.org/2004/02/skos/core#broader> <http://qudt.org/vocab/quantitykind/Temperature> ;
                           <https://w3id.org/h2v#appliesToSystem> <https://w3id.org/h2v#Electrolyzer> .


###  https://w3id.org/h2v/property#DistilledWaterTemperatureSet
:DistilledWaterTemperatureSet rdf:type owl:NamedIndividual ,
                                       <https://w3id.org/h2v#PropertySet> ;
                              rdfs:label "Distilled Water Temperature Set"^^rdfs:Literal ;
                              <https://w3id.org/h2v#hasMaximumPropertyMember> :MaximumDistilledWaterTemperature ;
                              <https://w3id.org/h2v#hasMinimumPropertyMember> :MinimumDistilledWaterTemperature ;
                              <https://w3id.org/h2v#hasPropertyMember> :MaximumDistilledWaterTemperature ,
                                                                       :MinimumDistilledWaterTemperature .


###  https://w3id.org/h2v/property#ElectricPower
:ElectricPower rdf:type owl:NamedIndividual ,
                        <https://w3id.org/h2v#DynamicProperty> ;
               <http://qudt.org/schema/qudt/applicableUnit> <http://qudt.org/vocab/unit/KiloW> ;
               rdfs:comment "The Electric Power [kW] of the electrolyzer of the HV is the available electric power absorbed by the electrolyzer"^^rdfs:Literal ;
               rdfs:label "Electric Power"^^rdfs:Literal ;
               <http://www.w3.org/2004/02/skos/core#broader> <http://qudt.org/vocab/quantitykind/ElectricPower> ;
               <https://w3id.org/h2v#appliesToSystem> <https://w3id.org/h2v#Electrolyzer> .


###  https://w3id.org/h2v/property#ElectricPowerSet
:ElectricPowerSet rdf:type owl:NamedIndividual ,
                           <https://w3id.org/h2v#PropertySet> ;
                  rdfs:label "Electric Power Set"^^rdfs:Literal ;
                  <https://w3id.org/h2v#hasMaximumPropertyMember> :MaximumElectricPower ;
                  <https://w3id.org/h2v#hasMinimumPropertyMember> :MinimumElectricPower ;
                  <https://w3id.org/h2v#hasPropertyMember> :MaximumElectricPower ,
                                                           :MinimumElectricPower .


###  https://w3id.org/h2v/property#ElectrolyzerH2FlowSet
:ElectrolyzerH2FlowSet rdf:type owl:NamedIndividual ,
                                <https://w3id.org/h2v#PropertySet> ;
                       rdfs:label "Electrolyzer H2 Flow Set"^^rdfs:Literal ;
                       <https://w3id.org/h2v#hasMaximumPropertyMember> :ElectrolyzerMaximumH2Flow ;
                       <https://w3id.org/h2v#hasMinimumPropertyMember> :ElectrolyzerMinimumH2Flow ;
                       <https://w3id.org/h2v#hasOptimalPropertyMember> :ElectrolyzerOptimalH2Flow ;
                       <https://w3id.org/h2v#hasPropertyMember> :ElectrolyzerMaximumH2Flow ,
                                                                :ElectrolyzerMinimumH2Flow ,
                                                                :ElectrolyzerOptimalH2Flow .


###  https://w3id.org/h2v/property#ElectrolyzerHydrogenMassFlow
:ElectrolyzerHydrogenMassFlow rdf:type owl:NamedIndividual ,
                                       <https://w3id.org/h2v#DynamicProperty> ;
                              <http://qudt.org/schema/qudt/applicableUnit> <http://qudt.org/vocab/unit/KiloGM-PER-HR> ;
                              rdfs:comment "The Hydrogen Mass Flow [kg/h] of the electrolyzer of the HV is the  hydrogen flow at the output of the electrolyzer"^^rdfs:Literal ;
                              rdfs:label "Electrolyzer Hydrogen Mass Flow"^^rdfs:Literal ;
                              <http://www.w3.org/2004/02/skos/core#broader> <http://qudt.org/vocab/quantitykind/MassFlowRate> ;
                              <https://w3id.org/h2v#appliesToSystem> <https://w3id.org/h2v#Electrolyzer> .


###  https://w3id.org/h2v/property#ElectrolyzerMaximumH2Flow
:ElectrolyzerMaximumH2Flow rdf:type owl:NamedIndividual ,
                                    <https://w3id.org/h2v#StaticProperty> ;
                           <http://qudt.org/schema/qudt/applicableUnit> <http://qudt.org/vocab/unit/SCM-PER-HR> ;
                           rdfs:comment "The Electrolyzer Maximum H2 Flow [Nm3/h] of the electrolyzer of the HV is the maximum hydrogen outlet flow the electrolyzer can produce "^^rdfs:Literal ;
                           rdfs:label "Electrolyzer Maximum H2 Flow"^^rdfs:Literal ;
                           <http://www.w3.org/2004/02/skos/core#broader> <http://qudt.org/vocab/quantitykind/MolarFlowRate> ;
                           <https://w3id.org/h2v#appliesToSystem> <https://w3id.org/h2v#Electrolyzer> .


###  https://w3id.org/h2v/property#ElectrolyzerMinimumH2Flow
:ElectrolyzerMinimumH2Flow rdf:type owl:NamedIndividual ,
                                    <https://w3id.org/h2v#StaticProperty> ;
                           <http://qudt.org/schema/qudt/applicableUnit> <http://qudt.org/vocab/unit/SCM-PER-HR> ;
                           rdfs:comment "The Electrolyzer Minimum H2 Flow [Nm3/h] of the electrolyzer of the HV is the minimum hydrogen outlet flow the electrolyzer can produce"^^rdfs:Literal ;
                           rdfs:label "Electrolyzer Minimum H2 Flow"^^rdfs:Literal ;
                           <http://www.w3.org/2004/02/skos/core#broader> <http://qudt.org/vocab/quantitykind/MolarFlowRate> ;
                           <https://w3id.org/h2v#appliesToSystem> <https://w3id.org/h2v#Electrolyzer> .


###  https://w3id.org/h2v/property#ElectrolyzerOptimalH2Flow
:ElectrolyzerOptimalH2Flow rdf:type owl:NamedIndividual ,
                                    <https://w3id.org/h2v#StaticProperty> ;
                           <http://qudt.org/schema/qudt/applicableUnit> <http://qudt.org/vocab/unit/SCM-PER-HR> ;
                           rdfs:comment "The Electrolyzer Optimal H2 Flow [Nm3/h] of the electrolyzer of the HV  is the hydrogen outlet flow the electrolyzer can produce with the highest efficiency"^^rdfs:Literal ;
                           rdfs:label "Electrolyzer Optimal H2 Flow"^^rdfs:Literal ;
                           <http://www.w3.org/2004/02/skos/core#broader> <http://qudt.org/vocab/quantitykind/MolarFlowRate> ;
                           <https://w3id.org/h2v#appliesToSystem> <https://w3id.org/h2v#Electrolyzer> .


###  https://w3id.org/h2v/property#ElectrolyzerWaterFlow
:ElectrolyzerWaterFlow rdf:type owl:NamedIndividual ,
                                <https://w3id.org/h2v#DynamicProperty> ;
                       <http://qudt.org/schema/qudt/applicableUnit> <http://qudt.org/vocab/unit/KiloGM-PER-HR> ;
                       rdfs:comment "The Electrolyzer Water Flow [kg/h] of the electrolyzer of the HV is the actual distilled water consumption"^^rdfs:Literal ;
                       rdfs:label "Electrolyzer Water Flow"^^rdfs:Literal ;
                       <http://www.w3.org/2004/02/skos/core#broader> <http://qudt.org/vocab/quantitykind/MassFlowRate> ;
                       <https://w3id.org/h2v#appliesToSystem> <https://w3id.org/h2v#Electrolyzer> .


###  https://w3id.org/h2v/property#EnvironmentalTemperature
:EnvironmentalTemperature rdf:type owl:NamedIndividual ,
                                   <https://w3id.org/h2v#WeatherProperty> ;
                          <http://qudt.org/schema/qudt/applicableUnit> <http://qudt.org/vocab/unit/DEG_C> ;
                          rdfs:comment "The Environmental Temperature [°C] is the actual ambient air temperatures, in degrees Celsius. It can be either actual (i.e., based on an observation) or forecasted (i.e., based on weather forecast)."^^rdfs:Literal ;
                          rdfs:label "Environmental Temperature"^^rdfs:Literal ;
                          <http://www.w3.org/2004/02/skos/core#broader> <http://qudt.org/vocab/quantitykind/Temperature> .


###  https://w3id.org/h2v/property#EnvironmentalWindSpeed
:EnvironmentalWindSpeed rdf:type owl:NamedIndividual ,
                                 <https://w3id.org/h2v#WeatherProperty> ;
                        <http://qudt.org/schema/qudt/applicableUnit> <http://qudt.org/vocab/unit/M-PER-SEC> ;
                        rdfs:comment "The Environmental Wind speed  [m/s] is the actual wind speed, in meter per second. It can be either actual (i.e., based on an observation) or forecasted (i.e., based on weather forecast)."^^rdfs:Literal ;
                        rdfs:label "Environmental Wind Speed"^^rdfs:Literal ;
                        <http://www.w3.org/2004/02/skos/core#broader> <http://qudt.org/vocab/quantitykind/Speed> .


###  https://w3id.org/h2v/property#ExportedHydrogenFlowPressure
:ExportedHydrogenFlowPressure rdf:type owl:NamedIndividual ,
                                       <https://w3id.org/h2v#DynamicProperty> ;
                              <http://qudt.org/schema/qudt/applicableUnit> <https://w3id.org/h2v#BARG> ;
                              rdfs:comment "The Exported Hydrogen Flow Pressure [barg] is the hydrogen flow pressure level during the export operations"^^rdfs:Literal ;
                              rdfs:label "Exported Hydrogen Flow Pressure"^^rdfs:Literal ;
                              <http://www.w3.org/2004/02/skos/core#broader> <http://qudt.org/vocab/quantitykind/GaugePressure> ;
                              <https://w3id.org/h2v#appliesToSystem> <https://w3id.org/h2v#HydrogenStorage> .


###  https://w3id.org/h2v/property#ExportedHydrogenPressureSet
:ExportedHydrogenPressureSet rdf:type owl:NamedIndividual ,
                                      <https://w3id.org/h2v#PropertySet> ;
                             rdfs:label "Exported Hydrogen Pressure Set"^^rdfs:Literal ;
                             <https://w3id.org/h2v#hasMaximumPropertyMember> :MaximumExportedHydrogenPressure ;
                             <https://w3id.org/h2v#hasMinimumPropertyMember> :MinimumExportedHydrogenPressure ;
                             <https://w3id.org/h2v#hasPropertyMember> :MaximumExportedHydrogenPressure ,
                                                                      :MinimumExportedHydrogenPressure .


###  https://w3id.org/h2v/property#FuelCellGasFlow
:FuelCellGasFlow rdf:type owl:NamedIndividual ,
                          <https://w3id.org/h2v#DynamicProperty> ;
                 <http://qudt.org/schema/qudt/applicableUnit> <http://qudt.org/vocab/unit/SCM-PER-HR> ;
                 rdfs:comment "The Fuel Cell Gas Flow [Nm3/h] of the fuel cell of the HV is the inlet amount of hydrogen"^^rdfs:Literal ;
                 rdfs:label "Fuel Cell Gas Flow"^^rdfs:Literal ;
                 <http://www.w3.org/2004/02/skos/core#broader> <http://qudt.org/vocab/quantitykind/MolarFlowRate> ;
                 <https://w3id.org/h2v#appliesToSystem> <https://w3id.org/h2v#FuelCell> .


###  https://w3id.org/h2v/property#FuelCellMaximumGasFlow
:FuelCellMaximumGasFlow rdf:type owl:NamedIndividual ,
                                 <https://w3id.org/h2v#StaticProperty> ;
                        <http://qudt.org/schema/qudt/applicableUnit> <http://qudt.org/vocab/unit/SCM-PER-HR> ;
                        rdfs:comment "The Fuel Cell Maximum Gas Flow [Nm3/h] of the fuel cell of the HV is the maximum inlet amount of hydrogen"^^rdfs:Literal ;
                        rdfs:label "Fuel Cell Maximum Gas Flow"^^rdfs:Literal ;
                        <http://www.w3.org/2004/02/skos/core#broader> <http://qudt.org/vocab/quantitykind/MolarFlowRate> ;
                        <https://w3id.org/h2v#appliesToSystem> <https://w3id.org/h2v#FuelCell> .


###  https://w3id.org/h2v/property#FuelCellOptimalPressure
:FuelCellOptimalPressure rdf:type owl:NamedIndividual ,
                                  <https://w3id.org/h2v#StaticProperty> ;
                         <http://qudt.org/schema/qudt/applicableUnit> <https://w3id.org/h2v#BARG> ;
                         rdfs:comment "The Fuel Cell Optimal Pressure [barg] of the fuel cell of the HV is the working pressure with the highest efficiency."^^rdfs:Literal ;
                         rdfs:label "Fuel Cell Optimal Pressure"^^rdfs:Literal ;
                         <http://www.w3.org/2004/02/skos/core#broader> <http://qudt.org/vocab/quantitykind/GaugePressure> ;
                         <https://w3id.org/h2v#appliesToSystem> <https://w3id.org/h2v#FuelCell> .


###  https://w3id.org/h2v/property#FuelCellOptimalTemperature
:FuelCellOptimalTemperature rdf:type owl:NamedIndividual ,
                                     <https://w3id.org/h2v#StaticProperty> ;
                            <http://qudt.org/schema/qudt/applicableUnit> <http://qudt.org/vocab/unit/DEG_C> ;
                            rdfs:comment "The Fuel Cell Optimal Temperature [°C] of the fuel cell of the HV is the working temperature with the highest efficiency."^^rdfs:Literal ;
                            rdfs:label "Fuel Cell Optimal Temperature "^^rdfs:Literal ;
                            <http://www.w3.org/2004/02/skos/core#broader> <http://qudt.org/vocab/quantitykind/Temperature> ;
                            <https://w3id.org/h2v#appliesToSystem> <https://w3id.org/h2v#FuelCell> .


###  https://w3id.org/h2v/property#FuelCellPressure
:FuelCellPressure rdf:type owl:NamedIndividual ,
                           <https://w3id.org/h2v#DynamicProperty> ;
                  <http://qudt.org/schema/qudt/applicableUnit> <https://w3id.org/h2v#BARG> ;
                  rdfs:comment "The Fuel Cell Pressure [barg] is the working pressure of the fuel cell "^^rdfs:Literal ;
                  rdfs:label "Fuel Cell Pressure"^^rdfs:Literal ;
                  <http://www.w3.org/2004/02/skos/core#broader> <http://qudt.org/vocab/quantitykind/GaugePressure> ;
                  <https://w3id.org/h2v#appliesToSystem> <https://w3id.org/h2v#FuelCell> .


###  https://w3id.org/h2v/property#FuelCellTemperature
:FuelCellTemperature rdf:type owl:NamedIndividual ,
                              <https://w3id.org/h2v#DynamicProperty> ;
                     <http://qudt.org/schema/qudt/applicableUnit> <http://qudt.org/vocab/unit/DEG_C> ;
                     rdfs:comment "The Fuel Cell Temperature [°C] is the working temperature of the fuel cell"^^rdfs:Literal ;
                     rdfs:label "Fuel Cell Temperature "^^rdfs:Literal ;
                     <http://www.w3.org/2004/02/skos/core#broader> <http://qudt.org/vocab/quantitykind/Temperature> ;
                     <https://w3id.org/h2v#appliesToSystem> <https://w3id.org/h2v#FuelCell> .


###  https://w3id.org/h2v/property#GasCompositionSet
:GasCompositionSet rdf:type owl:NamedIndividual ,
                            <https://w3id.org/h2v#PropertySet> ;
                   rdfs:label "Gas Composition Set"^^rdfs:Literal ;
                   <https://w3id.org/h2v#hasMaximumPropertyMember> :MaximumGasComposition ;
                   <https://w3id.org/h2v#hasMinimumPropertyMember> :MinimumGasComposition ;
                   <https://w3id.org/h2v#hasPropertyMember> :MaximumGasComposition ,
                                                            :MinimumGasComposition .


###  https://w3id.org/h2v/property#GasFlow
:GasFlow rdf:type owl:NamedIndividual ,
                  <https://w3id.org/h2v#DynamicProperty> ;
         <http://qudt.org/schema/qudt/applicableUnit> <http://qudt.org/vocab/unit/SCM-PER-HR> ;
         rdfs:comment "The Gas Flow [Nm3/h] of the electrolyzer of the HV is the  hydrogen flow at the output of the electrolyzer"^^rdfs:Literal ;
         rdfs:label "Gas Flow"^^rdfs:Literal ;
         <http://www.w3.org/2004/02/skos/core#broader> <http://qudt.org/vocab/quantitykind/MolarFlowRate> ;
         <https://w3id.org/h2v#appliesToSystem> <https://w3id.org/h2v#Electrolyzer> .


###  https://w3id.org/h2v/property#GlobalHorizontalIrradiance
:GlobalHorizontalIrradiance rdf:type owl:NamedIndividual ,
                                     <https://w3id.org/h2v#WeatherProperty> ;
                            <http://qudt.org/schema/qudt/applicableUnit> <http://qudt.org/vocab/unit/W-PER-M2> ;
                            rdfs:comment "The Global Horizontal Irradiance [W/m2] is the usable solar energy expected to hit a specific surface (per square meter) over a certain time period, after accounting for various real-world loss factors. It can be either actual (i.e., based on an observation) or forecasted (i.e., based on weather forecast)."^^rdfs:Literal ;
                            rdfs:label "Global Horizontal Irradiance"^^rdfs:Literal ;
                            <http://www.w3.org/2004/02/skos/core#broader> <http://qudt.org/vocab/quantitykind/PowerPerArea> .


###  https://w3id.org/h2v/property#GlobeValveInletFlow
:GlobeValveInletFlow rdf:type owl:NamedIndividual ,
                              <https://w3id.org/h2v#DynamicProperty> ;
                     <http://qudt.org/schema/qudt/applicableUnit> <http://qudt.org/vocab/unit/SCM-PER-HR> ;
                     rdfs:comment "The Globe Valve Inlet Flow [Nm3/h] is the measured inlet flow of the globe valve"^^rdfs:Literal ;
                     rdfs:label "Globe Valve Inlet Flow"^^rdfs:Literal ;
                     <http://www.w3.org/2004/02/skos/core#broader> <http://qudt.org/vocab/quantitykind/MolarFlowRate> ;
                     <https://w3id.org/h2v#appliesToSystem> <https://w3id.org/h2v#GlobeValve> .


###  https://w3id.org/h2v/property#GlobeValveInletNominalFlow
:GlobeValveInletNominalFlow rdf:type owl:NamedIndividual ,
                                     <https://w3id.org/h2v#StaticProperty> ;
                            <http://qudt.org/schema/qudt/applicableUnit> <http://qudt.org/vocab/unit/SCM-PER-HR> ;
                            rdfs:comment "The Globe Valve Inlet Nominal Flow [Nm3/h] is the inlet flow the valve has been designed for"^^rdfs:Literal ;
                            rdfs:label "Globe Valve Inlet Nominal Flow"^^rdfs:Literal ;
                            <http://www.w3.org/2004/02/skos/core#broader> <http://qudt.org/vocab/quantitykind/MolarFlowRate> ;
                            <https://w3id.org/h2v#appliesToSystem> <https://w3id.org/h2v#GlobeValve> .


###  https://w3id.org/h2v/property#GlobeValveMaximumOpeningPercentage
:GlobeValveMaximumOpeningPercentage rdf:type owl:NamedIndividual ,
                                             <https://w3id.org/h2v#StaticProperty> ;
                                    <http://qudt.org/schema/qudt/applicableUnit> <http://qudt.org/vocab/unit/PERCENT> ;
                                    rdfs:comment "The Globe Valve Maximum Opening Percentage [%]  is the maximum opening allowed by the valve"^^rdfs:Literal ;
                                    rdfs:label "Globe Valve Maximum Opening Percentage"^^rdfs:Literal ;
                                    <http://www.w3.org/2004/02/skos/core#broader> <http://qudt.org/vocab/quantitykind/DimensionlessRatio> ;
                                    <https://w3id.org/h2v#appliesToSystem> <https://w3id.org/h2v#GlobeValve> .


###  https://w3id.org/h2v/property#GlobeValveMinimumOpeningPercentage
:GlobeValveMinimumOpeningPercentage rdf:type owl:NamedIndividual ,
                                             <https://w3id.org/h2v#StaticProperty> ;
                                    <http://qudt.org/schema/qudt/applicableUnit> <http://qudt.org/vocab/unit/PERCENT> ;
                                    rdfs:comment "The Globe Valve Minimum Opening Percentage [%]  is the minimum opening allowed by the valve"^^rdfs:Literal ;
                                    rdfs:label "Globe Valve Minimum Opening Percentage"^^rdfs:Literal ;
                                    <http://www.w3.org/2004/02/skos/core#broader> <http://qudt.org/vocab/quantitykind/DimensionlessRatio> ;
                                    <https://w3id.org/h2v#appliesToSystem> <https://w3id.org/h2v#GlobeValve> .


###  https://w3id.org/h2v/property#GlobeValveOpeningPercentage
:GlobeValveOpeningPercentage rdf:type owl:NamedIndividual ,
                                      <https://w3id.org/h2v#DynamicProperty> ;
                             <http://qudt.org/schema/qudt/applicableUnit> <http://qudt.org/vocab/unit/PERCENT> ;
                             rdfs:comment "The Globe Valve Opening Percentage [%] is the actual percentage of opening of the valve, reducing the flow."^^rdfs:Literal ;
                             rdfs:label "Globe Valve Opening Percentage"^^rdfs:Literal ;
                             <http://www.w3.org/2004/02/skos/core#broader> <http://qudt.org/vocab/quantitykind/DimensionlessRatio> ;
                             <https://w3id.org/h2v#appliesToSystem> <https://w3id.org/h2v#GlobeValve> .


###  https://w3id.org/h2v/property#GlobeValveOpeningPercentageSet
:GlobeValveOpeningPercentageSet rdf:type owl:NamedIndividual ,
                                         <https://w3id.org/h2v#PropertySet> ;
                                rdfs:label "Globe Valve Opening Percentage Set"^^rdfs:Literal ;
                                <https://w3id.org/h2v#hasMaximumPropertyMember> :GlobeValveMaximumOpeningPercentage ;
                                <https://w3id.org/h2v#hasMinimumPropertyMember> :GlobeValveMinimumOpeningPercentage ;
                                <https://w3id.org/h2v#hasPropertyMember> :GlobeValveMaximumOpeningPercentage ,
                                                                         :GlobeValveMinimumOpeningPercentage .


###  https://w3id.org/h2v/property#GlobeValveOutletFlow
:GlobeValveOutletFlow rdf:type owl:NamedIndividual ,
                               <https://w3id.org/h2v#DynamicProperty> ;
                      <http://qudt.org/schema/qudt/applicableUnit> <http://qudt.org/vocab/unit/SCM-PER-HR> ;
                      rdfs:comment "The Globe Valve Outlet Flow [Nm3/h]  is the measured inlet flow of the globe valve"^^rdfs:Literal ;
                      rdfs:label "Globe Valve Outlet Flow"^^rdfs:Literal ;
                      <http://www.w3.org/2004/02/skos/core#broader> <http://qudt.org/vocab/quantitykind/MolarFlowRate> ;
                      <https://w3id.org/h2v#appliesToSystem> <https://w3id.org/h2v#GlobeValve> .


###  https://w3id.org/h2v/property#GlobeValveOutletNominalFlow
:GlobeValveOutletNominalFlow rdf:type owl:NamedIndividual ,
                                      <https://w3id.org/h2v#StaticProperty> ;
                             <http://qudt.org/schema/qudt/applicableUnit> <http://qudt.org/vocab/unit/SCM-PER-HR> ;
                             rdfs:comment "The Globe Valve Outlet Nominal Flow [Nm3/h] is the outlet flow the valve has been designed for"^^rdfs:Literal ;
                             rdfs:label "Globe Valve Outlet Nominal Flow"^^rdfs:Literal ;
                             <http://www.w3.org/2004/02/skos/core#broader> <http://qudt.org/vocab/quantitykind/MolarFlowRate> ;
                             <https://w3id.org/h2v#appliesToSystem> <https://w3id.org/h2v#GlobeValve> .


###  https://w3id.org/h2v/property#H2InletGasFlow
:H2InletGasFlow rdf:type owl:NamedIndividual ,
                         <https://w3id.org/h2v#DynamicProperty> ;
                <http://qudt.org/schema/qudt/applicableUnit> <http://qudt.org/vocab/unit/SCM-PER-HR> ;
                rdfs:comment "The H2 Inlet Gas Flow [Nm3/h] of the blender of the HV is the value of H2 in input of the blender"^^rdfs:Literal ;
                rdfs:label "H2 Inlet Gas Flow"^^rdfs:Literal ;
                <http://www.w3.org/2004/02/skos/core#broader> <http://qudt.org/vocab/quantitykind/MolarFlowRate> ;
                <https://w3id.org/h2v#appliesToSystem> <https://w3id.org/h2v#Blender> .


###  https://w3id.org/h2v/property#H2InletGasFlowSet
:H2InletGasFlowSet rdf:type owl:NamedIndividual ,
                            <https://w3id.org/h2v#PropertySet> ;
                   rdfs:label "H2 Inlet Gas Flow Set"^^rdfs:Literal ;
                   <https://w3id.org/h2v#hasMaximumPropertyMember> :MaximumH2InletGasFlow ;
                   <https://w3id.org/h2v#hasMinimumPropertyMember> :MinimumH2InletGasFlow ;
                   <https://w3id.org/h2v#hasPropertyMember> :MaximumH2InletGasFlow ,
                                                            :MinimumH2InletGasFlow .


###  https://w3id.org/h2v/property#H2OSet
:H2OSet rdf:type owl:NamedIndividual ,
                 <https://w3id.org/h2v#PropertySet> ;
        rdfs:label "H2O Set"^^rdfs:Literal ;
        <https://w3id.org/h2v#hasMaximumPropertyMember> :MaximumH2O ;
        <https://w3id.org/h2v#hasMinimumPropertyMember> :MinimumH2O ;
        <https://w3id.org/h2v#hasPropertyMember> :MaximumH2O ,
                                                 :MinimumH2O .


###  https://w3id.org/h2v/property#H2PressureSet
:H2PressureSet rdf:type owl:NamedIndividual ,
                        <https://w3id.org/h2v#PropertySet> ;
               rdfs:label "H2 Pressure Set"^^rdfs:Literal ;
               <https://w3id.org/h2v#hasMaximumPropertyMember> :MaximumH2Pressure ;
               <https://w3id.org/h2v#hasMinimumPropertyMember> :MinimumH2Pressure ;
               <https://w3id.org/h2v#hasOptimalPropertyMember> :OptimalH2Pressure ;
               <https://w3id.org/h2v#hasPropertyMember> :MaximumH2Pressure ,
                                                        :MinimumH2Pressure ,
                                                        :OptimalH2Pressure .


###  https://w3id.org/h2v/property#H2ProductionSet
:H2ProductionSet rdf:type owl:NamedIndividual ,
                          <https://w3id.org/h2v#PropertySet> ;
                 rdfs:label "H2 Production Set"^^rdfs:Literal ;
                 <https://w3id.org/h2v#hasMaximumPropertyMember> :MaximumH2Production ;
                 <https://w3id.org/h2v#hasMinimumPropertyMember> :MinimumH2Production ;
                 <https://w3id.org/h2v#hasPropertyMember> :MaximumH2Production ,
                                                          :MinimumH2Production .


###  https://w3id.org/h2v/property#H2TemperatureSet
:H2TemperatureSet rdf:type owl:NamedIndividual ,
                           <https://w3id.org/h2v#PropertySet> ;
                  rdfs:label "H2 Temperature Set"^^rdfs:Literal ;
                  <https://w3id.org/h2v#hasMaximumPropertyMember> :MaximumH2Temperature ;
                  <https://w3id.org/h2v#hasMinimumPropertyMember> :MinimumH2Temperature ;
                  <https://w3id.org/h2v#hasPropertyMember> :MaximumH2Temperature ,
                                                           :MinimumH2Temperature .


###  https://w3id.org/h2v/property#HHV
:HHV rdf:type owl:NamedIndividual ,
              <https://w3id.org/h2v#DynamicProperty> ;
     <http://qudt.org/schema/qudt/applicableUnit> <http://qudt.org/vocab/unit/MegaJ-PER-M3> ;
     rdfs:comment "The HHV [MJ/m^3] is the current calorific value of fuel on the gas network"^^rdfs:Literal ;
     rdfs:label "HHV"^^rdfs:Literal ;
     <http://www.w3.org/2004/02/skos/core#broader> <http://qudt.org/vocab/quantitykind/EnergyDensity> ;
     <https://w3id.org/h2v#appliesToSystem> <https://w3id.org/h2v#Blender> .


###  https://w3id.org/h2v/property#HHVH2Set
:HHVH2Set rdf:type owl:NamedIndividual ,
                   <https://w3id.org/h2v#PropertySet> ;
          rdfs:label "HHV H2 Set"^^rdfs:Literal ;
          <https://w3id.org/h2v#hasMaximumPropertyMember> :MaximumHHVH2 ;
          <https://w3id.org/h2v#hasMinimumPropertyMember> :MinimumHHVH2 ;
          <https://w3id.org/h2v#hasPropertyMember> :MaximumHHVH2 ,
                                                   :MinimumHHVH2 .


###  https://w3id.org/h2v/property#HydrogenFlowDemand
:HydrogenFlowDemand rdf:type owl:NamedIndividual ,
                             <https://w3id.org/h2v#DynamicProperty> ;
                    <http://qudt.org/schema/qudt/applicableUnit> <http://qudt.org/vocab/unit/KiloGM-PER-HR> ;
                    rdfs:comment "The Hydrogen Flow Demand [kg/h] is the hydrogen flow demand requested by the consumption facility in order to satisfy its need"^^rdfs:Literal ;
                    rdfs:label "Hydrogen Flow Demand"^^rdfs:Literal ;
                    <http://www.w3.org/2004/02/skos/core#broader> <http://qudt.org/vocab/quantitykind/MassFlowRate> ;
                    <https://w3id.org/h2v#appliesToSystem> <https://w3id.org/h2v#HydrogenConsumer> .


###  https://w3id.org/h2v/property#HydrogenFlowDemandSet
:HydrogenFlowDemandSet rdf:type owl:NamedIndividual ,
                                <https://w3id.org/h2v#PropertySet> ;
                       rdfs:label "Hydrogen Flow Demand Set"^^rdfs:Literal ;
                       <https://w3id.org/h2v#hasMaximumPropertyMember> :MaximumHydrogenFlowDemand ;
                       <https://w3id.org/h2v#hasMinimumPropertyMember> :MinimumHydrogenFlowDemand ;
                       <https://w3id.org/h2v#hasPropertyMember> :MaximumHydrogenFlowDemand ,
                                                                :MinimumHydrogenFlowDemand .


###  https://w3id.org/h2v/property#HydrogenPercentage
:HydrogenPercentage rdf:type owl:NamedIndividual ,
                             <https://w3id.org/h2v#DynamicProperty> ;
                    <http://qudt.org/schema/qudt/applicableUnit> <http://qudt.org/vocab/unit/PERCENT> ;
                    rdfs:comment "The Hydrogen Percentage [kgH2/kg gas] is the percentage of current hydrogen on the gas network "^^rdfs:Literal ;
                    rdfs:label "Hydrogen Percentage "^^rdfs:Literal ;
                    <http://www.w3.org/2004/02/skos/core#broader> <http://qudt.org/vocab/quantitykind/DimensionlessRatio> ;
                    <https://w3id.org/h2v#appliesToSystem> <https://w3id.org/h2v#Blender> .


###  https://w3id.org/h2v/property#HydrogenPressureSet
:HydrogenPressureSet rdf:type owl:NamedIndividual ,
                              <https://w3id.org/h2v#PropertySet> ;
                     rdfs:label "Hydrogen Pressure Set"^^rdfs:Literal ;
                     <https://w3id.org/h2v#hasMaximumPropertyMember> :MaximumHydrogenPressure ;
                     <https://w3id.org/h2v#hasMinimumPropertyMember> :MinimumHydrogenPressure ;
                     <https://w3id.org/h2v#hasPropertyMember> :MaximumHydrogenPressure ,
                                                              :MinimumHydrogenPressure .


###  https://w3id.org/h2v/property#Hydrogenpressure
:Hydrogenpressure rdf:type owl:NamedIndividual ,
                           <https://w3id.org/h2v#DynamicProperty> ;
                  <http://qudt.org/schema/qudt/applicableUnit> <http://qudt.org/vocab/unit/BAR> ;
                  rdfs:comment "The Hydrogen pressure [bar] is the hydrogen flow pressure level"^^rdfs:Literal ;
                  rdfs:label "Hydrogen pressure"^^rdfs:Literal ;
                  <http://www.w3.org/2004/02/skos/core#broader> <http://qudt.org/vocab/quantitykind/Pressure> ;
                  <https://w3id.org/h2v#appliesToSystem> <https://w3id.org/h2v#HydrogenConsumer> .


###  https://w3id.org/h2v/property#ImportedHydrogenFlowPressure
:ImportedHydrogenFlowPressure rdf:type owl:NamedIndividual ,
                                       <https://w3id.org/h2v#DynamicProperty> ;
                              <http://qudt.org/schema/qudt/applicableUnit> <https://w3id.org/h2v#BARG> ;
                              rdfs:comment "The Imported Hydrogen Flow Pressure [barg] is the hydrogen flow pressure level during the import operations"^^rdfs:Literal ;
                              rdfs:label "Imported Hydrogen Flow Pressure"^^rdfs:Literal ;
                              <http://www.w3.org/2004/02/skos/core#broader> <http://qudt.org/vocab/quantitykind/GaugePressure> ;
                              <https://w3id.org/h2v#appliesToSystem> <https://w3id.org/h2v#HydrogenStorage> .


###  https://w3id.org/h2v/property#ImportedHydrogenPressureSet
:ImportedHydrogenPressureSet rdf:type owl:NamedIndividual ,
                                      <https://w3id.org/h2v#PropertySet> ;
                             rdfs:label "Imported Hydrogen Pressure Set"^^rdfs:Literal ;
                             <https://w3id.org/h2v#hasMaximumPropertyMember> :MaximumImportedHydrogenPressure ;
                             <https://w3id.org/h2v#hasMinimumPropertyMember> :MinimumImportedHydrogenPressure ;
                             <https://w3id.org/h2v#hasPropertyMember> :MaximumImportedHydrogenPressure ,
                                                                      :MinimumImportedHydrogenPressure .


###  https://w3id.org/h2v/property#InletCH4Flow
:InletCH4Flow rdf:type owl:NamedIndividual ,
                       <https://w3id.org/h2v#DynamicProperty> ;
              <http://qudt.org/schema/qudt/applicableUnit> <http://qudt.org/vocab/unit/KiloGM-PER-HR> ;
              rdfs:comment "The Inlet CH4 Flow [kg/h] of the blender of the HV is the actual measured CH4 inlet flow"^^rdfs:Literal ;
              rdfs:label "Inlet CH4 Flow"^^rdfs:Literal ;
              <http://www.w3.org/2004/02/skos/core#broader> <http://qudt.org/vocab/quantitykind/MassFlowRate> ;
              <https://w3id.org/h2v#appliesToSystem> <https://w3id.org/h2v#Blender> .


###  https://w3id.org/h2v/property#InletH2Flow
:InletH2Flow rdf:type owl:NamedIndividual ,
                      <https://w3id.org/h2v#DynamicProperty> ;
             <http://qudt.org/schema/qudt/applicableUnit> <http://qudt.org/vocab/unit/KiloGM-PER-HR> ;
             rdfs:comment "The Inlet H2 Flow [Kg/h] of the blender of the HV is the actual measured h2 inlet flow"^^rdfs:Literal ;
             rdfs:label "Inlet H2 Flow"^^rdfs:Literal ;
             <http://www.w3.org/2004/02/skos/core#broader> <http://qudt.org/vocab/quantitykind/MassFlowRate> ;
             <https://w3id.org/h2v#appliesToSystem> <https://w3id.org/h2v#Blender> .


###  https://w3id.org/h2v/property#InletMassFlow
:InletMassFlow rdf:type owl:NamedIndividual ,
                        <https://w3id.org/h2v#DynamicProperty> ;
               <http://qudt.org/schema/qudt/applicableUnit> <http://qudt.org/vocab/unit/KiloGM-PER-HR> ;
               rdfs:comment "The Inlet Mass Flow [kg/h]  is the hydrogen flow that can be received from the HV"^^rdfs:Literal ;
               rdfs:label "Inlet Mass Flow"^^rdfs:Literal ;
               <http://www.w3.org/2004/02/skos/core#broader> <http://qudt.org/vocab/quantitykind/MassFlowRate> ;
               <https://w3id.org/h2v#appliesToSystem> <https://w3id.org/h2v#Blender> .


###  https://w3id.org/h2v/property#InletMassFlowToleratedSet
:InletMassFlowToleratedSet rdf:type owl:NamedIndividual ,
                                    <https://w3id.org/h2v#PropertySet> ;
                           rdfs:label "Inlet Mass Flow Tolerated Set"^^rdfs:Literal ;
                           <https://w3id.org/h2v#hasMaximumPropertyMember> :MaximumInletMassFlowTolerated ;
                           <https://w3id.org/h2v#hasMinimumPropertyMember> :MinimumInletMassFlowTolerated ;
                           <https://w3id.org/h2v#hasPropertyMember> :MaximumInletMassFlowTolerated ,
                                                                    :MinimumInletMassFlowTolerated .


###  https://w3id.org/h2v/property#InletWaterPressure
:InletWaterPressure rdf:type owl:NamedIndividual ,
                             <https://w3id.org/h2v#DynamicProperty> ;
                    <http://qudt.org/schema/qudt/applicableUnit> <https://w3id.org/h2v#BARG> ;
                    rdfs:comment "The Inlet Water Pressure [barg] is the measured inlet water pressure in the electrolyzer "^^rdfs:Literal ;
                    rdfs:label "Inlet Water Pressure"^^rdfs:Literal ;
                    <http://www.w3.org/2004/02/skos/core#broader> <http://qudt.org/vocab/quantitykind/GaugePressure> ;
                    <https://w3id.org/h2v#appliesToSystem> <https://w3id.org/h2v#Electrolyzer> .


###  https://w3id.org/h2v/property#InletWaterPressureSet
:InletWaterPressureSet rdf:type owl:NamedIndividual ,
                                <https://w3id.org/h2v#PropertySet> ;
                       rdfs:label "Inlet Water Pressure Set"^^rdfs:Literal ;
                       <https://w3id.org/h2v#hasMaximumPropertyMember> :MaximumInletWaterPressure ;
                       <https://w3id.org/h2v#hasMinimumPropertyMember> :MinimumInletWaterPressure ;
                       <https://w3id.org/h2v#hasOptimalPropertyMember> :OptimalInletWaterPressure ;
                       <https://w3id.org/h2v#hasPropertyMember> :MaximumInletWaterPressure ,
                                                                :MinimumInletWaterPressure ,
                                                                :OptimalInletWaterPressure .


###  https://w3id.org/h2v/property#InputMassFlow
:InputMassFlow rdf:type owl:NamedIndividual ,
                        <https://w3id.org/h2v#DynamicProperty> ;
               <http://qudt.org/schema/qudt/applicableUnit> <http://qudt.org/vocab/unit/KiloGM-PER-HR> ;
               rdfs:comment "The Input Mass Flow [kg/h] is the hydrogen input flow to storage"^^rdfs:Literal ;
               rdfs:label "Input Mass Flow"^^rdfs:Literal ;
               <http://www.w3.org/2004/02/skos/core#broader> <http://qudt.org/vocab/quantitykind/MassFlowRate> ;
               <https://w3id.org/h2v#appliesToSystem> <https://w3id.org/h2v#HydrogenStorage> .


###  https://w3id.org/h2v/property#InputMassFlowSet
:InputMassFlowSet rdf:type owl:NamedIndividual ,
                           <https://w3id.org/h2v#PropertySet> ;
                  rdfs:label "Input Mass Flow Set"^^rdfs:Literal ;
                  <https://w3id.org/h2v#hasMaximumPropertyMember> :MaximumInputMassFlow ;
                  <https://w3id.org/h2v#hasMinimumPropertyMember> :MinimumInputMassFlow ;
                  <https://w3id.org/h2v#hasPropertyMember> :MaximumInputMassFlow ,
                                                           :MinimumInputMassFlow .


###  https://w3id.org/h2v/property#InputPressure
:InputPressure rdf:type owl:NamedIndividual ,
                        <https://w3id.org/h2v#DynamicProperty> ;
               <http://qudt.org/schema/qudt/applicableUnit> <https://w3id.org/h2v#BARG> ;
               rdfs:comment "The Input Pressure [barg] of the storage of the HV is the hydrogen pressure as input to storage"^^rdfs:Literal ;
               rdfs:label "Input Pressure"^^rdfs:Literal ;
               <http://www.w3.org/2004/02/skos/core#broader> <http://qudt.org/vocab/quantitykind/GaugePressure> ;
               <https://w3id.org/h2v#appliesToSystem> <https://w3id.org/h2v#HydrogenStorage> .


###  https://w3id.org/h2v/property#InputPressureSet
:InputPressureSet rdf:type owl:NamedIndividual ,
                           <https://w3id.org/h2v#PropertySet> ;
                  rdfs:label "Input Pressure Set"^^rdfs:Literal ;
                  <https://w3id.org/h2v#hasMaximumPropertyMember> :MaximumInputPressure ;
                  <https://w3id.org/h2v#hasMinimumPropertyMember> :MinimumInputPressure ;
                  <https://w3id.org/h2v#hasPropertyMember> :MaximumInputPressure ,
                                                           :MinimumInputPressure .


###  https://w3id.org/h2v/property#InputTemperature
:InputTemperature rdf:type owl:NamedIndividual ,
                           <https://w3id.org/h2v#DynamicProperty> ;
                  <http://qudt.org/schema/qudt/applicableUnit> <http://qudt.org/vocab/unit/DEG_C> ;
                  rdfs:comment "The Input Temperature [°C] of the storage of the HV is the hydrogen input temperature at storage"^^rdfs:Literal ;
                  rdfs:label "Input Temperature"^^rdfs:Literal ;
                  <http://www.w3.org/2004/02/skos/core#broader> <http://qudt.org/vocab/quantitykind/Temperature> ;
                  <https://w3id.org/h2v#appliesToSystem> <https://w3id.org/h2v#HydrogenStorage> .


###  https://w3id.org/h2v/property#InputTemperatureSet
:InputTemperatureSet rdf:type owl:NamedIndividual ,
                              <https://w3id.org/h2v#PropertySet> ;
                     rdfs:label "Input Temperature Set"^^rdfs:Literal ;
                     <https://w3id.org/h2v#hasMaximumPropertyMember> :MaximumInputTemperature ;
                     <https://w3id.org/h2v#hasMinimumPropertyMember> :MinimumInputTemperature ;
                     <https://w3id.org/h2v#hasPropertyMember> :MaximumInputTemperature ,
                                                              :MinimumInputTemperature .


###  https://w3id.org/h2v/property#ManualValveNormalOpen
:ManualValveNormalOpen rdf:type owl:NamedIndividual ,
                                <https://w3id.org/h2v#StaticProperty> ;
                       <http://qudt.org/schema/qudt/applicableUnit> <http://qudt.org/vocab/unit/UNITLESS> ;
                       rdfs:comment "The Manual Valve Normal Open [boolean] is used when no measurements for the state of the value is present. If the value is 1, the valve is normally open, if the value is 0, the valve is normally closed."^^rdfs:Literal ;
                       rdfs:label "Manual Valve Normal Open"^^rdfs:Literal ;
                       <http://www.w3.org/2004/02/skos/core#broader> <http://qudt.org/vocab/quantitykind/Dimensionless> ;
                       <https://w3id.org/h2v#appliesToSystem> <https://w3id.org/h2v#ManualValve> .


###  https://w3id.org/h2v/property#ManualValveState
:ManualValveState rdf:type owl:NamedIndividual ,
                           <https://w3id.org/h2v#DynamicProperty> ;
                  <http://qudt.org/schema/qudt/applicableUnit> <http://qudt.org/vocab/unit/UNITLESS> ;
                  rdfs:comment "The Manual Valve State [boolean] of the manual valve of the HV is the actual state of the valve. If the value is 1, the valve is open, if the value is 0, the valve is closed."^^rdfs:Literal ;
                  rdfs:label "Manual Valve State"^^rdfs:Literal ;
                  <http://www.w3.org/2004/02/skos/core#broader> <http://qudt.org/vocab/quantitykind/Dimensionless> ;
                  <https://w3id.org/h2v#appliesToSystem> <https://w3id.org/h2v#ManualValve> .


###  https://w3id.org/h2v/property#MaximumAmountofStoredDistilledWater
:MaximumAmountofStoredDistilledWater rdf:type owl:NamedIndividual ,
                                              <https://w3id.org/h2v#StaticProperty> ;
                                     <http://qudt.org/schema/qudt/applicableUnit> <http://qudt.org/vocab/unit/KiloGM> ;
                                     rdfs:comment "The Maximum Amount of Stored Distilled Water [kg] of the electrolyzer is the maximum quantity of distilled water that can be contained in water storage of the electrolyzer"^^rdfs:Literal ;
                                     rdfs:label "Maximum Amount of Stored Distilled Water"^^rdfs:Literal ;
                                     <http://www.w3.org/2004/02/skos/core#broader> <http://qudt.org/vocab/quantitykind/Mass> ;
                                     <https://w3id.org/h2v#appliesToSystem> <https://w3id.org/h2v#Electrolyzer> .


###  https://w3id.org/h2v/property#MaximumCH4Flow
:MaximumCH4Flow rdf:type owl:NamedIndividual ,
                         <https://w3id.org/h2v#StaticProperty> ;
                <http://qudt.org/schema/qudt/applicableUnit> <http://qudt.org/vocab/unit/KiloGM-PER-HR> ;
                rdfs:comment "The Maximum CH4 Flow [kg/h] of the blender of the HV is the maximum value of CH4 allowed in input of the blender"^^rdfs:Literal ;
                rdfs:label "Maximum CH4 Flow"^^rdfs:Literal ;
                <http://www.w3.org/2004/02/skos/core#broader> <http://qudt.org/vocab/quantitykind/MassFlowRate> ;
                <https://w3id.org/h2v#appliesToSystem> <https://w3id.org/h2v#Blender> .


###  https://w3id.org/h2v/property#MaximumCH4InletGasFlow
:MaximumCH4InletGasFlow rdf:type owl:NamedIndividual ,
                                 <https://w3id.org/h2v#StaticProperty> ;
                        <http://qudt.org/schema/qudt/applicableUnit> <http://qudt.org/vocab/unit/SCM-PER-HR> ;
                        rdfs:comment "The Maximum CH4 Inlet Gas Flow [Nm3/h] of the blender of the HV is the maximum value of CH4 allowed in input of the blender"^^rdfs:Literal ;
                        rdfs:label "Maximum CH4 Inlet Gas Flow"^^rdfs:Literal ;
                        <http://www.w3.org/2004/02/skos/core#broader> <http://qudt.org/vocab/quantitykind/MolarFlowRate> ;
                        <https://w3id.org/h2v#appliesToSystem> <https://w3id.org/h2v#Blender> .


###  https://w3id.org/h2v/property#MaximumDepthofDischarge
:MaximumDepthofDischarge rdf:type owl:NamedIndividual ,
                                  <https://w3id.org/h2v#StaticProperty> ;
                         <http://qudt.org/schema/qudt/applicableUnit> <http://qudt.org/vocab/unit/PERCENT> ;
                         rdfs:comment "The Maximum Depth of Discharge [%] of the storage of the HV is the maximum percentage of discharge allowed by the storage (hydrogen storage allows discharging up to a certain pressure limit value to keep the system safe)"^^rdfs:Literal ;
                         rdfs:label "Maximum Depth of Discharge"^^rdfs:Literal ;
                         <http://www.w3.org/2004/02/skos/core#broader> <http://qudt.org/vocab/quantitykind/PressureRatio> ;
                         <https://w3id.org/h2v#appliesToSystem> <https://w3id.org/h2v#HydrogenStorage> .


###  https://w3id.org/h2v/property#MaximumDistilledWaterTemperature
:MaximumDistilledWaterTemperature rdf:type owl:NamedIndividual ,
                                           <https://w3id.org/h2v#StaticProperty> ;
                                  <http://qudt.org/schema/qudt/applicableUnit> <http://qudt.org/vocab/unit/DEG_C> ;
                                  rdfs:comment "The Maximum Distilled Water Temperature [°C] of the electrolyzer of the HV is the maximum temperature of the water stream allowed in the system"^^rdfs:Literal ;
                                  rdfs:label "Maximum Distilled Water Temperature"^^rdfs:Literal ;
                                  <http://www.w3.org/2004/02/skos/core#broader> <http://qudt.org/vocab/quantitykind/Temperature> ;
                                  <https://w3id.org/h2v#appliesToSystem> <https://w3id.org/h2v#Electrolyzer> .


###  https://w3id.org/h2v/property#MaximumElectricPower
:MaximumElectricPower rdf:type owl:NamedIndividual ,
                               <https://w3id.org/h2v#StaticProperty> ;
                      <http://qudt.org/schema/qudt/applicableUnit> <http://qudt.org/vocab/unit/KiloW> ;
                      rdfs:comment "The Maximum Electric Power [kW] of the electrolyzer of the HV is the maximum power that can be absorbed by the electrolyzer without compromising the integrity of its components."^^rdfs:Literal ;
                      rdfs:label "Maximum Electric Power"^^rdfs:Literal ;
                      <http://www.w3.org/2004/02/skos/core#broader> <http://qudt.org/vocab/quantitykind/ElectricPower> ;
                      <https://w3id.org/h2v#appliesToSystem> <https://w3id.org/h2v#Electrolyzer> .


###  https://w3id.org/h2v/property#MaximumExportedHydrogenPressure
:MaximumExportedHydrogenPressure rdf:type owl:NamedIndividual ,
                                          <https://w3id.org/h2v#StaticProperty> ;
                                 <http://qudt.org/schema/qudt/applicableUnit> <https://w3id.org/h2v#BARG> ;
                                 rdfs:comment "The Maximum Exported Hydrogen Pressure [barg] is the maximum acceptable hydrogen pressure due to plants’ constraints for the export operations"^^rdfs:Literal ;
                                 rdfs:label "Maximum Exported Hydrogen Pressure"^^rdfs:Literal ;
                                 <http://www.w3.org/2004/02/skos/core#broader> <http://qudt.org/vocab/quantitykind/GaugePressure> ;
                                 <https://w3id.org/h2v#appliesToSystem> <https://w3id.org/h2v#HydrogenStorage> .


###  https://w3id.org/h2v/property#MaximumGasComposition
:MaximumGasComposition rdf:type owl:NamedIndividual ,
                                <https://w3id.org/h2v#StaticProperty> ;
                       <http://qudt.org/schema/qudt/applicableUnit> <http://qudt.org/vocab/unit/PPM> ;
                       rdfs:comment """
The Maximum Gas Composition [ppm] of the electrolyzer of the HV is the maximum level of gas contaminant  (O2 , H2O and N2 ) allowed in the mainstream to be exported to consumers downstream of the treatment systems"""^^rdfs:Literal ;
                       rdfs:label "Maximum Gas Composition"^^rdfs:Literal ;
                       <http://www.w3.org/2004/02/skos/core#broader> <http://qudt.org/vocab/quantitykind/DimensionlessRatio> ;
                       <https://w3id.org/h2v#appliesToSystem> <https://w3id.org/h2v#Electrolyzer> .


###  https://w3id.org/h2v/property#MaximumH2InletGasFlow
:MaximumH2InletGasFlow rdf:type owl:NamedIndividual ,
                                <https://w3id.org/h2v#StaticProperty> ;
                       <http://qudt.org/schema/qudt/applicableUnit> <http://qudt.org/vocab/unit/SCM-PER-HR> ;
                       rdfs:comment "The Maximum H2 Inlet Gas Flow [Nm3/h] of the blender of the HV is the maximum value of H2 allowed in input of the blender"^^rdfs:Literal ;
                       rdfs:label "Maximum H2 Inlet Gas Flow"^^rdfs:Literal ;
                       <http://www.w3.org/2004/02/skos/core#broader> <http://qudt.org/vocab/quantitykind/MolarFlowRate> ;
                       <https://w3id.org/h2v#appliesToSystem> <https://w3id.org/h2v#Blender> .


###  https://w3id.org/h2v/property#MaximumH2O
:MaximumH2O rdf:type owl:NamedIndividual ,
                     <https://w3id.org/h2v#StaticProperty> ;
            <http://qudt.org/schema/qudt/applicableUnit> <http://qudt.org/vocab/unit/PPM> ;
            rdfs:comment "The Maximum H2O [ppm] of the electrolyzer of the HV is the maximum level of water vapor allowed in the mainstream to be exported to consumers downstream of the treatment systems"^^rdfs:Literal ;
            rdfs:label "Maximum H2O"^^rdfs:Literal ;
            <http://www.w3.org/2004/02/skos/core#broader> <http://qudt.org/vocab/quantitykind/DimensionlessRatio> ;
            <https://w3id.org/h2v#appliesToSystem> <https://w3id.org/h2v#Electrolyzer> .


###  https://w3id.org/h2v/property#MaximumH2Pressure
:MaximumH2Pressure rdf:type owl:NamedIndividual ,
                            <https://w3id.org/h2v#StaticProperty> ;
                   <http://qudt.org/schema/qudt/applicableUnit> <https://w3id.org/h2v#BARG> ;
                   rdfs:comment "The Maximum H2 Pressure [barg] of the electrolyzer of the HV is the maximum pressure of the hydrogen stream allowed as output of the system"^^rdfs:Literal ;
                   rdfs:label "Maximum H2 Pressure"^^rdfs:Literal ;
                   <http://www.w3.org/2004/02/skos/core#broader> <http://qudt.org/vocab/quantitykind/GaugePressure> ;
                   <https://w3id.org/h2v#appliesToSystem> <https://w3id.org/h2v#Electrolyzer> .


###  https://w3id.org/h2v/property#MaximumH2Production
:MaximumH2Production rdf:type owl:NamedIndividual ,
                              <https://w3id.org/h2v#StaticProperty> ;
                     <http://qudt.org/schema/qudt/applicableUnit> <http://qudt.org/vocab/unit/KiloGM-PER-HR> ;
                     rdfs:comment "The Maximum H2 Production [kg/h] of the electrolyzer of the HV is the maximum flow rate possible at the output of the electrolyzer "^^rdfs:Literal ;
                     rdfs:label "Maximum H2 Production"^^rdfs:Literal ;
                     <http://www.w3.org/2004/02/skos/core#broader> <http://qudt.org/vocab/quantitykind/MassFlowRate> ;
                     <https://w3id.org/h2v#appliesToSystem> <https://w3id.org/h2v#Electrolyzer> .


###  https://w3id.org/h2v/property#MaximumH2Temperature
:MaximumH2Temperature rdf:type owl:NamedIndividual ,
                               <https://w3id.org/h2v#StaticProperty> ;
                      <http://qudt.org/schema/qudt/applicableUnit> <http://qudt.org/vocab/unit/DEG_C> ;
                      rdfs:comment "The Maximum H2 Temperature [°C] of the electrolyzer of the HV is the maximum temperature of the hydrogen stream allowed as output of the system"^^rdfs:Literal ;
                      rdfs:label "Maximum H2 Temperature"^^rdfs:Literal ;
                      <http://www.w3.org/2004/02/skos/core#broader> <http://qudt.org/vocab/quantitykind/Temperature> ;
                      <https://w3id.org/h2v#appliesToSystem> <https://w3id.org/h2v#Electrolyzer> .


###  https://w3id.org/h2v/property#MaximumHHVH2
:MaximumHHVH2 rdf:type owl:NamedIndividual ,
                       <https://w3id.org/h2v#StaticProperty> ;
              <http://qudt.org/schema/qudt/applicableUnit> <http://qudt.org/vocab/unit/MegaJ-PER-M3> ;
              rdfs:comment "The Maximum HHV H2 [MJ/m^3] is the maximum upper calorific value of hydrogen accepted for gas (energy contained in the fuel per cubic metre under defined normal thermodynamic conditions)"^^rdfs:Literal ;
              rdfs:label "Maximum HHV H2"^^rdfs:Literal ;
              <http://www.w3.org/2004/02/skos/core#broader> <http://qudt.org/vocab/quantitykind/EnergyDensity> ;
              <https://w3id.org/h2v#appliesToSystem> <https://w3id.org/h2v#Blender> .


###  https://w3id.org/h2v/property#MaximumHydrogenFlowDemand
:MaximumHydrogenFlowDemand rdf:type owl:NamedIndividual ,
                                    <https://w3id.org/h2v#StaticProperty> ;
                           <http://qudt.org/schema/qudt/applicableUnit> <http://qudt.org/vocab/unit/KiloGM-PER-HR> ;
                           rdfs:comment "The Maximum Hydrogen flow demand [kg/h] is the maximum  acceptable hydrogen flow due to plants’ constraints"^^rdfs:Literal ;
                           rdfs:label "Maximum Hydrogen Flow Demand"^^rdfs:Literal ;
                           <http://www.w3.org/2004/02/skos/core#broader> <http://qudt.org/vocab/quantitykind/MassFlowRate> ;
                           <https://w3id.org/h2v#appliesToSystem> <https://w3id.org/h2v#HydrogenConsumer> .


###  https://w3id.org/h2v/property#MaximumHydrogenPressure
:MaximumHydrogenPressure rdf:type owl:NamedIndividual ,
                                  <https://w3id.org/h2v#StaticProperty> ;
                         <http://qudt.org/schema/qudt/applicableUnit> <http://qudt.org/vocab/unit/BAR> ;
                         rdfs:comment "The Maximum Hydrogen Pressure [bar] is the maximum acceptable hydrogen pressure due to plants’ constraints"^^rdfs:Literal ;
                         rdfs:label "Maximum Hydrogen Pressure"^^rdfs:Literal ;
                         <http://www.w3.org/2004/02/skos/core#broader> <http://qudt.org/vocab/quantitykind/Pressure> ;
                         <https://w3id.org/h2v#appliesToSystem> <https://w3id.org/h2v#HydrogenConsumer> .


###  https://w3id.org/h2v/property#MaximumHydrogenVolumePercentage
:MaximumHydrogenVolumePercentage rdf:type owl:NamedIndividual ,
                                          <https://w3id.org/h2v#StaticProperty> ;
                                 <http://qudt.org/schema/qudt/applicableUnit> <http://qudt.org/vocab/unit/PERCENT> ;
                                 rdfs:comment "The Maximum Hydrogen Volume Percentage [%] is the maximum hydrogen percentage in volume acceptable by the gas network"^^rdfs:Literal ;
                                 rdfs:label "Maximum Hydrogen Volume Percentage"^^rdfs:Literal ;
                                 <http://www.w3.org/2004/02/skos/core#broader> <http://qudt.org/vocab/quantitykind/DimensionlessRatio> ;
                                 <https://w3id.org/h2v#appliesToSystem> <https://w3id.org/h2v#Blender> .


###  https://w3id.org/h2v/property#MaximumImportedHydrogenPressure
:MaximumImportedHydrogenPressure rdf:type owl:NamedIndividual ,
                                          <https://w3id.org/h2v#StaticProperty> ;
                                 <http://qudt.org/schema/qudt/applicableUnit> <https://w3id.org/h2v#BARG> ;
                                 rdfs:comment "The Maximum Imported Hydrogen Pressure [barg] is the maximum acceptable hydrogen pressure due to plants’ constraints for the import operations"^^rdfs:Literal ;
                                 rdfs:label "Maximum Imported Hydrogen Pressure"^^rdfs:Literal ;
                                 <http://www.w3.org/2004/02/skos/core#broader> <http://qudt.org/vocab/quantitykind/GaugePressure> ;
                                 <https://w3id.org/h2v#appliesToSystem> <https://w3id.org/h2v#HydrogenStorage> .


###  https://w3id.org/h2v/property#MaximumInletMassFlowTolerated
:MaximumInletMassFlowTolerated rdf:type owl:NamedIndividual ,
                                        <https://w3id.org/h2v#StaticProperty> ;
                               <http://qudt.org/schema/qudt/applicableUnit> <http://qudt.org/vocab/unit/KiloGM-PER-HR> ;
                               rdfs:comment "The Maximum Inlet Mass Flow Tolerated [kg/h]  is the maximum hydrogen flow that can be received from the HV"^^rdfs:Literal ;
                               rdfs:label "Maximum Inlet Mass Flow Tolerated"^^rdfs:Literal ;
                               <http://www.w3.org/2004/02/skos/core#broader> <http://qudt.org/vocab/quantitykind/MassFlowRate> ;
                               <https://w3id.org/h2v#appliesToSystem> <https://w3id.org/h2v#Blender> .


###  https://w3id.org/h2v/property#MaximumInletWaterPressure
:MaximumInletWaterPressure rdf:type owl:NamedIndividual ,
                                    <https://w3id.org/h2v#StaticProperty> ;
                           <http://qudt.org/schema/qudt/applicableUnit> <https://w3id.org/h2v#BARG> ;
                           rdfs:comment "The Maximum Inlet Water Pressure [barg] of the electrolyzer of the HV  is the maximum amount of water pressure allowed by the electrolyzer"^^rdfs:Literal ;
                           rdfs:label "Maximum Inlet Water Pressure "^^rdfs:Literal ;
                           <http://www.w3.org/2004/02/skos/core#broader> <http://qudt.org/vocab/quantitykind/GaugePressure> ;
                           <https://w3id.org/h2v#appliesToSystem> <https://w3id.org/h2v#Electrolyzer> .


###  https://w3id.org/h2v/property#MaximumInputMassFlow
:MaximumInputMassFlow rdf:type owl:NamedIndividual ,
                               <https://w3id.org/h2v#StaticProperty> ;
                      <http://qudt.org/schema/qudt/applicableUnit> <http://qudt.org/vocab/unit/KiloGM-PER-HR> ;
                      rdfs:comment "The Maximum Input Mass Flow [kg/h] of the storage of the HV is the maximum hydrogen flow allowed as input to storage"^^rdfs:Literal ;
                      rdfs:label "Maximum Input Mass Flow"^^rdfs:Literal ;
                      <http://www.w3.org/2004/02/skos/core#broader> <http://qudt.org/vocab/quantitykind/MassFlowRate> ;
                      <https://w3id.org/h2v#appliesToSystem> <https://w3id.org/h2v#HydrogenStorage> .


###  https://w3id.org/h2v/property#MaximumInputPressure
:MaximumInputPressure rdf:type owl:NamedIndividual ,
                               <https://w3id.org/h2v#StaticProperty> ;
                      <http://qudt.org/schema/qudt/applicableUnit> <https://w3id.org/h2v#BARG> ;
                      rdfs:comment "The Maximum Input Pressure [barg] of the storage of the HV is the  maximum hydrogen pressure allowed as input to storage"^^rdfs:Literal ;
                      rdfs:label "Maximum Input Pressure"^^rdfs:Literal ;
                      <http://www.w3.org/2004/02/skos/core#broader> <http://qudt.org/vocab/quantitykind/GaugePressure> ;
                      <https://w3id.org/h2v#appliesToSystem> <https://w3id.org/h2v#HydrogenStorage> .


###  https://w3id.org/h2v/property#MaximumInputTemperature
:MaximumInputTemperature rdf:type owl:NamedIndividual ,
                                  <https://w3id.org/h2v#StaticProperty> ;
                         <http://qudt.org/schema/qudt/applicableUnit> <http://qudt.org/vocab/unit/DEG_C> ;
                         rdfs:comment "The Maximum Input Temperature [°C] of the storage of the HV is the  maximum hydrogen temperature allowed as input to storage"^^rdfs:Literal ;
                         rdfs:label "Maximum Input Temperature"^^rdfs:Literal ;
                         <http://www.w3.org/2004/02/skos/core#broader> <http://qudt.org/vocab/quantitykind/Temperature> ;
                         <https://w3id.org/h2v#appliesToSystem> <https://w3id.org/h2v#HydrogenStorage> .


###  https://w3id.org/h2v/property#MaximumN2
:MaximumN2 rdf:type owl:NamedIndividual ,
                    <https://w3id.org/h2v#StaticProperty> ;
           <http://qudt.org/schema/qudt/applicableUnit> <http://qudt.org/vocab/unit/PPM> ;
           rdfs:comment "The Maximum N2 [ppm] of the electrolyzer of the HV is the maximum level of nitrogen allowed in the mainstream to be exported to consumers downstream of the treatment systems"^^rdfs:Literal ;
           rdfs:label "Maximum N2 "^^rdfs:Literal ;
           <http://www.w3.org/2004/02/skos/core#broader> <http://qudt.org/vocab/quantitykind/DimensionlessRatio> ;
           <https://w3id.org/h2v#appliesToSystem> <https://w3id.org/h2v#Electrolyzer> .


###  https://w3id.org/h2v/property#MaximumO2
:MaximumO2 rdf:type owl:NamedIndividual ,
                    <https://w3id.org/h2v#StaticProperty> ;
           <http://qudt.org/schema/qudt/applicableUnit> <http://qudt.org/vocab/unit/PPM> ;
           rdfs:comment "The Maximum O2 [ppm] of the electrolyzer of the HV is the maximum level of oxygen allowed in the mainstream to be exported to consumers downstream of the treatment systems"^^rdfs:Literal ;
           rdfs:label "Maximum O2"^^rdfs:Literal ;
           <http://www.w3.org/2004/02/skos/core#broader> <http://qudt.org/vocab/quantitykind/DimensionlessRatio> ;
           <https://w3id.org/h2v#appliesToSystem> <https://w3id.org/h2v#Electrolyzer> .


###  https://w3id.org/h2v/property#MaximumOutletGasFlow
:MaximumOutletGasFlow rdf:type owl:NamedIndividual ,
                               <https://w3id.org/h2v#StaticProperty> ;
                      <http://qudt.org/schema/qudt/applicableUnit> <http://qudt.org/vocab/unit/SCM-PER-HR> ;
                      rdfs:comment "The Maximum Outlet Gas Flow [Nm3/h] of the blender of the HV is the maximum value of blended gas allowed in output of the blender"^^rdfs:Literal ;
                      rdfs:label "Maximum Outlet Gas Flow"^^rdfs:Literal ;
                      <http://www.w3.org/2004/02/skos/core#broader> <http://qudt.org/vocab/quantitykind/MolarFlowRate> ;
                      <https://w3id.org/h2v#appliesToSystem> <https://w3id.org/h2v#Blender> .


###  https://w3id.org/h2v/property#MaximumPipeMassFlow
:MaximumPipeMassFlow rdf:type owl:NamedIndividual ,
                              <https://w3id.org/h2v#StaticProperty> ;
                     <http://qudt.org/schema/qudt/applicableUnit> <http://qudt.org/vocab/unit/KiloGM-PER-HR> ;
                     rdfs:comment "The Maximum Pipe Mass Flow [kg/h] is the maximum transportable hydrogen flow"^^rdfs:Literal ;
                     rdfs:label "Maximum Pipe Mass Flow "^^rdfs:Literal ;
                     <http://www.w3.org/2004/02/skos/core#broader> <http://qudt.org/vocab/quantitykind/MassFlowRate> ;
                     <https://w3id.org/h2v#appliesToSystem> <https://w3id.org/h2v#Pipe> .


###  https://w3id.org/h2v/property#MaximumPipePressure
:MaximumPipePressure rdf:type owl:NamedIndividual ,
                              <https://w3id.org/h2v#StaticProperty> ;
                     <http://qudt.org/schema/qudt/applicableUnit> <http://qudt.org/vocab/unit/BAR> ;
                     rdfs:comment "The Maximum Pipe Pressure [bar] is the maximum pressure of transportable hydrogen"^^rdfs:Literal ;
                     rdfs:label "Maximum Pipe Pressure"^^rdfs:Literal ;
                     <http://www.w3.org/2004/02/skos/core#broader> <http://qudt.org/vocab/quantitykind/Pressure> ;
                     <https://w3id.org/h2v#appliesToSystem> <https://w3id.org/h2v#Pipe> .


###  https://w3id.org/h2v/property#MaximumStoragePressure
:MaximumStoragePressure rdf:type owl:NamedIndividual ,
                                 <https://w3id.org/h2v#StaticProperty> ;
                        <http://qudt.org/schema/qudt/applicableUnit> <https://w3id.org/h2v#BARG> ;
                        rdfs:comment "The Maximum Storage Pressure [barg] of the storage of the HV is the maximum permissible hydrogen pressure inside the storage unit"^^rdfs:Literal ;
                        rdfs:label "Maximum Storage Pressure"^^rdfs:Literal ;
                        <http://www.w3.org/2004/02/skos/core#broader> <http://qudt.org/vocab/quantitykind/GaugePressure> ;
                        <https://w3id.org/h2v#appliesToSystem> <https://w3id.org/h2v#HydrogenStorage> .


###  https://w3id.org/h2v/property#MaximumStorageSize
:MaximumStorageSize rdf:type owl:NamedIndividual ,
                             <https://w3id.org/h2v#StaticProperty> ;
                    <http://qudt.org/schema/qudt/applicableUnit> <http://qudt.org/vocab/unit/L> ;
                    rdfs:comment "The Maximum Storage Size [liter] of the storage of the HV is the maximum nominal quantity of hydrogen that can be contained in storage"^^rdfs:Literal ;
                    rdfs:label "Maximum Storage Size"^^rdfs:Literal ;
                    <http://www.w3.org/2004/02/skos/core#broader> <http://qudt.org/vocab/quantitykind/LiquidVolume> ;
                    <https://w3id.org/h2v#appliesToSystem> <https://w3id.org/h2v#HydrogenStorage> .


###  https://w3id.org/h2v/property#MaximumStorageTemperature
:MaximumStorageTemperature rdf:type owl:NamedIndividual ,
                                    <https://w3id.org/h2v#StaticProperty> ;
                           <http://qudt.org/schema/qudt/applicableUnit> <http://qudt.org/vocab/unit/DEG_C> ;
                           rdfs:comment "The Maximum Storage Temperature [°C] of the storage of the HV is the  maximum permissible hydrogen temperature inside the storage unit"^^rdfs:Literal ;
                           rdfs:label "Maximum Storage Temperature"^^rdfs:Literal ;
                           <http://www.w3.org/2004/02/skos/core#broader> <http://qudt.org/vocab/quantitykind/Temperature> ;
                           <https://w3id.org/h2v#appliesToSystem> <https://w3id.org/h2v#HydrogenStorage> .


###  https://w3id.org/h2v/property#MaximumWaterAcidity
:MaximumWaterAcidity rdf:type owl:NamedIndividual ,
                              <https://w3id.org/h2v#StaticProperty> ;
                     <http://qudt.org/schema/qudt/applicableUnit> <http://qudt.org/vocab/unit/PH> ;
                     rdfs:comment "The Maximum Water Acidity [ph] of the electrolyzer of the HV is the maximum level of acidity of the water allowed in the electrolyzer"^^rdfs:Literal ;
                     rdfs:label "Maximum Water Acidity"^^rdfs:Literal ;
                     <http://www.w3.org/2004/02/skos/core#broader> <http://qudt.org/vocab/quantitykind/Acidity> ;
                     <https://w3id.org/h2v#appliesToSystem> <https://w3id.org/h2v#Electrolyzer> .


###  https://w3id.org/h2v/property#MaximumWaterConductivity
:MaximumWaterConductivity rdf:type owl:NamedIndividual ,
                                   <https://w3id.org/h2v#StaticProperty> ;
                          <http://qudt.org/schema/qudt/applicableUnit> <http://qudt.org/vocab/unit/MicroS-PER-CentiM> ;
                          rdfs:comment "The Maximum Water Conductivity [µS/cm] of the electrolyzer of the HV is the maximum level of water conductivity acceptable. Conductivity measures the ability of water to conduct electricity, which depends on the presence of dissolved ions in water. High conductivity indicates the presence of ionic impurities, which can affect the efficiency of the electrolyzer and cause corrosion or other operational issues"^^rdfs:Literal ;
                          rdfs:label "Maximum Water Conductivity "^^rdfs:Literal ;
                          <http://www.w3.org/2004/02/skos/core#broader> <http://qudt.org/vocab/quantitykind/ElectrolyticConductivity> ;
                          <https://w3id.org/h2v#appliesToSystem> <https://w3id.org/h2v#Electrolyzer> .


###  https://w3id.org/h2v/property#MaximumWaterFlowRate
:MaximumWaterFlowRate rdf:type owl:NamedIndividual ,
                               <https://w3id.org/h2v#StaticProperty> ;
                      <http://qudt.org/schema/qudt/applicableUnit> <http://qudt.org/vocab/unit/KiloGM-PER-HR> ;
                      rdfs:comment "The Maximum Water Flow Rate [kg/h] of the electrolyzer of the HV is the maximum flow rate of distilled water available"^^rdfs:Literal ;
                      rdfs:label "Maximum Water Flow Rate"^^rdfs:Literal ;
                      <http://www.w3.org/2004/02/skos/core#broader> <http://qudt.org/vocab/quantitykind/MassFlowRate> ;
                      <https://w3id.org/h2v#appliesToSystem> <https://w3id.org/h2v#Electrolyzer> .


###  https://w3id.org/h2v/property#MaximumWaterPH
:MaximumWaterPH rdf:type owl:NamedIndividual ,
                         <https://w3id.org/h2v#StaticProperty> ;
                <http://qudt.org/schema/qudt/applicableUnit> <http://qudt.org/vocab/unit/PH> ;
                rdfs:comment "The Maximum Water PH [ph] of the electrolyzer of the HV is the maximum level acceptable of the acidity or basicity of distilled water. The pH can affect the solubility of various compounds and the formation of scale"^^rdfs:Literal ;
                rdfs:label "Maximum Water PH"^^rdfs:Literal ;
                <http://www.w3.org/2004/02/skos/core#broader> <http://qudt.org/vocab/quantitykind/Acidity> ;
                <https://w3id.org/h2v#appliesToSystem> <https://w3id.org/h2v#Electrolyzer> .


###  https://w3id.org/h2v/property#MaximumWaterTemperature
:MaximumWaterTemperature rdf:type owl:NamedIndividual ,
                                  <https://w3id.org/h2v#StaticProperty> ;
                         <http://qudt.org/schema/qudt/applicableUnit> <http://qudt.org/vocab/unit/DEG_C> ;
                         rdfs:comment "The Maximum Water Temperature [°C] of the electrolyzer of the HV is the highest water temperature allowed of the electrolyzer"^^rdfs:Literal ;
                         rdfs:label "Maximum Water Temperature"^^rdfs:Literal ;
                         <http://www.w3.org/2004/02/skos/core#broader> <http://qudt.org/vocab/quantitykind/Temperature> ;
                         <https://w3id.org/h2v#appliesToSystem> <https://w3id.org/h2v#Electrolyzer> .


###  https://w3id.org/h2v/property#MaximumWobbeIndexToleratedH2
:MaximumWobbeIndexToleratedH2 rdf:type owl:NamedIndividual ,
                                       <https://w3id.org/h2v#StaticProperty> ;
                              <http://qudt.org/schema/qudt/applicableUnit> <http://qudt.org/vocab/unit/MegaJ-PER-M3> ;
                              rdfs:comment "The Maximum Wobbe Index Tolerated H2 [MJ/m^3] is the ratio of HHV to the square root of the relative density of the fuel with respect to air. It gives information on the compatibility of a fuel with the gas network"^^rdfs:Literal ;
                              rdfs:label "Maximum Wobbe Index Tolerated H2"^^rdfs:Literal ;
                              <http://www.w3.org/2004/02/skos/core#broader> <http://qudt.org/vocab/quantitykind/EnergyDensity> ;
                              <https://w3id.org/h2v#appliesToSystem> <https://w3id.org/h2v#Blender> .


###  https://w3id.org/h2v/property#MinimumCH4InletGasFlow
:MinimumCH4InletGasFlow rdf:type owl:NamedIndividual ,
                                 <https://w3id.org/h2v#StaticProperty> ;
                        <http://qudt.org/schema/qudt/applicableUnit> <http://qudt.org/vocab/unit/SCM-PER-HR> ;
                        rdfs:comment "The Minimum CH4 Inlet Gas Flow [Nm3/h] of the blender of the HV is the minimum value of CH4 allowed in input of the blender"^^rdfs:Literal ;
                        rdfs:label "Minimum CH4 Inlet Gas Flow"^^rdfs:Literal ;
                        <http://www.w3.org/2004/02/skos/core#broader> <http://qudt.org/vocab/quantitykind/MolarFlowRate> ;
                        <https://w3id.org/h2v#appliesToSystem> <https://w3id.org/h2v#Blender> .


###  https://w3id.org/h2v/property#MinimumDistilledWaterTemperature
:MinimumDistilledWaterTemperature rdf:type owl:NamedIndividual ,
                                           <https://w3id.org/h2v#StaticProperty> ;
                                  <http://qudt.org/schema/qudt/applicableUnit> <http://qudt.org/vocab/unit/DEG_C> ;
                                  rdfs:comment "The Minimum Distilled Water Temperature [°C] of the electrolyzer of the HV is the minimum temperature of the water stream allowed in the system"^^rdfs:Literal ;
                                  rdfs:label "Minimum Distilled Water Temperature"^^rdfs:Literal ;
                                  <http://www.w3.org/2004/02/skos/core#broader> <http://qudt.org/vocab/quantitykind/Temperature> ;
                                  <https://w3id.org/h2v#appliesToSystem> <https://w3id.org/h2v#Electrolyzer> .


###  https://w3id.org/h2v/property#MinimumElectricPower
:MinimumElectricPower rdf:type owl:NamedIndividual ,
                               <https://w3id.org/h2v#StaticProperty> ;
                      <http://qudt.org/schema/qudt/applicableUnit> <http://qudt.org/vocab/unit/KiloW> ;
                      rdfs:comment "The Minimum Electric Power [kW] of the electrolyzer of the HV is the minimum power at which the electrolyzer can operate without compromising the electrolysis reaction"^^rdfs:Literal ;
                      rdfs:label "Minimum Electric Power"^^rdfs:Literal ;
                      <http://www.w3.org/2004/02/skos/core#broader> <http://qudt.org/vocab/quantitykind/ElectricPower> ;
                      <https://w3id.org/h2v#appliesToSystem> <https://w3id.org/h2v#Electrolyzer> .


###  https://w3id.org/h2v/property#MinimumExportedHydrogenPressure
:MinimumExportedHydrogenPressure rdf:type owl:NamedIndividual ,
                                          <https://w3id.org/h2v#StaticProperty> ;
                                 <http://qudt.org/schema/qudt/applicableUnit> <https://w3id.org/h2v#BARG> ;
                                 rdfs:comment "The Minimum Exported Hydrogen Pressure [barg] is the minimum acceptable hydrogen pressure due to plants’ constraints for the export operations"^^rdfs:Literal ;
                                 rdfs:label "Minimum Exported Hydrogen Pressure"^^rdfs:Literal ;
                                 <http://www.w3.org/2004/02/skos/core#broader> <http://qudt.org/vocab/quantitykind/GaugePressure> ;
                                 <https://w3id.org/h2v#appliesToSystem> <https://w3id.org/h2v#HydrogenStorage> .


###  https://w3id.org/h2v/property#MinimumGasComposition
:MinimumGasComposition rdf:type owl:NamedIndividual ,
                                <https://w3id.org/h2v#StaticProperty> ;
                       <http://qudt.org/schema/qudt/applicableUnit> <http://qudt.org/vocab/unit/PPM> ;
                       rdfs:comment "The Minimum Gas Composition [ppm] of the electrolyzer of the HV is the minimum level of gas contaminant  (O2 , H2O and N2 ) allowed in the mainstream to be exported to consumers downstream of the treatment systems"^^rdfs:Literal ;
                       rdfs:label "Minimum Gas Composition"^^rdfs:Literal ;
                       <http://www.w3.org/2004/02/skos/core#broader> <http://qudt.org/vocab/quantitykind/DimensionlessRatio> ;
                       <https://w3id.org/h2v#appliesToSystem> <https://w3id.org/h2v#Electrolyzer> .


###  https://w3id.org/h2v/property#MinimumH2InletGasFlow
:MinimumH2InletGasFlow rdf:type owl:NamedIndividual ,
                                <https://w3id.org/h2v#StaticProperty> ;
                       <http://qudt.org/schema/qudt/applicableUnit> <http://qudt.org/vocab/unit/SCM-PER-HR> ;
                       rdfs:comment "The Minimum H2 Inlet Gas Flow [Nm3/h] of the blender of the HV is the minimum value of H2 allowed in input of the blender"^^rdfs:Literal ;
                       rdfs:label "Minimum H2 Inlet Gas Flow"^^rdfs:Literal ;
                       <http://www.w3.org/2004/02/skos/core#broader> <http://qudt.org/vocab/quantitykind/MolarFlowRate> ;
                       <https://w3id.org/h2v#appliesToSystem> <https://w3id.org/h2v#Blender> .


###  https://w3id.org/h2v/property#MinimumH2O
:MinimumH2O rdf:type owl:NamedIndividual ,
                     <https://w3id.org/h2v#StaticProperty> ;
            <http://qudt.org/schema/qudt/applicableUnit> <http://qudt.org/vocab/unit/PPM> ;
            rdfs:comment "The Minimum H2O [ppm] of the electrolyzer of the HV is the minimum level of water vapor allowed in the mainstream to be exported to consumers downstream of the treatment systems"^^rdfs:Literal ;
            rdfs:label "Minimum H2O"^^rdfs:Literal ;
            <http://www.w3.org/2004/02/skos/core#broader> <http://qudt.org/vocab/quantitykind/DimensionlessRatio> ;
            <https://w3id.org/h2v#appliesToSystem> <https://w3id.org/h2v#Electrolyzer> .


###  https://w3id.org/h2v/property#MinimumH2Pressure
:MinimumH2Pressure rdf:type owl:NamedIndividual ,
                            <https://w3id.org/h2v#StaticProperty> ;
                   <http://qudt.org/schema/qudt/applicableUnit> <https://w3id.org/h2v#BARG> ;
                   rdfs:comment "The Minimum H2 Pressure [barg] of the electrolyzer of the HV is the minimum pressure of the hydrogen stream allowed as output of the system"^^rdfs:Literal ;
                   rdfs:label "Minimum H2 Pressure"^^rdfs:Literal ;
                   <http://www.w3.org/2004/02/skos/core#broader> <http://qudt.org/vocab/quantitykind/GaugePressure> ;
                   <https://w3id.org/h2v#appliesToSystem> <https://w3id.org/h2v#Electrolyzer> .


###  https://w3id.org/h2v/property#MinimumH2Production
:MinimumH2Production rdf:type owl:NamedIndividual ,
                              <https://w3id.org/h2v#StaticProperty> ;
                     <http://qudt.org/schema/qudt/applicableUnit> <http://qudt.org/vocab/unit/KiloGM-PER-HR> ;
                     rdfs:comment "The Minimum H2 Production [kg/h] of the electrolyzer of the HV is the  minimum flow rate possible at the output of the electrolyzer "^^rdfs:Literal ;
                     rdfs:label "Minimum H2 Production"^^rdfs:Literal ;
                     <http://www.w3.org/2004/02/skos/core#broader> <http://qudt.org/vocab/quantitykind/MassFlowRate> ;
                     <https://w3id.org/h2v#appliesToSystem> <https://w3id.org/h2v#Electrolyzer> .


###  https://w3id.org/h2v/property#MinimumH2Temperature
:MinimumH2Temperature rdf:type owl:NamedIndividual ,
                               <https://w3id.org/h2v#StaticProperty> ;
                      <http://qudt.org/schema/qudt/applicableUnit> <http://qudt.org/vocab/unit/DEG_C> ;
                      rdfs:comment "The Minimum H2 Temperature [°C] of the electrolyzer of the HV is the minimum temperature of the hydrogen stream allowed as output of the system"^^rdfs:Literal ;
                      rdfs:label "Minimum H2 Temperature"^^rdfs:Literal ;
                      <http://www.w3.org/2004/02/skos/core#broader> <http://qudt.org/vocab/quantitykind/Temperature> ;
                      <https://w3id.org/h2v#appliesToSystem> <https://w3id.org/h2v#Electrolyzer> .


###  https://w3id.org/h2v/property#MinimumHHVH2
:MinimumHHVH2 rdf:type owl:NamedIndividual ,
                       <https://w3id.org/h2v#StaticProperty> ;
              <http://qudt.org/schema/qudt/applicableUnit> <http://qudt.org/vocab/unit/MegaJ-PER-M3> ;
              rdfs:comment "The Minimum HHV H2 [MJ/m^3] is the minimum upper calorific value of hydrogen accepted for gas (energy contained in the fuel per cubic metre under defined normal thermodynamic conditions)"^^rdfs:Literal ;
              rdfs:label "Minimum HHV H2"^^rdfs:Literal ;
              <http://www.w3.org/2004/02/skos/core#broader> <http://qudt.org/vocab/quantitykind/EnergyDensity> ;
              <https://w3id.org/h2v#appliesToSystem> <https://w3id.org/h2v#Blender> .


###  https://w3id.org/h2v/property#MinimumHydrogenFlowDemand
:MinimumHydrogenFlowDemand rdf:type owl:NamedIndividual ,
                                    <https://w3id.org/h2v#StaticProperty> ;
                           <http://qudt.org/schema/qudt/applicableUnit> <http://qudt.org/vocab/unit/KiloGM-PER-HR> ;
                           rdfs:comment "The Minimum Hydrogen flow demand [kg/h] is the minimum   acceptable hydrogen flow due to plants’ constraints"^^rdfs:Literal ;
                           rdfs:label "Minimum Hydrogen Flow Demand"^^rdfs:Literal ;
                           <http://www.w3.org/2004/02/skos/core#broader> <http://qudt.org/vocab/quantitykind/MassFlowRate> ;
                           <https://w3id.org/h2v#appliesToSystem> <https://w3id.org/h2v#HydrogenConsumer> .


###  https://w3id.org/h2v/property#MinimumHydrogenPressure
:MinimumHydrogenPressure rdf:type owl:NamedIndividual ,
                                  <https://w3id.org/h2v#StaticProperty> ;
                         <http://qudt.org/schema/qudt/applicableUnit> <http://qudt.org/vocab/unit/BAR> ;
                         rdfs:comment "The Minimum Hydrogen Pressure [bar] is the minimum acceptable hydrogen pressure due to plants’ constraints"^^rdfs:Literal ;
                         rdfs:label "Minimum Hydrogen Pressure "^^rdfs:Literal ;
                         <http://www.w3.org/2004/02/skos/core#broader> <http://qudt.org/vocab/quantitykind/Pressure> ;
                         <https://w3id.org/h2v#appliesToSystem> <https://w3id.org/h2v#HydrogenConsumer> .


###  https://w3id.org/h2v/property#MinimumImportedHydrogenPressure
:MinimumImportedHydrogenPressure rdf:type owl:NamedIndividual ,
                                          <https://w3id.org/h2v#StaticProperty> ;
                                 <http://qudt.org/schema/qudt/applicableUnit> <https://w3id.org/h2v#BARG> ;
                                 rdfs:comment "The Minimum Imported Hydrogen Pressure [barg] is the minimum acceptable hydrogen pressure due to plants’ constraints for the import operations"^^rdfs:Literal ;
                                 rdfs:label "Minimum Imported Hydrogen Pressure"^^rdfs:Literal ;
                                 <http://www.w3.org/2004/02/skos/core#broader> <http://qudt.org/vocab/quantitykind/GaugePressure> ;
                                 <https://w3id.org/h2v#appliesToSystem> <https://w3id.org/h2v#HydrogenStorage> .


###  https://w3id.org/h2v/property#MinimumInletMassFlowTolerated
:MinimumInletMassFlowTolerated rdf:type owl:NamedIndividual ,
                                        <https://w3id.org/h2v#StaticProperty> ;
                               <http://qudt.org/schema/qudt/applicableUnit> <http://qudt.org/vocab/unit/KiloGM-PER-HR> ;
                               rdfs:comment "The Minimum Inlet Mass Flow Tolerated [kg/h]  is the minimum hydrogen flow that can be received from the HV"^^rdfs:Literal ;
                               rdfs:label "Minimum Inlet Mass Flow Tolerated"^^rdfs:Literal ;
                               <http://www.w3.org/2004/02/skos/core#broader> <http://qudt.org/vocab/quantitykind/MassFlowRate> ;
                               <https://w3id.org/h2v#appliesToSystem> <https://w3id.org/h2v#Blender> .


###  https://w3id.org/h2v/property#MinimumInletWaterPressure
:MinimumInletWaterPressure rdf:type owl:NamedIndividual ,
                                    <https://w3id.org/h2v#StaticProperty> ;
                           <http://qudt.org/schema/qudt/applicableUnit> <https://w3id.org/h2v#BARG> ;
                           rdfs:comment "The Minimum Inlet Water Pressure [barg] of the electrolyzer of the HV  is the minimum amount of water pressure allowed by the electrolyzer"^^rdfs:Literal ;
                           rdfs:label "Minimum Inlet Water Pressure"^^rdfs:Literal ;
                           <http://www.w3.org/2004/02/skos/core#broader> <http://qudt.org/vocab/quantitykind/GaugePressure> ;
                           <https://w3id.org/h2v#appliesToSystem> <https://w3id.org/h2v#Electrolyzer> .


###  https://w3id.org/h2v/property#MinimumInputMassFlow
:MinimumInputMassFlow rdf:type owl:NamedIndividual ,
                               <https://w3id.org/h2v#StaticProperty> ;
                      <http://qudt.org/schema/qudt/applicableUnit> <http://qudt.org/vocab/unit/KiloGM-PER-HR> ;
                      rdfs:comment "The Minimum Input Mass Flow [kg/h] of the storage of the HV is the minimum hydrogen flow allowed as input to storage"^^rdfs:Literal ;
                      rdfs:label "Minimum Input Mass Flow"^^rdfs:Literal ;
                      <http://www.w3.org/2004/02/skos/core#broader> <http://qudt.org/vocab/quantitykind/MassFlowRate> ;
                      <https://w3id.org/h2v#appliesToSystem> <https://w3id.org/h2v#HydrogenStorage> .


###  https://w3id.org/h2v/property#MinimumInputPressure
:MinimumInputPressure rdf:type owl:NamedIndividual ,
                               <https://w3id.org/h2v#StaticProperty> ;
                      <http://qudt.org/schema/qudt/applicableUnit> <https://w3id.org/h2v#BARG> ;
                      rdfs:comment "The Minimum Input Pressure [barg] of the storage of the HV is the  minimum hydrogen pressure allowed as input to storage"^^rdfs:Literal ;
                      rdfs:label "Minimum Input Pressure"^^rdfs:Literal ;
                      <http://www.w3.org/2004/02/skos/core#broader> <http://qudt.org/vocab/quantitykind/GaugePressure> ;
                      <https://w3id.org/h2v#appliesToSystem> <https://w3id.org/h2v#HydrogenStorage> .


###  https://w3id.org/h2v/property#MinimumInputTemperature
:MinimumInputTemperature rdf:type owl:NamedIndividual ,
                                  <https://w3id.org/h2v#StaticProperty> ;
                         <http://qudt.org/schema/qudt/applicableUnit> <http://qudt.org/vocab/unit/DEG_C> ;
                         rdfs:comment "The Minimum Input Temperature [°C] of the storage of the HV is the  minimum hydrogen temperature allowed as input to storage"^^rdfs:Literal ;
                         rdfs:label "Minimum Input Temperature"^^rdfs:Literal ;
                         <http://www.w3.org/2004/02/skos/core#broader> <http://qudt.org/vocab/quantitykind/Temperature> ;
                         <https://w3id.org/h2v#appliesToSystem> <https://w3id.org/h2v#HydrogenStorage> .


###  https://w3id.org/h2v/property#MinimumN2
:MinimumN2 rdf:type owl:NamedIndividual ,
                    <https://w3id.org/h2v#StaticProperty> ;
           <http://qudt.org/schema/qudt/applicableUnit> <http://qudt.org/vocab/unit/PPM> ;
           rdfs:comment "The Minimum N2 [ppm] of the electrolyzer of the HV is the minimum level of nitrogen allowed in the mainstream to be exported to consumers downstream of the treatment systems"^^rdfs:Literal ;
           rdfs:label "Minimum N2 "^^rdfs:Literal ;
           <http://www.w3.org/2004/02/skos/core#broader> <http://qudt.org/vocab/quantitykind/DimensionlessRatio> ;
           <https://w3id.org/h2v#appliesToSystem> <https://w3id.org/h2v#Electrolyzer> .


###  https://w3id.org/h2v/property#MinimumO2
:MinimumO2 rdf:type owl:NamedIndividual ,
                    <https://w3id.org/h2v#StaticProperty> ;
           <http://qudt.org/schema/qudt/applicableUnit> <http://qudt.org/vocab/unit/PPM> ;
           rdfs:comment "The Minimum O2 [ppm] of the electrolyzer of the HV is the minimum level of oxygen allowed in the mainstream to be exported to consumers downstream of the treatment systems"^^rdfs:Literal ;
           rdfs:label "Minimum O2"^^rdfs:Literal ;
           <http://www.w3.org/2004/02/skos/core#broader> <http://qudt.org/vocab/quantitykind/DimensionlessRatio> ;
           <https://w3id.org/h2v#appliesToSystem> <https://w3id.org/h2v#Electrolyzer> .


###  https://w3id.org/h2v/property#MinimumOutletGasFlow
:MinimumOutletGasFlow rdf:type owl:NamedIndividual ,
                               <https://w3id.org/h2v#StaticProperty> ;
                      <http://qudt.org/schema/qudt/applicableUnit> <http://qudt.org/vocab/unit/SCM-PER-HR> ;
                      rdfs:comment "The Minimum Outlet Gas Flow [Nm3/h] of the blender of the HV is the minimum value of blended gas allowed in output of the blender"^^rdfs:Literal ;
                      rdfs:label "Minimum Outlet Gas Flow"^^rdfs:Literal ;
                      <http://www.w3.org/2004/02/skos/core#broader> <http://qudt.org/vocab/quantitykind/MolarFlowRate> ;
                      <https://w3id.org/h2v#appliesToSystem> <https://w3id.org/h2v#Blender> .


###  https://w3id.org/h2v/property#MinimumOutputHydrogenPurity
:MinimumOutputHydrogenPurity rdf:type owl:NamedIndividual ,
                                      <https://w3id.org/h2v#StaticProperty> ;
                             <http://qudt.org/schema/qudt/applicableUnit> <http://qudt.org/vocab/unit/PERCENT> ;
                             rdfs:comment "The Minimum Output Hydrogen Purity  [%] of the electrolyzer of the HV is the minimum accepted percentage in volume of hydrogen with respect to the total output gas from electrolyzer"^^rdfs:Literal ;
                             rdfs:label "Minimum Output Hydrogen Purity"^^rdfs:Literal ;
                             <http://www.w3.org/2004/02/skos/core#broader> <http://qudt.org/vocab/quantitykind/DimensionlessRatio> ;
                             <https://w3id.org/h2v#appliesToSystem> <https://w3id.org/h2v#Electrolyzer> .


###  https://w3id.org/h2v/property#MinimumPipePressure
:MinimumPipePressure rdf:type owl:NamedIndividual ,
                              <https://w3id.org/h2v#StaticProperty> ;
                     <http://qudt.org/schema/qudt/applicableUnit> <http://qudt.org/vocab/unit/BAR> ;
                     rdfs:comment """
The Minimum Pipe Pressure [bar] is the minimum pressure of transportable hydrogen"""^^rdfs:Literal ;
                     rdfs:label "Minimum Pipe Pressure"^^rdfs:Literal ;
                     <http://www.w3.org/2004/02/skos/core#broader> <http://qudt.org/vocab/quantitykind/Pressure> ;
                     <https://w3id.org/h2v#appliesToSystem> <https://w3id.org/h2v#Pipe> .


###  https://w3id.org/h2v/property#MinimumStoragePressure
:MinimumStoragePressure rdf:type owl:NamedIndividual ,
                                 <https://w3id.org/h2v#StaticProperty> ;
                        <http://qudt.org/schema/qudt/applicableUnit> <https://w3id.org/h2v#BARG> ;
                        rdfs:comment "The Minimum Storage Pressure [barg] of the storage of the HV is the minimum permissible hydrogen pressure inside the storage unit"^^rdfs:Literal ;
                        rdfs:label "Minimum Storage Pressure"^^rdfs:Literal ;
                        <http://www.w3.org/2004/02/skos/core#broader> <http://qudt.org/vocab/quantitykind/GaugePressure> ;
                        <https://w3id.org/h2v#appliesToSystem> <https://w3id.org/h2v#HydrogenStorage> .


###  https://w3id.org/h2v/property#MinimumStorageSize
:MinimumStorageSize rdf:type owl:NamedIndividual ,
                             <https://w3id.org/h2v#StaticProperty> ;
                    <http://qudt.org/schema/qudt/applicableUnit> <http://qudt.org/vocab/unit/L> ;
                    rdfs:comment "The Minimum Storage Size [liter] of the storage of the HV is the minimum nominal quantity of hydrogen that can be contained in storage"^^rdfs:Literal ;
                    rdfs:label "Minimum Storage Size"^^rdfs:Literal ;
                    <http://www.w3.org/2004/02/skos/core#broader> <http://qudt.org/vocab/quantitykind/LiquidVolume> ;
                    <https://w3id.org/h2v#appliesToSystem> <https://w3id.org/h2v#HydrogenStorage> .


###  https://w3id.org/h2v/property#MinimumStorageTemperature
:MinimumStorageTemperature rdf:type owl:NamedIndividual ,
                                    <https://w3id.org/h2v#StaticProperty> ;
                           <http://qudt.org/schema/qudt/applicableUnit> <http://qudt.org/vocab/unit/DEG_C> ;
                           rdfs:comment "The Minimum Storage Temperature [°C] of the storage of the HV is the  minimum permissible hydrogen temperature inside the storage unit"^^rdfs:Literal ;
                           rdfs:label "Minimum Storage Temperature"^^rdfs:Literal ;
                           <http://www.w3.org/2004/02/skos/core#broader> <http://qudt.org/vocab/quantitykind/Temperature> ;
                           <https://w3id.org/h2v#appliesToSystem> <https://w3id.org/h2v#HydrogenStorage> .


###  https://w3id.org/h2v/property#MinimumWaterAcidity
:MinimumWaterAcidity rdf:type owl:NamedIndividual ,
                              <https://w3id.org/h2v#StaticProperty> ;
                     <http://qudt.org/schema/qudt/applicableUnit> <http://qudt.org/vocab/unit/PH> ;
                     rdfs:comment "The Minimum Water Acidity [ph] of the electrolyzer of the HV is the minimum level of acidity of the water allowed in the electrolyzer"^^rdfs:Literal ;
                     rdfs:label "Minimum Water Acidity"^^rdfs:Literal ;
                     <http://www.w3.org/2004/02/skos/core#broader> <http://qudt.org/vocab/quantitykind/Acidity> ;
                     <https://w3id.org/h2v#appliesToSystem> <https://w3id.org/h2v#Electrolyzer> .


###  https://w3id.org/h2v/property#MinimumWaterConductivity
:MinimumWaterConductivity rdf:type owl:NamedIndividual ,
                                   <https://w3id.org/h2v#StaticProperty> ;
                          <http://qudt.org/schema/qudt/applicableUnit> <http://qudt.org/vocab/unit/MicroS-PER-CentiM> ;
                          rdfs:comment "The Minimum Water Conductivity [µS/cm] of the electrolyzer of the HV is the minimum level of water conductivity acceptable. Conductivity measures the ability of water to conduct electricity, which depends on the presence of dissolved ions in water. High conductivity indicates the presence of ionic impurities, which can affect the efficiency of the electrolyzer and cause corrosion or other operational issues"^^rdfs:Literal ;
                          rdfs:label "Minimum Water Conductivity "^^rdfs:Literal ;
                          <http://www.w3.org/2004/02/skos/core#broader> <http://qudt.org/vocab/quantitykind/ElectrolyticConductivity> ;
                          <https://w3id.org/h2v#appliesToSystem> <https://w3id.org/h2v#Electrolyzer> .


###  https://w3id.org/h2v/property#MinimumWaterFlowRate
:MinimumWaterFlowRate rdf:type owl:NamedIndividual ,
                               <https://w3id.org/h2v#StaticProperty> ;
                      <http://qudt.org/schema/qudt/applicableUnit> <http://qudt.org/vocab/unit/KiloGM-PER-HR> ;
                      rdfs:comment "The Minimum Water Flow Rate [kg/h] of the electrolyzer of the HV is the minimum flow rate of distilled water available"^^rdfs:Literal ;
                      rdfs:label "Minimum Water Flow Rate"^^rdfs:Literal ;
                      <http://www.w3.org/2004/02/skos/core#broader> <http://qudt.org/vocab/quantitykind/MassFlowRate> ;
                      <https://w3id.org/h2v#appliesToSystem> <https://w3id.org/h2v#Electrolyzer> .


###  https://w3id.org/h2v/property#MinimumWaterPH
:MinimumWaterPH rdf:type owl:NamedIndividual ,
                         <https://w3id.org/h2v#StaticProperty> ;
                <http://qudt.org/schema/qudt/applicableUnit> <http://qudt.org/vocab/unit/PH> ;
                rdfs:comment "The Minimum Water PH [ph] of the electrolyzer of the HV is the minimum level acceptable of the acidity or basicity of distilled water. The pH can affect the solubility of various compounds and the formation of scale"^^rdfs:Literal ;
                rdfs:label "Minimum Water PH"^^rdfs:Literal ;
                <http://www.w3.org/2004/02/skos/core#broader> <http://qudt.org/vocab/quantitykind/Acidity> ;
                <https://w3id.org/h2v#appliesToSystem> <https://w3id.org/h2v#Electrolyzer> .


###  https://w3id.org/h2v/property#MinimumWaterTemperature
:MinimumWaterTemperature rdf:type owl:NamedIndividual ,
                                  <https://w3id.org/h2v#StaticProperty> ;
                         <http://qudt.org/schema/qudt/applicableUnit> <http://qudt.org/vocab/unit/DEG_C> ;
                         rdfs:comment "The Minimum Water Temperature [°C] of the electrolyzer of the HV is the lowest water temperature allowed of the electrolyzer"^^rdfs:Literal ;
                         rdfs:label "Minimum Water Temperature"^^rdfs:Literal ;
                         <http://www.w3.org/2004/02/skos/core#broader> <http://qudt.org/vocab/quantitykind/Temperature> ;
                         <https://w3id.org/h2v#appliesToSystem> <https://w3id.org/h2v#Electrolyzer> .


###  https://w3id.org/h2v/property#MinimumWobbeIndexToleratedH2
:MinimumWobbeIndexToleratedH2 rdf:type owl:NamedIndividual ,
                                       <https://w3id.org/h2v#StaticProperty> ;
                              <http://qudt.org/schema/qudt/applicableUnit> <http://qudt.org/vocab/unit/MegaJ-PER-M3> ;
                              rdfs:comment "The Minimum Wobbe Index Tolerated H2 [MJ/m^3] is the ratio of HHV to the square root of the relative density of the fuel with respect to air. It gives information on the compatibility of a fuel with the gas network"^^rdfs:Literal ;
                              rdfs:label "Minimum Wobbe Index Tolerated H2"^^rdfs:Literal ;
                              <http://www.w3.org/2004/02/skos/core#broader> <http://qudt.org/vocab/quantitykind/EnergyDensity> ;
                              <https://w3id.org/h2v#appliesToSystem> <https://w3id.org/h2v#Blender> .


###  https://w3id.org/h2v/property#ModuleTemperature
:ModuleTemperature rdf:type owl:NamedIndividual ,
                            <https://w3id.org/h2v#DynamicProperty> ;
                   <http://qudt.org/schema/qudt/applicableUnit> <http://qudt.org/vocab/unit/DEG_C> ;
                   rdfs:comment "The Module Temperature [°C] of the PV system of the HV is the PV module temperature, used for efficiency calculation, dependent on wind and enviromental temperature.  It can be either actual (i.e., based on an observation) or forecasted (i.e., based on a forecast)."^^rdfs:Literal ;
                   rdfs:label "Module Temperature"^^rdfs:Literal ;
                   <http://www.w3.org/2004/02/skos/core#broader> <http://qudt.org/vocab/quantitykind/Temperature> ;
                   <https://w3id.org/h2v#appliesToSystem> <https://w3id.org/h2v#PVsystem> .


###  https://w3id.org/h2v/property#N2Set
:N2Set rdf:type owl:NamedIndividual ,
                <https://w3id.org/h2v#PropertySet> ;
       rdfs:label "N2 Set"^^rdfs:Literal ;
       <https://w3id.org/h2v#hasMaximumPropertyMember> :MaximumN2 ;
       <https://w3id.org/h2v#hasMinimumPropertyMember> :MinimumN2 ;
       <https://w3id.org/h2v#hasPropertyMember> :MaximumN2 ,
                                                :MinimumN2 .


###  https://w3id.org/h2v/property#NominalModuleTemperature
:NominalModuleTemperature rdf:type owl:NamedIndividual ,
                                   <https://w3id.org/h2v#StaticProperty> ;
                          <http://qudt.org/schema/qudt/applicableUnit> <http://qudt.org/vocab/unit/DEG_C> ;
                          rdfs:comment "The Nominal Module Temperature [°C] of the PV system of the HV is the nominal of module temperature related to global nominal efficiency"^^rdfs:Literal ;
                          rdfs:label "Nominal Module Temperature"^^rdfs:Literal ;
                          <http://www.w3.org/2004/02/skos/core#broader> <http://qudt.org/vocab/quantitykind/Temperature> ;
                          <https://w3id.org/h2v#appliesToSystem> <https://w3id.org/h2v#PVsystem> .


###  https://w3id.org/h2v/property#NominalPower
:NominalPower rdf:type owl:NamedIndividual ,
                       <https://w3id.org/h2v#StaticProperty> ;
              <http://qudt.org/schema/qudt/applicableUnit> <http://qudt.org/vocab/unit/KiloW> ;
              rdfs:comment "The Nominal Power [kW] of the PV system of the HV is the nominal power production"^^rdfs:Literal ;
              rdfs:label "Nominal Power"^^rdfs:Literal ;
              <http://www.w3.org/2004/02/skos/core#broader> <http://qudt.org/vocab/quantitykind/ElectricPower> ;
              <https://w3id.org/h2v#appliesToSystem> <https://w3id.org/h2v#PVsystem> .


###  https://w3id.org/h2v/property#NominalStorageLeakage
:NominalStorageLeakage rdf:type owl:NamedIndividual ,
                                <https://w3id.org/h2v#StaticProperty> ;
                       <http://qudt.org/schema/qudt/applicableUnit> <http://qudt.org/vocab/unit/PERCENT> ;
                       rdfs:comment "The Nominal Storage Leakage [%kg loss/day] of the storage of the HV is the daily hydrogen leakage through leakage and valves"^^rdfs:Literal ;
                       rdfs:label "Nominal Storage Leakage"^^rdfs:Literal ;
                       <http://www.w3.org/2004/02/skos/core#broader> <http://qudt.org/vocab/quantitykind/Ratio> ;
                       <https://w3id.org/h2v#appliesToSystem> <https://w3id.org/h2v#HydrogenStorage> .


###  https://w3id.org/h2v/property#NominalThermalPower
:NominalThermalPower rdf:type owl:NamedIndividual ,
                              <https://w3id.org/h2v#StaticProperty> ;
                     <http://qudt.org/schema/qudt/applicableUnit> <http://qudt.org/vocab/unit/KiloW> ;
                     rdfs:comment "The Nominal Thermal Power [kW] of the fuel cell of the HV is the output power of the fuel cell"^^rdfs:Literal ;
                     rdfs:label "Nominal Thermal Power"^^rdfs:Literal ;
                     <http://www.w3.org/2004/02/skos/core#broader> <http://qudt.org/vocab/quantitykind/ElectricPower> ;
                     <https://w3id.org/h2v#appliesToSystem> <https://w3id.org/h2v#FuelCell> .


###  https://w3id.org/h2v/property#O2Set
:O2Set rdf:type owl:NamedIndividual ,
                <https://w3id.org/h2v#PropertySet> ;
       rdfs:label "O2 Set"^^rdfs:Literal ;
       <https://w3id.org/h2v#hasMaximumPropertyMember> :MaximumO2 ;
       <https://w3id.org/h2v#hasMinimumPropertyMember> :MinimumO2 ;
       <https://w3id.org/h2v#hasPropertyMember> :MaximumO2 ,
                                                :MinimumO2 .


###  https://w3id.org/h2v/property#OptimalH2Pressure
:OptimalH2Pressure rdf:type owl:NamedIndividual ,
                            <https://w3id.org/h2v#StaticProperty> ;
                   <http://qudt.org/schema/qudt/applicableUnit> <https://w3id.org/h2v#BARG> ;
                   rdfs:comment "The Optimal H2 Pressure [barg] of the electrolyzer of the HV is the optimal pressure of the hydrogen stream allowed as output of the system"^^rdfs:Literal ;
                   rdfs:label "Optimal H2 Pressure"^^rdfs:Literal ;
                   <http://www.w3.org/2004/02/skos/core#broader> <http://qudt.org/vocab/quantitykind/GaugePressure> ;
                   <https://w3id.org/h2v#appliesToSystem> <https://w3id.org/h2v#Electrolyzer> .


###  https://w3id.org/h2v/property#OptimalInletWaterPressure
:OptimalInletWaterPressure rdf:type owl:NamedIndividual ,
                                    <https://w3id.org/h2v#StaticProperty> ;
                           <http://qudt.org/schema/qudt/applicableUnit> <https://w3id.org/h2v#BARG> ;
                           rdfs:comment "The Optimal Inlet Water Pressure [barg] of the electrolyzer of the HV  is the optimal amount of water pressure allowed by the electrolyzer"^^rdfs:Literal ;
                           rdfs:label "Optimal Inlet Water Pressure"^^rdfs:Literal ;
                           <http://www.w3.org/2004/02/skos/core#broader> <http://qudt.org/vocab/quantitykind/GaugePressure> ;
                           <https://w3id.org/h2v#appliesToSystem> <https://w3id.org/h2v#Electrolyzer> .


###  https://w3id.org/h2v/property#OptimalPowerConsumption
:OptimalPowerConsumption rdf:type owl:NamedIndividual ,
                                  <https://w3id.org/h2v#StaticProperty> ;
                         <http://qudt.org/schema/qudt/applicableUnit> <http://qudt.org/vocab/unit/KiloW> ;
                         rdfs:comment "The Optimal Power Consumption [KW] of the electrolyzer of the HV is the optimal working input power of the electrolyzer"^^rdfs:Literal ;
                         rdfs:label "Optimal Power Consumption"^^rdfs:Literal ;
                         <http://www.w3.org/2004/02/skos/core#broader> <http://qudt.org/vocab/quantitykind/ElectricPower> ;
                         <https://w3id.org/h2v#appliesToSystem> <https://w3id.org/h2v#Electrolyzer> .


###  https://w3id.org/h2v/property#OptimalStorageSize
:OptimalStorageSize rdf:type owl:NamedIndividual ,
                             <https://w3id.org/h2v#StaticProperty> ;
                    <http://qudt.org/schema/qudt/applicableUnit> <http://qudt.org/vocab/unit/L> ;
                    rdfs:comment "The Optimal Storage Size [liter] of the storage of the HV is the optimal quantity of hydrogen that can be contained in storage"^^rdfs:Literal ;
                    rdfs:label "Optimal Storage Size"^^rdfs:Literal ;
                    <http://www.w3.org/2004/02/skos/core#broader> <http://qudt.org/vocab/quantitykind/LiquidVolume> ;
                    <https://w3id.org/h2v#appliesToSystem> <https://w3id.org/h2v#HydrogenStorage> .


###  https://w3id.org/h2v/property#OutletGasFlow
:OutletGasFlow rdf:type owl:NamedIndividual ,
                        <https://w3id.org/h2v#DynamicProperty> ;
               <http://qudt.org/schema/qudt/applicableUnit> <http://qudt.org/vocab/unit/SCM-PER-HR> ;
               rdfs:comment "The Outlet Gas Flow [Nm3/h] of the blender of the HV is the value of blended gas in output of the blender"^^rdfs:Literal ;
               rdfs:label "Outlet Gas Flow"^^rdfs:Literal ;
               <http://www.w3.org/2004/02/skos/core#broader> <http://qudt.org/vocab/quantitykind/MolarFlowRate> ;
               <https://w3id.org/h2v#appliesToSystem> <https://w3id.org/h2v#Blender> .


###  https://w3id.org/h2v/property#OutletGasFlowSet
:OutletGasFlowSet rdf:type owl:NamedIndividual ,
                           <https://w3id.org/h2v#PropertySet> ;
                  rdfs:label "Outlet Gas Flow Set"^^rdfs:Literal ;
                  <https://w3id.org/h2v#hasMaximumPropertyMember> :MaximumOutletGasFlow ;
                  <https://w3id.org/h2v#hasMinimumPropertyMember> :MinimumOutletGasFlow ;
                  <https://w3id.org/h2v#hasPropertyMember> :MaximumOutletGasFlow ,
                                                           :MinimumOutletGasFlow .


###  https://w3id.org/h2v/property#OutputH2Pressure
:OutputH2Pressure rdf:type owl:NamedIndividual ,
                           <https://w3id.org/h2v#DynamicProperty> ;
                  <http://qudt.org/schema/qudt/applicableUnit> <https://w3id.org/h2v#BARG> ;
                  rdfs:comment "The Output H2 Pressure [barg] of the electrolyzer of the HV is the measured H2 pressure to be compared with the allowed range"^^rdfs:Literal ;
                  rdfs:label "Output H2 Pressure"^^rdfs:Literal ;
                  <http://www.w3.org/2004/02/skos/core#broader> <http://qudt.org/vocab/quantitykind/GaugePressure> ;
                  <https://w3id.org/h2v#appliesToSystem> <https://w3id.org/h2v#Electrolyzer> .


###  https://w3id.org/h2v/property#OutputH2Temperature
:OutputH2Temperature rdf:type owl:NamedIndividual ,
                              <https://w3id.org/h2v#DynamicProperty> ;
                     <http://qudt.org/schema/qudt/applicableUnit> <http://qudt.org/vocab/unit/DEG_C> ;
                     rdfs:comment "The Output H2 Temperature [°C] of the electrolyzer of the HV is the measured H2 temperature to be compared with the allowed range"^^rdfs:Literal ;
                     rdfs:label "Output H2 Temperature"^^rdfs:Literal ;
                     <http://www.w3.org/2004/02/skos/core#broader> <http://qudt.org/vocab/quantitykind/Temperature> ;
                     <https://w3id.org/h2v#appliesToSystem> <https://w3id.org/h2v#Electrolyzer> .


###  https://w3id.org/h2v/property#OutputHydrogenPurity
:OutputHydrogenPurity rdf:type owl:NamedIndividual ,
                               <https://w3id.org/h2v#DynamicProperty> ;
                      <http://qudt.org/schema/qudt/applicableUnit> <http://qudt.org/vocab/unit/PERCENT> ;
                      rdfs:comment "The Output Hydrogen Purity [%] is the percentage of hydrogen in volume with respect to the total volume of output gas from the electrolyzer"^^rdfs:Literal ;
                      rdfs:label "Output Hydrogen Purity "^^rdfs:Literal ;
                      <http://www.w3.org/2004/02/skos/core#broader> <http://qudt.org/vocab/quantitykind/DimensionlessRatio> ;
                      <https://w3id.org/h2v#appliesToSystem> <https://w3id.org/h2v#Electrolyzer> .


###  https://w3id.org/h2v/property#OutputMassFlow
:OutputMassFlow rdf:type owl:NamedIndividual ,
                         <https://w3id.org/h2v#DynamicProperty> ;
                <http://qudt.org/schema/qudt/applicableUnit> <http://qudt.org/vocab/unit/KiloGM-PER-HR> ;
                rdfs:comment "The Output Mass Flow [kg/h] of the storage of the HV is the hydrogen flow output at storage"^^rdfs:Literal ;
                rdfs:label "Output Mass Flow"^^rdfs:Literal ;
                <http://www.w3.org/2004/02/skos/core#broader> <http://qudt.org/vocab/quantitykind/MassFlowRate> ;
                <https://w3id.org/h2v#appliesToSystem> <https://w3id.org/h2v#HydrogenStorage> .


###  https://w3id.org/h2v/property#PVSystemEnvironmentalTemperatureSet
:PVSystemEnvironmentalTemperatureSet rdf:type owl:NamedIndividual ,
                                              <https://w3id.org/h2v#PropertySet> ;
                                     rdfs:label "PV System Environmental Temperature Set"^^rdfs:Literal ;
                                     <https://w3id.org/h2v#hasMaximumPropertyMember> :PVSystemMaximumEnvironmentalTemperature ;
                                     <https://w3id.org/h2v#hasMinimumPropertyMember> :PVSystemMinimumEnvironmentalTemperature ;
                                     <https://w3id.org/h2v#hasPropertyMember> :PVSystemMaximumEnvironmentalTemperature ,
                                                                              :PVSystemMinimumEnvironmentalTemperature .


###  https://w3id.org/h2v/property#PVSystemEnvironmentalWindSpeedSet
:PVSystemEnvironmentalWindSpeedSet rdf:type owl:NamedIndividual ,
                                            <https://w3id.org/h2v#PropertySet> ;
                                   rdfs:label "PV System Environmental Wind Speed Set"^^rdfs:Literal ;
                                   <https://w3id.org/h2v#hasMaximumPropertyMember> :PVSystemMaximumEnvironmentalWindSpeed ;
                                   <https://w3id.org/h2v#hasPropertyMember> :PVSystemMaximumEnvironmentalWindSpeed .


###  https://w3id.org/h2v/property#PVSystemEnvironmentalWindspeedSet
:PVSystemEnvironmentalWindspeedSet rdf:type owl:NamedIndividual ,
                                            <https://w3id.org/h2v#PropertySet> ;
                                   rdfs:label "PV System Environmental Wind speed Set"^^rdfs:Literal ;
                                   <https://w3id.org/h2v#hasMinimumPropertyMember> :PVSystemMinimumEnvironmentalWindspeed ;
                                   <https://w3id.org/h2v#hasPropertyMember> :PVSystemMinimumEnvironmentalWindspeed .


###  https://w3id.org/h2v/property#PVSystemGlobalEfficiency
:PVSystemGlobalEfficiency rdf:type owl:NamedIndividual ,
                                   <https://w3id.org/h2v#DynamicProperty> ;
                          <http://qudt.org/schema/qudt/applicableUnit> <http://qudt.org/vocab/unit/ONE-PER-ONE> ;
                          rdfs:comment "The PV System Global Efficiency [-] of the PV system of the HV is the overall system's energy conversion efficiency calculated based on the inputs and outputs under real operating conditions. It can be either actual (i.e., based on an observation) or forecasted (i.e., based on a forecast)."^^rdfs:Literal ;
                          rdfs:label "PV System Global Efficiency"^^rdfs:Literal ;
                          <http://www.w3.org/2004/02/skos/core#broader> <http://qudt.org/vocab/quantitykind/Efficiency> ;
                          <https://w3id.org/h2v#appliesToSystem> <https://w3id.org/h2v#PVsystem> .


###  https://w3id.org/h2v/property#PVSystemMaximumEnvironmentalTemperature
:PVSystemMaximumEnvironmentalTemperature rdf:type owl:NamedIndividual ,
                                                  <https://w3id.org/h2v#StaticProperty> ;
                                         <http://qudt.org/schema/qudt/applicableUnit> <http://qudt.org/vocab/unit/DEG_C> ;
                                         rdfs:comment "The PV System Maximum Environmental Temperature [°C] of the PV system of the HV is the maximum enviromental temperature which guarantees the good performance of the PV plant"^^rdfs:Literal ;
                                         rdfs:label "PV System Maximum Environmental Temperature"^^rdfs:Literal ;
                                         <http://www.w3.org/2004/02/skos/core#broader> <http://qudt.org/vocab/quantitykind/Temperature> ;
                                         <https://w3id.org/h2v#appliesToSystem> <https://w3id.org/h2v#PVsystem> .


###  https://w3id.org/h2v/property#PVSystemMaximumEnvironmentalWindSpeed
:PVSystemMaximumEnvironmentalWindSpeed rdf:type owl:NamedIndividual ,
                                                <https://w3id.org/h2v#StaticProperty> ;
                                       <http://qudt.org/schema/qudt/applicableUnit> <http://qudt.org/vocab/unit/M-PER-SEC> ;
                                       rdfs:comment "The PV System Maximum Environmental Wind Speed [m/s] of the PV system of the HV is the maximum wind speed which guarantees the good performance of the PV plant"^^rdfs:Literal ;
                                       rdfs:label "PV System Maximum Environmental Wind Speed"^^rdfs:Literal ;
                                       <http://www.w3.org/2004/02/skos/core#broader> <http://qudt.org/vocab/quantitykind/Speed> ;
                                       <https://w3id.org/h2v#appliesToSystem> <https://w3id.org/h2v#PVsystem> .


###  https://w3id.org/h2v/property#PVSystemMinimumEnvironmentalTemperature
:PVSystemMinimumEnvironmentalTemperature rdf:type owl:NamedIndividual ,
                                                  <https://w3id.org/h2v#StaticProperty> ;
                                         <http://qudt.org/schema/qudt/applicableUnit> <http://qudt.org/vocab/unit/DEG_C> ;
                                         rdfs:comment "The PV System Minimum Environmental Temperature [°C] of the PV system of the HV is the minimum enviromental temperature which guarantees the good performance of the PV plant"^^rdfs:Literal ;
                                         rdfs:label "PV System Minimum Environmental Temperature"^^rdfs:Literal ;
                                         <http://www.w3.org/2004/02/skos/core#broader> <http://qudt.org/vocab/quantitykind/Temperature> ;
                                         <https://w3id.org/h2v#appliesToSystem> <https://w3id.org/h2v#PVsystem> .


###  https://w3id.org/h2v/property#PVSystemMinimumEnvironmentalWindspeed
:PVSystemMinimumEnvironmentalWindspeed rdf:type owl:NamedIndividual ,
                                                <https://w3id.org/h2v#StaticProperty> ;
                                       <http://qudt.org/schema/qudt/applicableUnit> <http://qudt.org/vocab/unit/M-PER-SEC> ;
                                       rdfs:comment "The PV System Minimum Environmental Wind Speed [m/s] of the PV system of the HV is the minimum wind speed which guarantees the good performance of the PV plant"^^rdfs:Literal ;
                                       rdfs:label "PV System Minimum Environmental Wind speed"^^rdfs:Literal ;
                                       <http://www.w3.org/2004/02/skos/core#broader> <http://qudt.org/vocab/quantitykind/Speed> ;
                                       <https://w3id.org/h2v#appliesToSystem> <https://w3id.org/h2v#PVsystem> .


###  https://w3id.org/h2v/property#PVSystemNominalGlobalEfficiency
:PVSystemNominalGlobalEfficiency rdf:type owl:NamedIndividual ,
                                          <https://w3id.org/h2v#StaticProperty> ;
                                 <http://qudt.org/schema/qudt/applicableUnit> <http://qudt.org/vocab/unit/ONE-PER-ONE> ;
                                 rdfs:comment "The PV System Nominal Global Efficiency [-] of the PV system of the HV is the overall efficiency of an entire system, calculated under specified standard conditions, and expressed as a dimensionless ratio or percentage. It represents the system's rated performance in converting initial energy input into final useful output"^^rdfs:Literal ;
                                 rdfs:label "PV System Nominal Global Efficiency"^^rdfs:Literal ;
                                 <http://www.w3.org/2004/02/skos/core#broader> <http://qudt.org/vocab/quantitykind/Efficiency> ;
                                 <https://w3id.org/h2v#appliesToSystem> <https://w3id.org/h2v#PVsystem> .


###  https://w3id.org/h2v/property#PipePressureSet
:PipePressureSet rdf:type owl:NamedIndividual ,
                          <https://w3id.org/h2v#PropertySet> ;
                 rdfs:label "Pipe Pressure Set"^^rdfs:Literal ;
                 <https://w3id.org/h2v#hasMaximumPropertyMember> :MaximumPipePressure ;
                 <https://w3id.org/h2v#hasMinimumPropertyMember> :MinimumPipePressure ;
                 <https://w3id.org/h2v#hasPropertyMember> :MaximumPipePressure ,
                                                          :MinimumPipePressure .


###  https://w3id.org/h2v/property#PipesActualH2O
:PipesActualH2O rdf:type owl:NamedIndividual ,
                         <https://w3id.org/h2v#DynamicProperty> ;
                <http://qudt.org/schema/qudt/applicableUnit> <http://qudt.org/vocab/unit/PPM> ;
                rdfs:comment "The Pipes Actual H2O [ppm] is the actual amount of water vapor in the hydrogen gas across the pipe of the HV"^^rdfs:Literal ;
                rdfs:label "Pipes Actual H2O"^^rdfs:Literal ;
                <http://www.w3.org/2004/02/skos/core#broader> <http://qudt.org/vocab/quantitykind/DimensionlessRatio> ;
                <https://w3id.org/h2v#appliesToSystem> <https://w3id.org/h2v#Pipe> .


###  https://w3id.org/h2v/property#PipesActualN2
:PipesActualN2 rdf:type owl:NamedIndividual ,
                        <https://w3id.org/h2v#DynamicProperty> ;
               <http://qudt.org/schema/qudt/applicableUnit> <http://qudt.org/vocab/unit/PPM> ;
               rdfs:comment "The Pipes Actual N2 [ppm] is the actual amount of nitrogen in the hydrogen gas across the pipe of the HV"^^rdfs:Literal ;
               rdfs:label "Pipes Actual N2"^^rdfs:Literal ;
               <http://www.w3.org/2004/02/skos/core#broader> <http://qudt.org/vocab/quantitykind/DimensionlessRatio> ;
               <https://w3id.org/h2v#appliesToSystem> <https://w3id.org/h2v#Pipe> .


###  https://w3id.org/h2v/property#PipesActualO2
:PipesActualO2 rdf:type owl:NamedIndividual ,
                        <https://w3id.org/h2v#DynamicProperty> ;
               <http://qudt.org/schema/qudt/applicableUnit> <http://qudt.org/vocab/unit/PPM> ;
               rdfs:comment "The Pipes Actual O2 [ppm] is the actual amount of oxigen in the hydrogen gas across the pipe of the HV"^^rdfs:Literal ;
               rdfs:label "Pipes Actual O2"^^rdfs:Literal ;
               <http://www.w3.org/2004/02/skos/core#broader> <http://qudt.org/vocab/quantitykind/DimensionlessRatio> ;
               <https://w3id.org/h2v#appliesToSystem> <https://w3id.org/h2v#Pipe> .


###  https://w3id.org/h2v/property#PipesChemicalComposition
:PipesChemicalComposition rdf:type owl:NamedIndividual ,
                                   <https://w3id.org/h2v#DynamicProperty> ;
                          <http://qudt.org/schema/qudt/applicableUnit> <http://qudt.org/vocab/unit/PPM> ;
                          rdfs:comment "The Pipes Chemical Composition [ppm] is the actual chemical composition of the hydrogen gas in the pipe (actual O2, actual H2O and actual N2), as measured at a certain time"^^rdfs:Literal ;
                          rdfs:label "Pipes Chemical Composition"^^rdfs:Literal ;
                          <http://www.w3.org/2004/02/skos/core#broader> <http://qudt.org/vocab/quantitykind/DimensionlessRatio> ;
                          <https://w3id.org/h2v#appliesToSystem> <https://w3id.org/h2v#Pipe> .


###  https://w3id.org/h2v/property#PipesMassFlow
:PipesMassFlow rdf:type owl:NamedIndividual ,
                        <https://w3id.org/h2v#DynamicProperty> ;
               <http://qudt.org/schema/qudt/applicableUnit> <http://qudt.org/vocab/unit/KiloGM-PER-HR> ;
               rdfs:comment "The Pipes Mass Flow [kgH2/h] is the actual hydrogen flow, as measured at a certain time"^^rdfs:Literal ;
               rdfs:label "Pipes Mass Flow"^^rdfs:Literal ;
               <http://www.w3.org/2004/02/skos/core#broader> <http://qudt.org/vocab/quantitykind/MassFlowRate> ;
               <https://w3id.org/h2v#appliesToSystem> <https://w3id.org/h2v#Pipe> .


###  https://w3id.org/h2v/property#PipesNominalChemicalCompositionTolerated
:PipesNominalChemicalCompositionTolerated rdf:type owl:NamedIndividual ,
                                                   <https://w3id.org/h2v#StaticProperty> ;
                                          <http://qudt.org/schema/qudt/applicableUnit> <http://qudt.org/vocab/unit/PPM> ;
                                          rdfs:comment "The Pipes Nominal Chemical Composition Tolerated [ppm] is the chemical composition of the gas acceptable in the pipe of the HV (Nominal O2, Nominal H2O, Nominal N2)"^^rdfs:Literal ;
                                          rdfs:label "Pipes Nominal Chemical Composition Tolerated"^^rdfs:Literal ;
                                          <http://www.w3.org/2004/02/skos/core#broader> <http://qudt.org/vocab/quantitykind/DimensionlessRatio> ;
                                          <https://w3id.org/h2v#appliesToSystem> <https://w3id.org/h2v#Pipe> .


###  https://w3id.org/h2v/property#PipesNominalH2OTolerated
:PipesNominalH2OTolerated rdf:type owl:NamedIndividual ,
                                   <https://w3id.org/h2v#StaticProperty> ;
                          <http://qudt.org/schema/qudt/applicableUnit> <http://qudt.org/vocab/unit/PPM> ;
                          rdfs:comment "The Pipes Nominal H2O Tolerated [ppm] is the amount of water vapor acceptable in the hydrogen gas across the pipe of the HV"^^rdfs:Literal ;
                          rdfs:label "Pipes Nominal H2O Tolerated"^^rdfs:Literal ;
                          <http://www.w3.org/2004/02/skos/core#broader> <http://qudt.org/vocab/quantitykind/DimensionlessRatio> ;
                          <https://w3id.org/h2v#appliesToSystem> <https://w3id.org/h2v#Pipe> .


###  https://w3id.org/h2v/property#PipesNominalN2Tolerated
:PipesNominalN2Tolerated rdf:type owl:NamedIndividual ,
                                  <https://w3id.org/h2v#StaticProperty> ;
                         <http://qudt.org/schema/qudt/applicableUnit> <http://qudt.org/vocab/unit/PPM> ;
                         rdfs:comment "The Pipes Nominal N2 Tolerated [ppm] is the amount of nitrogen acceptable in the hydrogen gas across the pipe of the HV"^^rdfs:Literal ;
                         rdfs:label "Pipes Nominal N2 Tolerated"^^rdfs:Literal ;
                         <http://www.w3.org/2004/02/skos/core#broader> <http://qudt.org/vocab/quantitykind/DimensionlessRatio> ;
                         <https://w3id.org/h2v#appliesToSystem> <https://w3id.org/h2v#Pipe> .


###  https://w3id.org/h2v/property#PipesNominalO2Tolerated
:PipesNominalO2Tolerated rdf:type owl:NamedIndividual ,
                                  <https://w3id.org/h2v#StaticProperty> ;
                         <http://qudt.org/schema/qudt/applicableUnit> <http://qudt.org/vocab/unit/PPM> ;
                         rdfs:comment "The Pipes Nominal O2 Tolerated [ppm] is the amount of oxigen acceptable in the hydrogen gas across the pipe of the HV"^^rdfs:Literal ;
                         rdfs:label "Pipes Nominal O2 Tolerated"^^rdfs:Literal ;
                         <http://www.w3.org/2004/02/skos/core#broader> <http://qudt.org/vocab/quantitykind/DimensionlessRatio> ;
                         <https://w3id.org/h2v#appliesToSystem> <https://w3id.org/h2v#Pipe> .


###  https://w3id.org/h2v/property#PipesPressure
:PipesPressure rdf:type owl:NamedIndividual ,
                        <https://w3id.org/h2v#DynamicProperty> ;
               <http://qudt.org/schema/qudt/applicableUnit> <http://qudt.org/vocab/unit/BAR> ;
               rdfs:comment "The Pipes Pressure [bar] is the actual pressure of hydrogen, as measured at a certain time"^^rdfs:Literal ;
               rdfs:label "Pipes Pressure"^^rdfs:Literal ;
               <http://www.w3.org/2004/02/skos/core#broader> <http://qudt.org/vocab/quantitykind/Pressure> ;
               <https://w3id.org/h2v#appliesToSystem> <https://w3id.org/h2v#Pipe> .


###  https://w3id.org/h2v/property#PlaneOfArrayIrradiancePOA
:PlaneOfArrayIrradiancePOA rdf:type owl:NamedIndividual ,
                                    <https://w3id.org/h2v#DynamicProperty> ;
                           <http://qudt.org/schema/qudt/applicableUnit> <http://qudt.org/vocab/unit/KiloW-HR-PER-M2> ;
                           rdfs:comment "The Plane Of Array Irradiance POA [kWh/m^2] is the usable solar energy expected to reach the PV panels (per square meter of useful surface) over a certain time period. It is the GHI and its component (direct, diffusive and albedo) adjusted by each possible losses such as incindence angle, shading, soiling, etc. It can be either actual (i.e., based on an observation) or forecasted (i.e., based on a forecast)."^^rdfs:Literal ;
                           rdfs:label "Plane Of Array Irradiance POA"^^rdfs:Literal ;
                           <http://www.w3.org/2004/02/skos/core#broader> <http://qudt.org/vocab/quantitykind/EnergyPerArea> ;
                           <https://w3id.org/h2v#appliesToSystem> <https://w3id.org/h2v#PVsystem> .


###  https://w3id.org/h2v/property#PowerConsumption
:PowerConsumption rdf:type owl:NamedIndividual ,
                           <https://w3id.org/h2v#DynamicProperty> ;
                  <http://qudt.org/schema/qudt/applicableUnit> <http://qudt.org/vocab/unit/KiloW> ;
                  rdfs:comment "The Power Consumption [kW] is the power consumption of the electrolyzer"^^rdfs:Literal ;
                  rdfs:label "Power Consumption"^^rdfs:Literal ;
                  <http://www.w3.org/2004/02/skos/core#broader> <http://qudt.org/vocab/quantitykind/ElectricPower> ;
                  <https://w3id.org/h2v#appliesToSystem> <https://w3id.org/h2v#Electrolyzer> .


###  https://w3id.org/h2v/property#PowerProduction
:PowerProduction rdf:type owl:NamedIndividual ,
                          <https://w3id.org/h2v#DynamicProperty> ;
                 <http://qudt.org/schema/qudt/applicableUnit> <http://qudt.org/vocab/unit/KiloW> ;
                 rdfs:comment "The Power Production [kW] of the PV system of the HV is the average power output. It can be either actual (i.e., based on an observation) by using actual performance data, or forecasted (i.e., based on a forecast)."^^rdfs:Literal ;
                 rdfs:label "Power Production"^^rdfs:Literal ;
                 <http://www.w3.org/2004/02/skos/core#broader> <http://qudt.org/vocab/quantitykind/ElectricPower> ;
                 <https://w3id.org/h2v#appliesToSystem> <https://w3id.org/h2v#PVsystem> .


###  https://w3id.org/h2v/property#PressureControlValveInletPressure
:PressureControlValveInletPressure rdf:type owl:NamedIndividual ,
                                            <https://w3id.org/h2v#DynamicProperty> ;
                                   <http://qudt.org/schema/qudt/applicableUnit> <https://w3id.org/h2v#BARG> ;
                                   rdfs:comment "The Pressure Control Valve Inlet Pressure [barg] of the pressure control valve of the HV is the measured inlet pressure"^^rdfs:Literal ;
                                   rdfs:label "Pressure Control Valve Inlet Pressure"^^rdfs:Literal ;
                                   <http://www.w3.org/2004/02/skos/core#broader> <http://qudt.org/vocab/quantitykind/GaugePressure> ;
                                   <https://w3id.org/h2v#appliesToSystem> <https://w3id.org/h2v#PressureControlValve> .


###  https://w3id.org/h2v/property#PressureControlValveInletPressureSet
:PressureControlValveInletPressureSet rdf:type owl:NamedIndividual ,
                                               <https://w3id.org/h2v#PropertySet> ;
                                      rdfs:label "Pressure Control Valve Inlet Pressure Set"^^rdfs:Literal ;
                                      <https://w3id.org/h2v#hasMaximumPropertyMember> :PressureControlValveMaximumInletNominalPressure ;
                                      <https://w3id.org/h2v#hasMinimumPropertyMember> :PressureControlValveMinimumInletNominalPressure ;
                                      <https://w3id.org/h2v#hasPropertyMember> :PressureControlValveMaximumInletNominalPressure ,
                                                                               :PressureControlValveMinimumInletNominalPressure .


###  https://w3id.org/h2v/property#PressureControlValveMaximumInletNominalPressure
:PressureControlValveMaximumInletNominalPressure rdf:type owl:NamedIndividual ,
                                                          <https://w3id.org/h2v#StaticProperty> ;
                                                 <http://qudt.org/schema/qudt/applicableUnit> <https://w3id.org/h2v#BARG> ;
                                                 rdfs:comment "The Pressure Control Valve Maximum Inlet Nominal Pressure [barg] of the pressure control valve of the HV is the maximum inlet pressure based on how the valve has been designed"^^rdfs:Literal ;
                                                 rdfs:label "Pressure Control Valve Maximum Inlet Nominal Pressure"^^rdfs:Literal ;
                                                 <http://www.w3.org/2004/02/skos/core#broader> <http://qudt.org/vocab/quantitykind/GaugePressure> ;
                                                 <https://w3id.org/h2v#appliesToSystem> <https://w3id.org/h2v#PressureControlValve> .


###  https://w3id.org/h2v/property#PressureControlValveMaximumOutletNominalPressure
:PressureControlValveMaximumOutletNominalPressure rdf:type owl:NamedIndividual ,
                                                           <https://w3id.org/h2v#StaticProperty> ;
                                                  <http://qudt.org/schema/qudt/applicableUnit> <https://w3id.org/h2v#BARG> ;
                                                  rdfs:comment "The Pressure Control Valve Maximum Outlet Nominal Pressure [barg] of the pressure control valve of the HV is the maximum outlet pressure based on how the valve has been designed"^^rdfs:Literal ;
                                                  rdfs:label "Pressure Control Valve Maximum Outlet Nominal Pressure"^^rdfs:Literal ;
                                                  <http://www.w3.org/2004/02/skos/core#broader> <http://qudt.org/vocab/quantitykind/GaugePressure> ;
                                                  <https://w3id.org/h2v#appliesToSystem> <https://w3id.org/h2v#PressureControlValve> .


###  https://w3id.org/h2v/property#PressureControlValveMinimumInletNominalPressure
:PressureControlValveMinimumInletNominalPressure rdf:type owl:NamedIndividual ,
                                                          <https://w3id.org/h2v#StaticProperty> ;
                                                 <http://qudt.org/schema/qudt/applicableUnit> <https://w3id.org/h2v#BARG> ;
                                                 rdfs:comment "The Pressure Control Valve Minimum Inlet Nominal Pressure [barg] of the pressure control valve of the HV is the minimum inlet pressure based on how the valve has been designed"^^rdfs:Literal ;
                                                 rdfs:label "Pressure Control Valve Minimum Inlet Nominal Pressure"^^rdfs:Literal ;
                                                 <http://www.w3.org/2004/02/skos/core#broader> <http://qudt.org/vocab/quantitykind/GaugePressure> ;
                                                 <https://w3id.org/h2v#appliesToSystem> <https://w3id.org/h2v#PressureControlValve> .


###  https://w3id.org/h2v/property#PressureControlValveMinimumOutletNominalPressure
:PressureControlValveMinimumOutletNominalPressure rdf:type owl:NamedIndividual ,
                                                           <https://w3id.org/h2v#StaticProperty> ;
                                                  <http://qudt.org/schema/qudt/applicableUnit> <https://w3id.org/h2v#BARG> ;
                                                  rdfs:comment "The Pressure Control Valve Minimum  Outlet Nominal Pressure [barg] of the pressure control valve of the HV is the minimum outlet pressure based on how the valve has been designed"^^rdfs:Literal ;
                                                  rdfs:label "Pressure Control Valve Minimum  Outlet Nominal Pressure"^^rdfs:Literal ;
                                                  <http://www.w3.org/2004/02/skos/core#broader> <http://qudt.org/vocab/quantitykind/GaugePressure> ;
                                                  <https://w3id.org/h2v#appliesToSystem> <https://w3id.org/h2v#PressureControlValve> .


###  https://w3id.org/h2v/property#PressureControlValveOutletPressure
:PressureControlValveOutletPressure rdf:type owl:NamedIndividual ,
                                             <https://w3id.org/h2v#DynamicProperty> ;
                                    <http://qudt.org/schema/qudt/applicableUnit> <https://w3id.org/h2v#BARG> ;
                                    rdfs:comment "The Pressure Control Valve Outlet Pressure [barg] of the pressure control valve of the HV is the measured outlet pressure"^^rdfs:Literal ;
                                    rdfs:label "Pressure Control Valve Outlet Pressure "^^rdfs:Literal ;
                                    <http://www.w3.org/2004/02/skos/core#broader> <http://qudt.org/vocab/quantitykind/GaugePressure> ;
                                    <https://w3id.org/h2v#appliesToSystem> <https://w3id.org/h2v#PressureControlValve> .


###  https://w3id.org/h2v/property#PressureControlValveOutletPressureSet
:PressureControlValveOutletPressureSet rdf:type owl:NamedIndividual ,
                                                <https://w3id.org/h2v#PropertySet> ;
                                       rdfs:label "Pressure Control Valve Outlet Pressure Set"^^rdfs:Literal ;
                                       <https://w3id.org/h2v#hasMaximumPropertyMember> :PressureControlValveMaximumOutletNominalPressure ;
                                       <https://w3id.org/h2v#hasMinimumPropertyMember> :PressureControlValveMinimumOutletNominalPressure ;
                                       <https://w3id.org/h2v#hasPropertyMember> :PressureControlValveMaximumOutletNominalPressure ,
                                                                                :PressureControlValveMinimumOutletNominalPressure .


###  https://w3id.org/h2v/property#RatioH2
:RatioH2 rdf:type owl:NamedIndividual ,
                  <https://w3id.org/h2v#DynamicProperty> ;
         <http://qudt.org/schema/qudt/applicableUnit> <http://qudt.org/vocab/unit/ONE-PER-ONE> ;
         rdfs:comment "The Ratio H2 [kg H2/kg water] of the electrolyzer of the HV is the hydrogen production relative to the consumption of distilled water"^^rdfs:Literal ;
         rdfs:label "Ratio H2"^^rdfs:Literal ;
         <http://www.w3.org/2004/02/skos/core#broader> <http://qudt.org/vocab/quantitykind/VolumeFlowRatio> ;
         <https://w3id.org/h2v#appliesToSystem> <https://w3id.org/h2v#Electrolyzer> .


###  https://w3id.org/h2v/property#StoragePressure
:StoragePressure rdf:type owl:NamedIndividual ,
                          <https://w3id.org/h2v#DynamicProperty> ;
                 <http://qudt.org/schema/qudt/applicableUnit> <https://w3id.org/h2v#BARG> ;
                 rdfs:comment "The Storage Pressure [barg] of the storage of the HV is the hydrogen pressure inside the storage unit"^^rdfs:Literal ;
                 rdfs:label "Storage Pressure"^^rdfs:Literal ;
                 <http://www.w3.org/2004/02/skos/core#broader> <http://qudt.org/vocab/quantitykind/GaugePressure> ;
                 <https://w3id.org/h2v#appliesToSystem> <https://w3id.org/h2v#HydrogenStorage> .


###  https://w3id.org/h2v/property#StoragePressureSet
:StoragePressureSet rdf:type owl:NamedIndividual ,
                             <https://w3id.org/h2v#PropertySet> ;
                    rdfs:label "Storage Pressure Set"^^rdfs:Literal ;
                    <https://w3id.org/h2v#hasMaximumPropertyMember> :MaximumStoragePressure ;
                    <https://w3id.org/h2v#hasMinimumPropertyMember> :MinimumStoragePressure ;
                    <https://w3id.org/h2v#hasPropertyMember> :MaximumStoragePressure ,
                                                             :MinimumStoragePressure .


###  https://w3id.org/h2v/property#StorageSizeSet
:StorageSizeSet rdf:type owl:NamedIndividual ,
                         <https://w3id.org/h2v#PropertySet> ;
                rdfs:label "Storage Size Set"^^rdfs:Literal ;
                <https://w3id.org/h2v#hasMaximumPropertyMember> :MaximumStorageSize ;
                <https://w3id.org/h2v#hasMinimumPropertyMember> :MinimumStorageSize ;
                <https://w3id.org/h2v#hasOptimalPropertyMember> :OptimalStorageSize ;
                <https://w3id.org/h2v#hasPropertyMember> :MaximumStorageSize ,
                                                         :MinimumStorageSize ,
                                                         :OptimalStorageSize .


###  https://w3id.org/h2v/property#StorageStateOfCharge
:StorageStateOfCharge rdf:type owl:NamedIndividual ,
                               <https://w3id.org/h2v#DynamicProperty> ;
                      <http://qudt.org/schema/qudt/applicableUnit> <http://qudt.org/vocab/unit/PERCENT> ;
                      rdfs:comment "The Storage State Of Charge  [%] of the Storage of the HV is the ratio between the amount of hydrogen stored at a certain time and the maximum amount of hydrogen allowed in storage"^^rdfs:Literal ;
                      rdfs:label "Storage State Of Charge"^^rdfs:Literal ;
                      <http://www.w3.org/2004/02/skos/core#broader> <http://qudt.org/vocab/quantitykind/DimensionlessRatio> ;
                      <https://w3id.org/h2v#appliesToSystem> <https://w3id.org/h2v#HydrogenStorage> .


###  https://w3id.org/h2v/property#StorageTemperature
:StorageTemperature rdf:type owl:NamedIndividual ,
                             <https://w3id.org/h2v#DynamicProperty> ;
                    <http://qudt.org/schema/qudt/applicableUnit> <http://qudt.org/vocab/unit/DEG_C> ;
                    rdfs:comment "The Storage Temperature [°C] of the storage of the HV is the hydrogen temperature inside the storage unit"^^rdfs:Literal ;
                    rdfs:label "Storage Temperature"^^rdfs:Literal ;
                    <http://www.w3.org/2004/02/skos/core#broader> <http://qudt.org/vocab/quantitykind/Temperature> ;
                    <https://w3id.org/h2v#appliesToSystem> <https://w3id.org/h2v#HydrogenStorage> .


###  https://w3id.org/h2v/property#StorageTemperatureSet
:StorageTemperatureSet rdf:type owl:NamedIndividual ,
                                <https://w3id.org/h2v#PropertySet> ;
                       rdfs:label "Storage Temperature Set"^^rdfs:Literal ;
                       <https://w3id.org/h2v#hasMaximumPropertyMember> :MaximumStorageTemperature ;
                       <https://w3id.org/h2v#hasMinimumPropertyMember> :MinimumStorageTemperature ;
                       <https://w3id.org/h2v#hasPropertyMember> :MaximumStorageTemperature ,
                                                                :MinimumStorageTemperature .


###  https://w3id.org/h2v/property#StoredWater
:StoredWater rdf:type owl:NamedIndividual ,
                      <https://w3id.org/h2v#DynamicProperty> ;
             <http://qudt.org/schema/qudt/applicableUnit> <http://qudt.org/vocab/unit/L> ;
             rdfs:comment "The Stored Water [liter] is the amout of water currently stored in the water tank"^^rdfs:Literal ;
             rdfs:label "Stored Water"^^rdfs:Literal ;
             <http://www.w3.org/2004/02/skos/core#broader> <http://qudt.org/vocab/quantitykind/LiquidVolume> ;
             <https://w3id.org/h2v#appliesToSystem> <https://w3id.org/h2v#WaterTank> .


###  https://w3id.org/h2v/property#SystemArea
:SystemArea rdf:type owl:NamedIndividual ,
                     <https://w3id.org/h2v#StaticProperty> ;
            <http://qudt.org/schema/qudt/applicableUnit> <http://qudt.org/vocab/unit/M2> ;
            rdfs:comment "The System Area [m2] of the PV system of the HV is the useful surface for PV panels"^^rdfs:Literal ;
            rdfs:label "System Area"^^rdfs:Literal ;
            <http://www.w3.org/2004/02/skos/core#broader> <http://qudt.org/vocab/quantitykind/Area> ;
            <https://w3id.org/h2v#appliesToSystem> <https://w3id.org/h2v#PVsystem> .


###  https://w3id.org/h2v/property#SystemSpecificEnergy
:SystemSpecificEnergy rdf:type owl:NamedIndividual ,
                               <https://w3id.org/h2v#DynamicProperty> ;
                      <http://qudt.org/schema/qudt/applicableUnit> <http://qudt.org/vocab/unit/MegaJ-PER-KiloGM> ;
                      rdfs:comment "The System Specific Energy [MJ/kg] of the electrolyzer of the HV is the electric energy consumed for each kg of H2 produced, which depends on the operating conditions and the state of the components"^^rdfs:Literal ;
                      rdfs:label "System Specific Energy"^^rdfs:Literal ;
                      <http://www.w3.org/2004/02/skos/core#broader> <http://qudt.org/vocab/quantitykind/SpecificEnergy> ;
                      <https://w3id.org/h2v#appliesToSystem> <https://w3id.org/h2v#Electrolyzer> .


###  https://w3id.org/h2v/property#ThermalPower
:ThermalPower rdf:type owl:NamedIndividual ,
                       <https://w3id.org/h2v#DynamicProperty> ;
              <http://qudt.org/schema/qudt/applicableUnit> <http://qudt.org/vocab/unit/KiloW> ;
              rdfs:comment "The Thermal Power [kW] of the fuel cell of the HV is the output power of the fuel cell"^^rdfs:Literal ;
              rdfs:label "Thermal Power"^^rdfs:Literal ;
              <http://www.w3.org/2004/02/skos/core#broader> <http://qudt.org/vocab/quantitykind/ElectricPower> ;
              <https://w3id.org/h2v#appliesToSystem> <https://w3id.org/h2v#FuelCell> .


###  https://w3id.org/h2v/property#WaterAcidity
:WaterAcidity rdf:type owl:NamedIndividual ,
                       <https://w3id.org/h2v#DynamicProperty> ;
              <http://qudt.org/schema/qudt/applicableUnit> <http://qudt.org/vocab/unit/PH> ;
              rdfs:comment "The Water Acidity [ph] is the measured PH value of the water in the electrolyzer"^^rdfs:Literal ;
              rdfs:label "Water Acidity"^^rdfs:Literal ;
              <http://www.w3.org/2004/02/skos/core#broader> <http://qudt.org/vocab/quantitykind/Acidity> ;
              <https://w3id.org/h2v#appliesToSystem> <https://w3id.org/h2v#Electrolyzer> .


###  https://w3id.org/h2v/property#WaterAciditySet
:WaterAciditySet rdf:type owl:NamedIndividual ,
                          <https://w3id.org/h2v#PropertySet> ;
                 rdfs:label "Water Acidity Set"^^rdfs:Literal ;
                 <https://w3id.org/h2v#hasMaximumPropertyMember> :MaximumWaterAcidity ;
                 <https://w3id.org/h2v#hasMinimumPropertyMember> :MinimumWaterAcidity ;
                 <https://w3id.org/h2v#hasPropertyMember> :MaximumWaterAcidity ,
                                                          :MinimumWaterAcidity .


###  https://w3id.org/h2v/property#WaterConductivitySet
:WaterConductivitySet rdf:type owl:NamedIndividual ,
                               <https://w3id.org/h2v#PropertySet> ;
                      rdfs:label "Water Conductivity Set"^^rdfs:Literal ;
                      <https://w3id.org/h2v#hasMaximumPropertyMember> :MaximumWaterConductivity ;
                      <https://w3id.org/h2v#hasMinimumPropertyMember> :MinimumWaterConductivity ;
                      <https://w3id.org/h2v#hasPropertyMember> :MaximumWaterConductivity ,
                                                               :MinimumWaterConductivity .


###  https://w3id.org/h2v/property#WaterFlowRateSet
:WaterFlowRateSet rdf:type owl:NamedIndividual ,
                           <https://w3id.org/h2v#PropertySet> ;
                  rdfs:label "Water Flow Rate Set"^^rdfs:Literal ;
                  <https://w3id.org/h2v#hasMaximumPropertyMember> :MaximumWaterFlowRate ;
                  <https://w3id.org/h2v#hasMinimumPropertyMember> :MinimumWaterFlowRate ;
                  <https://w3id.org/h2v#hasPropertyMember> :MaximumWaterFlowRate ,
                                                           :MinimumWaterFlowRate .


###  https://w3id.org/h2v/property#WaterPHSet
:WaterPHSet rdf:type owl:NamedIndividual ,
                     <https://w3id.org/h2v#PropertySet> ;
            rdfs:label "Water PH Set"^^rdfs:Literal ;
            <https://w3id.org/h2v#hasMaximumPropertyMember> :MaximumWaterPH ;
            <https://w3id.org/h2v#hasMinimumPropertyMember> :MinimumWaterPH ;
            <https://w3id.org/h2v#hasPropertyMember> :MaximumWaterPH ,
                                                     :MinimumWaterPH .


###  https://w3id.org/h2v/property#WaterPumpInletPressure
:WaterPumpInletPressure rdf:type owl:NamedIndividual ,
                                 <https://w3id.org/h2v#DynamicProperty> ;
                        <http://qudt.org/schema/qudt/applicableUnit> <https://w3id.org/h2v#BARG> ;
                        rdfs:comment "The Water Pump Inlet Pressure [barg] of the water pump of the HV  is the measured inlet pressure of the water pump"^^rdfs:Literal ;
                        rdfs:label "Water Pump Inlet Pressure"^^rdfs:Literal ;
                        <http://www.w3.org/2004/02/skos/core#broader> <http://qudt.org/vocab/quantitykind/GaugePressure> ;
                        <https://w3id.org/h2v#appliesToSystem> <https://w3id.org/h2v#WaterPump> .


###  https://w3id.org/h2v/property#WaterPumpInletPressureSet
:WaterPumpInletPressureSet rdf:type owl:NamedIndividual ,
                                    <https://w3id.org/h2v#PropertySet> ;
                           rdfs:label "Water Pump Inlet Pressure Set"^^rdfs:Literal ;
                           <https://w3id.org/h2v#hasMaximumPropertyMember> :WaterPumpMaximumInletPressure ;
                           <https://w3id.org/h2v#hasMinimumPropertyMember> :WaterPumpMinimumInletPressure ;
                           <https://w3id.org/h2v#hasPropertyMember> :WaterPumpMaximumInletPressure ,
                                                                    :WaterPumpMinimumInletPressure .


###  https://w3id.org/h2v/property#WaterPumpMaximumInletPressure
:WaterPumpMaximumInletPressure rdf:type owl:NamedIndividual ,
                                        <https://w3id.org/h2v#StaticProperty> ;
                               <http://qudt.org/schema/qudt/applicableUnit> <https://w3id.org/h2v#BARG> ;
                               rdfs:comment "The Water Pump Maximum Inlet Pressure [barg] of the water pump of the HV is the minimum inlet pressure allowed in the water pump "^^rdfs:Literal ;
                               rdfs:label "Water Pump Maximum Inlet Pressure"^^rdfs:Literal ;
                               <http://www.w3.org/2004/02/skos/core#broader> <http://qudt.org/vocab/quantitykind/GaugePressure> ;
                               <https://w3id.org/h2v#appliesToSystem> <https://w3id.org/h2v#WaterPump> .


###  https://w3id.org/h2v/property#WaterPumpMaximumOutletPressure
:WaterPumpMaximumOutletPressure rdf:type owl:NamedIndividual ,
                                         <https://w3id.org/h2v#StaticProperty> ;
                                <http://qudt.org/schema/qudt/applicableUnit> <https://w3id.org/h2v#BARG> ;
                                rdfs:comment "The Water Pump Maximum Outlet Pressure [barg] of the water pump of the HV is the maximum inlet pressure allowed in the water pump "^^rdfs:Literal ;
                                rdfs:label "Water Pump Maximum Outlet Pressure"^^rdfs:Literal ;
                                <http://www.w3.org/2004/02/skos/core#broader> <http://qudt.org/vocab/quantitykind/GaugePressure> ;
                                <https://w3id.org/h2v#appliesToSystem> <https://w3id.org/h2v#WaterPump> .


###  https://w3id.org/h2v/property#WaterPumpMaximumWaterFlow
:WaterPumpMaximumWaterFlow rdf:type owl:NamedIndividual ,
                                    <https://w3id.org/h2v#StaticProperty> ;
                           <http://qudt.org/schema/qudt/applicableUnit> <http://qudt.org/vocab/unit/L-PER-HR> ;
                           rdfs:comment "The Water Pump Maximum Water Flow [liter/h] of the water pump of the HV is the maximum volume of water per hour ."^^rdfs:Literal ;
                           rdfs:label "Water Pump Maximum Water Flow"^^rdfs:Literal ;
                           <http://www.w3.org/2004/02/skos/core#broader> <http://qudt.org/vocab/quantitykind/VolumePerTime> ;
                           <https://w3id.org/h2v#appliesToSystem> <https://w3id.org/h2v#WaterPump> .


###  https://w3id.org/h2v/property#WaterPumpMinimumInletPressure
:WaterPumpMinimumInletPressure rdf:type owl:NamedIndividual ,
                                        <https://w3id.org/h2v#StaticProperty> ;
                               <http://qudt.org/schema/qudt/applicableUnit> <https://w3id.org/h2v#BARG> ;
                               rdfs:comment "The Water Pump Minimum Inlet Pressure [barg] of the water pump of the HV is the minimum inlet pressure allowed in the water pump "^^rdfs:Literal ;
                               rdfs:label "Water Pump Minimum Inlet Pressure"^^rdfs:Literal ;
                               <http://www.w3.org/2004/02/skos/core#broader> <http://qudt.org/vocab/quantitykind/GaugePressure> ;
                               <https://w3id.org/h2v#appliesToSystem> <https://w3id.org/h2v#WaterPump> .


###  https://w3id.org/h2v/property#WaterPumpMinimumOutletPressure
:WaterPumpMinimumOutletPressure rdf:type owl:NamedIndividual ,
                                         <https://w3id.org/h2v#StaticProperty> ;
                                <http://qudt.org/schema/qudt/applicableUnit> <https://w3id.org/h2v#BARG> ;
                                rdfs:comment "The Water Pump Minimum Outlet Pressure [barg] of the water pump of the HV is the minimum inlet pressure allowed in the water pump "^^rdfs:Literal ;
                                rdfs:label "Water Pump Minimum Outlet Pressure"^^rdfs:Literal ;
                                <http://www.w3.org/2004/02/skos/core#broader> <http://qudt.org/vocab/quantitykind/GaugePressure> ;
                                <https://w3id.org/h2v#appliesToSystem> <https://w3id.org/h2v#WaterPump> .


###  https://w3id.org/h2v/property#WaterPumpMinimumWaterFlow
:WaterPumpMinimumWaterFlow rdf:type owl:NamedIndividual ,
                                    <https://w3id.org/h2v#StaticProperty> ;
                           <http://qudt.org/schema/qudt/applicableUnit> <http://qudt.org/vocab/unit/L-PER-HR> ;
                           rdfs:comment "The Water Pump Minimum Water Flow [liter/h] of the water pump of the HV is the minimum volume of water per hour ."^^rdfs:Literal ;
                           rdfs:label "Water Pump Minimum Water Flow"^^rdfs:Literal ;
                           <http://www.w3.org/2004/02/skos/core#broader> <http://qudt.org/vocab/quantitykind/VolumePerTime> ;
                           <https://w3id.org/h2v#appliesToSystem> <https://w3id.org/h2v#WaterPump> .


###  https://w3id.org/h2v/property#WaterPumpOptimalWaterFlow
:WaterPumpOptimalWaterFlow rdf:type owl:NamedIndividual ,
                                    <https://w3id.org/h2v#StaticProperty> ;
                           <http://qudt.org/schema/qudt/applicableUnit> <http://qudt.org/vocab/unit/L-PER-HR> ;
                           rdfs:comment "The Water Pump Optimal Water Flow [liter/h] of the water pump of the HV is the optimal volume of water per hour ."^^rdfs:Literal ;
                           rdfs:label "Water Pump Optimal Water Flow"^^rdfs:Literal ;
                           <http://www.w3.org/2004/02/skos/core#broader> <http://qudt.org/vocab/quantitykind/VolumePerTime> ;
                           <https://w3id.org/h2v#appliesToSystem> <https://w3id.org/h2v#WaterPump> .


###  https://w3id.org/h2v/property#WaterPumpOutletPressure
:WaterPumpOutletPressure rdf:type owl:NamedIndividual ,
                                  <https://w3id.org/h2v#DynamicProperty> ;
                         <http://qudt.org/schema/qudt/applicableUnit> <https://w3id.org/h2v#BARG> ;
                         rdfs:comment "The Water Pump Outlet Pressure [barg] of the water pump of the HV is  the outlet pressure of the water pump"^^rdfs:Literal ;
                         rdfs:label "Water Pump Outlet Pressure"^^rdfs:Literal ;
                         <http://www.w3.org/2004/02/skos/core#broader> <http://qudt.org/vocab/quantitykind/GaugePressure> ;
                         <https://w3id.org/h2v#appliesToSystem> <https://w3id.org/h2v#WaterPump> .


###  https://w3id.org/h2v/property#WaterPumpOutletPressureSet
:WaterPumpOutletPressureSet rdf:type owl:NamedIndividual ,
                                     <https://w3id.org/h2v#PropertySet> ;
                            rdfs:label "Water Pump Outlet Pressure Set"^^rdfs:Literal ;
                            <https://w3id.org/h2v#hasMaximumPropertyMember> :WaterPumpMaximumOutletPressure ;
                            <https://w3id.org/h2v#hasMinimumPropertyMember> :WaterPumpMinimumOutletPressure ;
                            <https://w3id.org/h2v#hasPropertyMember> :WaterPumpMaximumOutletPressure ,
                                                                     :WaterPumpMinimumOutletPressure .


###  https://w3id.org/h2v/property#WaterPumpWaterFlow
:WaterPumpWaterFlow rdf:type owl:NamedIndividual ,
                             <https://w3id.org/h2v#DynamicProperty> ;
                    <http://qudt.org/schema/qudt/applicableUnit> <http://qudt.org/vocab/unit/L-PER-HR> ;
                    rdfs:comment "The Water Pump Water Flow [liter/h] of the water pump of the HV is the volume of water per hour ."^^rdfs:Literal ;
                    rdfs:label "Water Pump Water Flow"^^rdfs:Literal ;
                    <http://www.w3.org/2004/02/skos/core#broader> <http://qudt.org/vocab/quantitykind/VolumePerTime> ;
                    <https://w3id.org/h2v#appliesToSystem> <https://w3id.org/h2v#WaterPump> .


###  https://w3id.org/h2v/property#WaterPumpWaterFlowSet
:WaterPumpWaterFlowSet rdf:type owl:NamedIndividual ,
                                <https://w3id.org/h2v#PropertySet> ;
                       rdfs:label "Water Pump Water Flow Set"^^rdfs:Literal ;
                       <https://w3id.org/h2v#hasMaximumPropertyMember> :WaterPumpMaximumWaterFlow ;
                       <https://w3id.org/h2v#hasMinimumPropertyMember> :WaterPumpMinimumWaterFlow ;
                       <https://w3id.org/h2v#hasOptimalPropertyMember> :WaterPumpOptimalWaterFlow ;
                       <https://w3id.org/h2v#hasPropertyMember> :WaterPumpMaximumWaterFlow ,
                                                                :WaterPumpMinimumWaterFlow ,
                                                                :WaterPumpOptimalWaterFlow .


###  https://w3id.org/h2v/property#WaterTankCapacitySet
:WaterTankCapacitySet rdf:type owl:NamedIndividual ,
                               <https://w3id.org/h2v#PropertySet> ;
                      rdfs:label "Water Tank Capacity Set"^^rdfs:Literal ;
                      <https://w3id.org/h2v#hasMaximumPropertyMember> :WaterTankMaximumCapacity ;
                      <https://w3id.org/h2v#hasMinimumPropertyMember> :WaterTankMinimumCapacity ;
                      <https://w3id.org/h2v#hasOptimalPropertyMember> :WaterTankOptimalCapacity ;
                      <https://w3id.org/h2v#hasPropertyMember> :WaterTankMaximumCapacity ,
                                                               :WaterTankMinimumCapacity ,
                                                               :WaterTankOptimalCapacity .


###  https://w3id.org/h2v/property#WaterTankMaximumCapacity
:WaterTankMaximumCapacity rdf:type owl:NamedIndividual ,
                                   <https://w3id.org/h2v#StaticProperty> ;
                          <http://qudt.org/schema/qudt/applicableUnit> <http://qudt.org/vocab/unit/L> ;
                          rdfs:comment "The Water Tank Maximum Capacity [liter] of the water tank of the HV is the maximum amount of water it can store."^^rdfs:Literal ;
                          rdfs:label "Water Tank Maximum Capacity"^^rdfs:Literal ;
                          <http://www.w3.org/2004/02/skos/core#broader> <http://qudt.org/vocab/quantitykind/LiquidVolume> ;
                          <https://w3id.org/h2v#appliesToSystem> <https://w3id.org/h2v#WaterTank> .


###  https://w3id.org/h2v/property#WaterTankMinimumCapacity
:WaterTankMinimumCapacity rdf:type owl:NamedIndividual ,
                                   <https://w3id.org/h2v#StaticProperty> ;
                          <http://qudt.org/schema/qudt/applicableUnit> <http://qudt.org/vocab/unit/L> ;
                          rdfs:comment "The Water Tank Minimum Capacity [liter] of the water tank of the HV is the minimum amount of water it can store."^^rdfs:Literal ;
                          rdfs:label "Water Tank Minimum Capacity"^^rdfs:Literal ;
                          <http://www.w3.org/2004/02/skos/core#broader> <http://qudt.org/vocab/quantitykind/LiquidVolume> ;
                          <https://w3id.org/h2v#appliesToSystem> <https://w3id.org/h2v#WaterTank> .


###  https://w3id.org/h2v/property#WaterTankOptimalCapacity
:WaterTankOptimalCapacity rdf:type owl:NamedIndividual ,
                                   <https://w3id.org/h2v#StaticProperty> ;
                          <http://qudt.org/schema/qudt/applicableUnit> <http://qudt.org/vocab/unit/L> ;
                          rdfs:comment "The Water Tank Optimal Capacity [liter] of the water tank of the HV is the optimal amount of water it can store."^^rdfs:Literal ;
                          rdfs:label "Water Tank Optimal Capacity "^^rdfs:Literal ;
                          <http://www.w3.org/2004/02/skos/core#broader> <http://qudt.org/vocab/quantitykind/LiquidVolume> ;
                          <https://w3id.org/h2v#appliesToSystem> <https://w3id.org/h2v#WaterTank> .


###  https://w3id.org/h2v/property#WaterTankOptimalPressure
:WaterTankOptimalPressure rdf:type owl:NamedIndividual ,
                                   <https://w3id.org/h2v#StaticProperty> ;
                          <http://qudt.org/schema/qudt/applicableUnit> <https://w3id.org/h2v#BARG> ;
                          rdfs:comment "The Water Tank Optimal Pressure [barg] of the water tank of the HV is the operating pressure of the tank."^^rdfs:Literal ;
                          rdfs:label "Water Tank Optimal Pressure"^^rdfs:Literal ;
                          <http://www.w3.org/2004/02/skos/core#broader> <http://qudt.org/vocab/quantitykind/GaugePressure> ;
                          <https://w3id.org/h2v#appliesToSystem> <https://w3id.org/h2v#WaterTank> .


###  https://w3id.org/h2v/property#WaterTankOptimalTemperature
:WaterTankOptimalTemperature rdf:type owl:NamedIndividual ,
                                      <https://w3id.org/h2v#StaticProperty> ;
                             <http://qudt.org/schema/qudt/applicableUnit> <http://qudt.org/vocab/unit/DEG_C> ;
                             rdfs:comment "The Water Tank Optimal Temperature [°C] of the water tank of the HV is the operating temperature of the tank."^^rdfs:Literal ;
                             rdfs:label "Water Tank Optimal Temperature "^^rdfs:Literal ;
                             <http://www.w3.org/2004/02/skos/core#broader> <http://qudt.org/vocab/quantitykind/Temperature> ;
                             <https://w3id.org/h2v#appliesToSystem> <https://w3id.org/h2v#WaterTank> .


###  https://w3id.org/h2v/property#WaterTankPressure
:WaterTankPressure rdf:type owl:NamedIndividual ,
                            <https://w3id.org/h2v#DynamicProperty> ;
                   <http://qudt.org/schema/qudt/applicableUnit> <https://w3id.org/h2v#BARG> ;
                   rdfs:comment "The Water Tank Pressure [barg] of the water tank of the HV is the operating pressure of the tank."^^rdfs:Literal ;
                   rdfs:label "Water Tank Pressure"^^rdfs:Literal ;
                   <http://www.w3.org/2004/02/skos/core#broader> <http://qudt.org/vocab/quantitykind/GaugePressure> ;
                   <https://w3id.org/h2v#appliesToSystem> <https://w3id.org/h2v#WaterTank> .


###  https://w3id.org/h2v/property#WaterTankTemperature
:WaterTankTemperature rdf:type owl:NamedIndividual ,
                               <https://w3id.org/h2v#DynamicProperty> ;
                      <http://qudt.org/schema/qudt/applicableUnit> <http://qudt.org/vocab/unit/DEG_C> ;
                      rdfs:comment "The Water Tank Temperature [°C] of the water tank of the HV is the operating temperature of the tank."^^rdfs:Literal ;
                      rdfs:label "Water Tank Temperature "^^rdfs:Literal ;
                      <http://www.w3.org/2004/02/skos/core#broader> <http://qudt.org/vocab/quantitykind/Temperature> ;
                      <https://w3id.org/h2v#appliesToSystem> <https://w3id.org/h2v#WaterTank> .


###  https://w3id.org/h2v/property#WaterTemperature
:WaterTemperature rdf:type owl:NamedIndividual ,
                           <https://w3id.org/h2v#DynamicProperty> ;
                  <http://qudt.org/schema/qudt/applicableUnit> <http://qudt.org/vocab/unit/DEG_C> ;
                  rdfs:comment "The Water Temperature [°C] is the measured temperature of the water in the electrolyzer"^^rdfs:Literal ;
                  rdfs:label "Water Temperature"^^rdfs:Literal ;
                  <http://www.w3.org/2004/02/skos/core#broader> <http://qudt.org/vocab/quantitykind/Temperature> ;
                  <https://w3id.org/h2v#appliesToSystem> <https://w3id.org/h2v#Electrolyzer> .


###  https://w3id.org/h2v/property#WaterTemperatureSet
:WaterTemperatureSet rdf:type owl:NamedIndividual ,
                              <https://w3id.org/h2v#PropertySet> ;
                     rdfs:label "Water Temperature Set"^^rdfs:Literal ;
                     <https://w3id.org/h2v#hasMaximumPropertyMember> :MaximumWaterTemperature ;
                     <https://w3id.org/h2v#hasMinimumPropertyMember> :MinimumWaterTemperature ;
                     <https://w3id.org/h2v#hasPropertyMember> :MaximumWaterTemperature ,
                                                              :MinimumWaterTemperature .


###  https://w3id.org/h2v/property#WobbeIndex
:WobbeIndex rdf:type owl:NamedIndividual ,
                     <https://w3id.org/h2v#DynamicProperty> ;
            <http://qudt.org/schema/qudt/applicableUnit> <http://qudt.org/vocab/unit/MegaJ-PER-M3> ;
            rdfs:comment "The Wobbe Index [MJ/m^3] is the current Wobbe index on the gas network"^^rdfs:Literal ;
            rdfs:label "Wobbe Index"^^rdfs:Literal ;
            <http://www.w3.org/2004/02/skos/core#broader> <http://qudt.org/vocab/quantitykind/EnergyDensity> ;
            <https://w3id.org/h2v#appliesToSystem> <https://w3id.org/h2v#Blender> .


###  https://w3id.org/h2v/property#WobbeIndexToleratedH2Set
:WobbeIndexToleratedH2Set rdf:type owl:NamedIndividual ,
                                   <https://w3id.org/h2v#PropertySet> ;
                          rdfs:label "Wobbe Index Tolerated H2 Set"^^rdfs:Literal ;
                          <https://w3id.org/h2v#hasMaximumPropertyMember> :MaximumWobbeIndexToleratedH2 ;
                          <https://w3id.org/h2v#hasMinimumPropertyMember> :MinimumWobbeIndexToleratedH2 ;
                          <https://w3id.org/h2v#hasPropertyMember> :MaximumWobbeIndexToleratedH2 ,
                                                                   :MinimumWobbeIndexToleratedH2 .


###  Generated by the OWL API (version 5.1.18) https://github.com/owlcs/owlapi/
